<?xml version="1.0"?>
<rdf:RDF xmlns="https://w3id.org/def/gtfs_v1#"
     xml:base="https://w3id.org/def/gtfs_v1"
     xmlns:dc="http://purl.org/dc/elements/1.1/"
     xmlns:XML="http://www.w3.org/XML/1998/"
     xmlns:owl="http://www.w3.org/2002/07/owl#"
     xmlns:rdf="http://www.w3.org/1999/02/22-rdf-syntax-ns#"
     xmlns:xml="http://www.w3.org/XML/1998/namespace"
     xmlns:xsd="http://www.w3.org/2001/XMLSchema#"
     xmlns:gtfs="http://gtfs.org/"
     xmlns:rdfs="http://www.w3.org/2000/01/rdf-schema#">
    <owl:Ontology rdf:about="https://w3id.org/def/gtfs_v1">
        <dc:abstract>The General Transit Feed Specification (GTFS) ontology is a comprehensive framework designed to standardize and represent public transit information in a machine-readable format, facilitating the sharing, analysis, and utilization of transit data across different platforms and applications. This ontology extends the GTFS, a widely adopted format for specifying public transit schedules, routes, and associated geographic information, by providing a semantic model that captures the relationships and constraints inherent in transit data.

At its core, the GTFS ontology defines a set of classes and properties corresponding to the various components of transit data, such as agencies, stops, routes, trips, and schedules. Each class represents a specific aspect of transit information, with properties detailing the attributes and relationships between these aspects. For instance, the ontology includes classes for transit agencies, with properties describing agency details, and for transit routes, with properties defining route characteristics and linking routes to their serving agencies and stops.

The ontology leverages RDF (Resource Description Framework) to define these classes and properties, employing URIs (Uniform Resource Identifiers) to uniquely identify each element. RDFS (RDF Schema) and OWL (Web Ontology Language) are used to express hierarchies, constraints, and logical relationships, enabling sophisticated querying and reasoning over transit data. This semantic richness allows for the detailed representation of transit operations, supporting advanced use cases such as multimodal journey planning, accessibility analysis, and dynamic schedule adjustments.</dc:abstract>
        <dc:creator>Saipraneeth Devunuri</dc:creator>
        <dc:description>This is the ontology created for General Transit Feed Specification(GTFS)</dc:description>
        <dc:language>en</dc:language>
        <dc:rights>https://creativecommons.org/licenses/by-sa/4.0/</dc:rights>
        <dc:source>https://gtfs.org/</dc:source>
        <dc:title>GTFS Ontology</dc:title>
    </owl:Ontology>
    


    <!-- 
    ///////////////////////////////////////////////////////////////////////////////////////
    //
    // Annotation properties
    //
    ///////////////////////////////////////////////////////////////////////////////////////
     -->


    


    <!-- http://gtfs.org/hasAdditionalInfo -->


    <owl:AnnotationProperty rdf:about="http://gtfs.org/hasAdditionalInfo">
        <rdfs:comment>Any additional information about the object</rdfs:comment>
        <rdfs:label xml:lang="en">hasAdditionalInfo</rdfs:label>
        <rdfs:range rdf:resource="http://www.w3.org/2001/XMLSchema#string"/>
        <rdfs:domain rdf:resource="http://gtfs.org/Field"/>
        <rdfs:domain rdf:resource="http://gtfs.org/File"/>
    </owl:AnnotationProperty>
    


    <!-- http://gtfs.org/hasCondition -->


    <owl:AnnotationProperty rdf:about="http://gtfs.org/hasCondition">
        <rdfs:comment>This property specifies the conditions for a File or Field if they are Conditionally Required or Conditionally Forbidden</rdfs:comment>
        <rdfs:label xml:lang="en">hasCondition</rdfs:label>
        <rdfs:range rdf:resource="http://www.w3.org/2001/XMLSchema#string"/>
        <rdfs:domain rdf:resource="http://gtfs.org/Field"/>
        <rdfs:domain rdf:resource="http://gtfs.org/File"/>
    </owl:AnnotationProperty>
    


    <!-- http://gtfs.org/hasEnumValue -->


    <owl:AnnotationProperty rdf:about="http://gtfs.org/hasEnumValue">
        <rdfs:comment>This property specifies the enum value for the named individual within an Enum Class</rdfs:comment>
        <rdfs:label xml:lang="en">hasEnumValue</rdfs:label>
        <rdfs:range rdf:resource="http://www.w3.org/2001/XMLSchema#string"/>
        <rdfs:domain rdf:resource="http://gtfs.org/Enum"/>
    </owl:AnnotationProperty>
    


    <!-- http://gtfs.org/hasExample -->


    <owl:AnnotationProperty rdf:about="http://gtfs.org/hasExample">
        <rdfs:comment>An example FieldType or use case</rdfs:comment>
        <rdfs:label xml:lang="en">hasExample</rdfs:label>
        <rdfs:range rdf:resource="http://www.w3.org/2001/XMLSchema#string"/>
        <rdfs:domain rdf:resource="http://gtfs.org/Field"/>
        <rdfs:domain rdf:resource="http://gtfs.org/File"/>
    </owl:AnnotationProperty>
    


    <!-- http://gtfs.org/isForeignID -->


    <owl:AnnotationProperty rdf:about="http://gtfs.org/isForeignID"/>
    


    <!-- http://gtfs.org/isUniqueID -->


    <owl:AnnotationProperty rdf:about="http://gtfs.org/isUniqueID"/>
    


    <!-- http://purl.org/dc/elements/1.1/abstract -->


    <owl:AnnotationProperty rdf:about="http://purl.org/dc/elements/1.1/abstract"/>
    


    <!-- http://purl.org/dc/elements/1.1/creator -->


    <owl:AnnotationProperty rdf:about="http://purl.org/dc/elements/1.1/creator"/>
    


    <!-- http://purl.org/dc/elements/1.1/description -->


    <owl:AnnotationProperty rdf:about="http://purl.org/dc/elements/1.1/description"/>
    


    <!-- http://purl.org/dc/elements/1.1/language -->


    <owl:AnnotationProperty rdf:about="http://purl.org/dc/elements/1.1/language"/>
    


    <!-- http://purl.org/dc/elements/1.1/rights -->


    <owl:AnnotationProperty rdf:about="http://purl.org/dc/elements/1.1/rights"/>
    


    <!-- http://purl.org/dc/elements/1.1/source -->


    <owl:AnnotationProperty rdf:about="http://purl.org/dc/elements/1.1/source"/>
    


    <!-- http://purl.org/dc/elements/1.1/title -->


    <owl:AnnotationProperty rdf:about="http://purl.org/dc/elements/1.1/title"/>
    


    <!-- http://www.w3.org/XML/1998/namespacelang -->


    <owl:AnnotationProperty rdf:about="http://www.w3.org/XML/1998/namespacelang"/>
    


    <!-- 
    ///////////////////////////////////////////////////////////////////////////////////////
    //
    // Object Properties
    //
    ///////////////////////////////////////////////////////////////////////////////////////
     -->


    


    <!-- http://gtfs.org/hasField -->


    <owl:ObjectProperty rdf:about="http://gtfs.org/hasField">
        <rdfs:subPropertyOf rdf:resource="http://www.w3.org/2002/07/owl#topObjectProperty"/>
        <owl:inverseOf rdf:resource="http://gtfs.org/isFieldOf"/>
        <rdfs:domain rdf:resource="http://gtfs.org/File"/>
        <rdfs:range rdf:resource="http://gtfs.org/Field"/>
        <rdfs:comment>This property links a file to its fields</rdfs:comment>
        <rdfs:label xml:lang="en">hasField</rdfs:label>
    </owl:ObjectProperty>
    


    <!-- http://gtfs.org/hasFile -->


    <owl:ObjectProperty rdf:about="http://gtfs.org/hasFile">
        <rdfs:subPropertyOf rdf:resource="http://www.w3.org/2002/07/owl#topObjectProperty"/>
        <owl:inverseOf rdf:resource="http://gtfs.org/isFileOf"/>
        <rdfs:domain rdf:resource="http://gtfs.org/Specification"/>
        <rdfs:range rdf:resource="http://gtfs.org/File"/>
        <rdfs:comment>This property links the specification to its files</rdfs:comment>
        <rdfs:label>hasFile</rdfs:label>
    </owl:ObjectProperty>
    


    <!-- http://gtfs.org/isConditionallyForbiddenIn -->


    <owl:ObjectProperty rdf:about="http://gtfs.org/isConditionallyForbiddenIn">
        <rdfs:subPropertyOf rdf:resource="http://www.w3.org/2002/07/owl#topObjectProperty"/>
        <rdfs:domain rdf:resource="http://gtfs.org/Field"/>
        <rdfs:domain rdf:resource="http://gtfs.org/File"/>
        <rdfs:range rdf:resource="http://gtfs.org/File"/>
        <rdfs:range rdf:resource="http://gtfs.org/Specification"/>
        <rdfs:comment>The property is used to link file to a specification or field to a file. The file or field must not be included under conditions outlined in the field description.</rdfs:comment>
        <rdfs:label>isConditionallyForbiddenIn</rdfs:label>
    </owl:ObjectProperty>
    


    <!-- http://gtfs.org/isConditionallyRequiredIn -->


    <owl:ObjectProperty rdf:about="http://gtfs.org/isConditionallyRequiredIn">
        <rdfs:subPropertyOf rdf:resource="http://www.w3.org/2002/07/owl#topObjectProperty"/>
        <rdfs:domain rdf:resource="http://gtfs.org/Field"/>
        <rdfs:domain rdf:resource="http://gtfs.org/File"/>
        <rdfs:range rdf:resource="http://gtfs.org/File"/>
        <rdfs:range rdf:resource="http://gtfs.org/Specification"/>
        <rdfs:comment>The property is used to link file to a specification or field to a file. The file or field must be included under conditions outlined in the field description.</rdfs:comment>
        <rdfs:label>isConditionallyRequiredIn</rdfs:label>
    </owl:ObjectProperty>
    


    <!-- http://gtfs.org/isFieldOf -->


    <owl:ObjectProperty rdf:about="http://gtfs.org/isFieldOf">
        <rdfs:domain rdf:resource="http://gtfs.org/Field"/>
        <rdfs:range rdf:resource="http://gtfs.org/File"/>
        <rdfs:comment>This property links a field back to its file</rdfs:comment>
        <rdfs:label xml:lang="en">isFieldOf</rdfs:label>
    </owl:ObjectProperty>
    


    <!-- http://gtfs.org/isFileOf -->


    <owl:ObjectProperty rdf:about="http://gtfs.org/isFileOf">
        <rdfs:subPropertyOf rdf:resource="http://www.w3.org/2002/07/owl#topObjectProperty"/>
        <rdfs:domain rdf:resource="http://gtfs.org/File"/>
        <rdfs:range rdf:resource="http://gtfs.org/Specification"/>
        <rdfs:comment>This property links a file to its specification</rdfs:comment>
        <rdfs:label>isFileOf</rdfs:label>
    </owl:ObjectProperty>
    


    <!-- http://gtfs.org/isOptionalIn -->


    <owl:ObjectProperty rdf:about="http://gtfs.org/isOptionalIn">
        <rdfs:subPropertyOf rdf:resource="http://www.w3.org/2002/07/owl#topObjectProperty"/>
        <rdfs:domain rdf:resource="http://gtfs.org/Field"/>
        <rdfs:domain rdf:resource="http://gtfs.org/File"/>
        <rdfs:range rdf:resource="http://gtfs.org/File"/>
        <rdfs:range rdf:resource="http://gtfs.org/Specification"/>
        <rdfs:comment>The property is used to link field to a file or file to specification. The file or field may be omitted from the dataset.</rdfs:comment>
        <rdfs:label>isOptionalIn</rdfs:label>
    </owl:ObjectProperty>
    


    <!-- http://gtfs.org/isPresence -->


    <owl:ObjectProperty rdf:about="http://gtfs.org/isPresence">
        <rdfs:subPropertyOf rdf:resource="http://www.w3.org/2002/07/owl#topObjectProperty"/>
        <rdfs:domain rdf:resource="http://gtfs.org/Field"/>
        <rdfs:domain rdf:resource="http://gtfs.org/File"/>
        <rdfs:range rdf:resource="http://gtfs.org/PresenceCondition"/>
        <rdfs:comment>This property links a file or field to its PresenceCondition.</rdfs:comment>
        <rdfs:label xml:lang="en">isPresence</rdfs:label>
    </owl:ObjectProperty>
    


    <!-- http://gtfs.org/isRecommendedIn -->


    <owl:ObjectProperty rdf:about="http://gtfs.org/isRecommendedIn">
        <rdfs:subPropertyOf rdf:resource="http://www.w3.org/2002/07/owl#topObjectProperty"/>
        <rdfs:domain rdf:resource="http://gtfs.org/Field"/>
        <rdfs:domain rdf:resource="http://gtfs.org/File"/>
        <rdfs:range rdf:resource="http://gtfs.org/File"/>
        <rdfs:range rdf:resource="http://gtfs.org/Specification"/>
        <rdfs:comment>The field or file may be omitted from the dataset, but it is a best practice to include it. Before omitting this field or file, the best practice should be carefully evaluated and the full implications of omission should be understood.</rdfs:comment>
        <rdfs:label>isRecommendedIn</rdfs:label>
    </owl:ObjectProperty>
    


    <!-- http://gtfs.org/isRequiredIn -->


    <owl:ObjectProperty rdf:about="http://gtfs.org/isRequiredIn">
        <rdfs:subPropertyOf rdf:resource="http://www.w3.org/2002/07/owl#topObjectProperty"/>
        <rdfs:domain rdf:resource="http://gtfs.org/Field"/>
        <rdfs:domain rdf:resource="http://gtfs.org/File"/>
        <rdfs:range rdf:resource="http://gtfs.org/File"/>
        <rdfs:range rdf:resource="http://gtfs.org/Specification"/>
        <rdfs:comment>The property is used to link file to a specification or field to a file. The file or field must be included in the dataset and contain a valid value for each record.</rdfs:comment>
        <rdfs:label>isRequiredIn</rdfs:label>
    </owl:ObjectProperty>
    


    <!-- http://gtfs.org/isType -->


    <owl:ObjectProperty rdf:about="http://gtfs.org/isType">
        <rdfs:subPropertyOf rdf:resource="http://www.w3.org/2002/07/owl#topObjectProperty"/>
        <rdfs:domain rdf:resource="http://gtfs.org/Field"/>
        <rdfs:range rdf:resource="http://gtfs.org/FieldType"/>
        <rdfs:comment>This property is used to specify the FieldType for a Field</rdfs:comment>
        <rdfs:label>isType</rdfs:label>
    </owl:ObjectProperty>
    


    <!-- 
    ///////////////////////////////////////////////////////////////////////////////////////
    //
    // Data properties
    //
    ///////////////////////////////////////////////////////////////////////////////////////
     -->


    


    <!-- http://www.w3.org/2002/07/owl#topDataProperty -->


    <rdf:Description rdf:about="http://www.w3.org/2002/07/owl#topDataProperty">
        <rdf:type rdf:resource="http://www.w3.org/2002/07/owl#FunctionalProperty"/>
        <rdfs:domain rdf:resource="http://gtfs.org/Field"/>
        <rdfs:domain rdf:resource="http://gtfs.org/File"/>
    </rdf:Description>
    


    <!-- 
    ///////////////////////////////////////////////////////////////////////////////////////
    //
    // Classes
    //
    ///////////////////////////////////////////////////////////////////////////////////////
     -->


    


    <!-- http://gtfs.org/BikesAllowedEnum -->


    <owl:Class rdf:about="http://gtfs.org/BikesAllowedEnum">
        <rdfs:subClassOf rdf:resource="http://gtfs.org/Enum"/>
    </owl:Class>
    


    <!-- http://gtfs.org/ContinuousDropOffEnum -->


    <owl:Class rdf:about="http://gtfs.org/ContinuousDropOffEnum">
        <rdfs:subClassOf rdf:resource="http://gtfs.org/Enum"/>
    </owl:Class>
    


    <!-- http://gtfs.org/ContinuousPickupEnum -->


    <owl:Class rdf:about="http://gtfs.org/ContinuousPickupEnum">
        <rdfs:subClassOf rdf:resource="http://gtfs.org/Enum"/>
    </owl:Class>
    


    <!-- http://gtfs.org/CurrencyAmount -->


    <owl:Class rdf:about="http://gtfs.org/CurrencyAmount">
        <rdfs:subClassOf rdf:resource="http://gtfs.org/FieldType"/>
    </owl:Class>
    


    <!-- http://gtfs.org/Dataset -->


    <owl:Class rdf:about="http://gtfs.org/Dataset">
        <gtfs:hasExample>https://www.agency.org/gtfs/gtfs.zip</gtfs:hasExample>
        <rdfs:comment>A complete set of files defined by this specification reference. Altering the dataset creates a new version of the dataset. Datasets should be published at a public, permanent URL, including the zip file name.</rdfs:comment>
        <rdfs:label>Dataset</rdfs:label>
    </owl:Class>
    


    <!-- http://gtfs.org/Date -->


    <owl:Class rdf:about="http://gtfs.org/Date">
        <rdfs:subClassOf rdf:resource="http://gtfs.org/FieldType"/>
    </owl:Class>
    


    <!-- http://gtfs.org/DirectionIdEnum -->


    <owl:Class rdf:about="http://gtfs.org/DirectionIdEnum">
        <rdfs:subClassOf rdf:resource="http://gtfs.org/Enum"/>
    </owl:Class>
    


    <!-- http://gtfs.org/DropOffTypeEnum -->


    <owl:Class rdf:about="http://gtfs.org/DropOffTypeEnum">
        <rdfs:subClassOf rdf:resource="http://gtfs.org/Enum"/>
    </owl:Class>
    


    <!-- http://gtfs.org/DurationLimitTypeEnum -->


    <owl:Class rdf:about="http://gtfs.org/DurationLimitTypeEnum">
        <rdfs:subClassOf rdf:resource="http://gtfs.org/Enum"/>
    </owl:Class>
    


    <!-- http://gtfs.org/Email -->


    <owl:Class rdf:about="http://gtfs.org/Email">
        <rdfs:subClassOf rdf:resource="http://gtfs.org/FieldType"/>
    </owl:Class>
    


    <!-- http://gtfs.org/Enum -->


    <owl:Class rdf:about="http://gtfs.org/Enum">
        <owl:equivalentClass rdf:resource="http://schema.org/Enumeration"/>
        <rdfs:subClassOf rdf:resource="http://gtfs.org/FieldType"/>
        <rdfs:comment xml:lang="en">An option from a set of predefined constants defined in the &quot;Description&quot; column.</rdfs:comment>
        <rdfs:label xml:lang="en">Enum</rdfs:label>
    </owl:Class>
    


    <!-- http://gtfs.org/ExactTimesEnum -->


    <owl:Class rdf:about="http://gtfs.org/ExactTimesEnum">
        <rdfs:subClassOf rdf:resource="http://gtfs.org/Enum"/>
    </owl:Class>
    


    <!-- http://gtfs.org/ExceptionTypeEnum -->


    <owl:Class rdf:about="http://gtfs.org/ExceptionTypeEnum">
        <rdfs:subClassOf rdf:resource="http://gtfs.org/Enum"/>
    </owl:Class>
    


    <!-- http://gtfs.org/FareMediaTypeEnum -->


    <owl:Class rdf:about="http://gtfs.org/FareMediaTypeEnum">
        <rdfs:subClassOf rdf:resource="http://gtfs.org/Enum"/>
    </owl:Class>
    


    <!-- http://gtfs.org/FareProduct -->


    <owl:Class rdf:about="http://gtfs.org/FareProduct">
        <rdfs:comment>Purchasable fare products that can be used to pay for or validate travel.</rdfs:comment>
        <rdfs:label>FareProduct</rdfs:label>
    </owl:Class>
    


    <!-- http://gtfs.org/FareTransferTypeEnum -->


    <owl:Class rdf:about="http://gtfs.org/FareTransferTypeEnum">
        <rdfs:subClassOf rdf:resource="http://gtfs.org/Enum"/>
    </owl:Class>
    


    <!-- http://gtfs.org/Field -->


    <owl:Class rdf:about="http://gtfs.org/Field">
        <rdfs:subClassOf rdf:resource="http://schema.org/Intangible"/>
        <rdfs:comment>A field refers to a single item of data or a column header within a GTFS file</rdfs:comment>
        <rdfs:comment>A property of an object or entity. Represented, in a table, as a column. The field exists if added in a file as a header. It may or may not have field values defined.</rdfs:comment>
        <rdfs:label xml:lang="en">Field</rdfs:label>
        <rdfs:label>Field</rdfs:label>
    </owl:Class>
    


    <!-- http://gtfs.org/FieldType -->


    <owl:Class rdf:about="http://gtfs.org/FieldType">
        <rdfs:subClassOf rdf:resource="http://schema.org/Intangible"/>
        <rdfs:label xml:lang="en">FieldType</rdfs:label>
    </owl:Class>
    


    <!-- http://gtfs.org/FieldValue -->


    <owl:Class rdf:about="http://gtfs.org/FieldValue">
        <rdfs:comment>An individual entry in a field. Represented, in a table, as a single cell.</rdfs:comment>
        <rdfs:label>FieldValue</rdfs:label>
    </owl:Class>
    


    <!-- http://gtfs.org/File -->


    <owl:Class rdf:about="http://gtfs.org/File">
        <rdfs:subClassOf rdf:resource="http://schema.org/Intangible"/>
        <rdfs:comment>A File refers to a single file within the GTFS feed</rdfs:comment>
        <rdfs:label xml:lang="en">File</rdfs:label>
    </owl:Class>
    


    <!-- http://gtfs.org/Float -->


    <owl:Class rdf:about="http://gtfs.org/Float">
        <rdfs:subClassOf rdf:resource="http://gtfs.org/FieldType"/>
    </owl:Class>
    


    <!-- http://gtfs.org/FridayEnum -->


    <owl:Class rdf:about="http://gtfs.org/FridayEnum">
        <rdfs:subClassOf rdf:resource="http://gtfs.org/Enum"/>
    </owl:Class>
    


    <!-- http://gtfs.org/ID -->


    <owl:Class rdf:about="http://gtfs.org/ID">
        <rdfs:subClassOf rdf:resource="http://gtfs.org/FieldType"/>
    </owl:Class>
    


    <!-- http://gtfs.org/Integer -->


    <owl:Class rdf:about="http://gtfs.org/Integer">
        <rdfs:subClassOf rdf:resource="http://gtfs.org/FieldType"/>
    </owl:Class>
    


    <!-- http://gtfs.org/IsAuthorityEnum -->


    <owl:Class rdf:about="http://gtfs.org/IsAuthorityEnum">
        <rdfs:subClassOf rdf:resource="http://gtfs.org/Enum"/>
    </owl:Class>
    


    <!-- http://gtfs.org/IsBidirectionalEnum -->


    <owl:Class rdf:about="http://gtfs.org/IsBidirectionalEnum">
        <rdfs:subClassOf rdf:resource="http://gtfs.org/Enum"/>
    </owl:Class>
    


    <!-- http://gtfs.org/IsOperatorEnum -->


    <owl:Class rdf:about="http://gtfs.org/IsOperatorEnum">
        <rdfs:subClassOf rdf:resource="http://gtfs.org/Enum"/>
    </owl:Class>
    


    <!-- http://gtfs.org/IsProducerEnum -->


    <owl:Class rdf:about="http://gtfs.org/IsProducerEnum">
        <rdfs:subClassOf rdf:resource="http://gtfs.org/Enum"/>
    </owl:Class>
    


    <!-- http://gtfs.org/Journey -->


    <owl:Class rdf:about="http://gtfs.org/Journey">
        <rdfs:comment>Overall travel from origin to destination, including all legs and transfers in-between.</rdfs:comment>
        <rdfs:label>Journey</rdfs:label>
    </owl:Class>
    


    <!-- http://gtfs.org/LanguageCode -->


    <owl:Class rdf:about="http://gtfs.org/LanguageCode">
        <rdfs:subClassOf rdf:resource="http://gtfs.org/FieldType"/>
    </owl:Class>
    


    <!-- http://gtfs.org/Latitude -->


    <owl:Class rdf:about="http://gtfs.org/Latitude">
        <rdfs:subClassOf rdf:resource="http://gtfs.org/FieldType"/>
    </owl:Class>
    


    <!-- http://gtfs.org/Leg -->


    <owl:Class rdf:about="http://gtfs.org/Leg">
        <rdfs:comment>Travel in which a rider boards and alights between a pair of subsequent locations along a trip.</rdfs:comment>
        <rdfs:label>Leg</rdfs:label>
    </owl:Class>
    


    <!-- http://gtfs.org/LocationTypeEnum -->


    <owl:Class rdf:about="http://gtfs.org/LocationTypeEnum">
        <rdfs:subClassOf rdf:resource="http://gtfs.org/Enum"/>
    </owl:Class>
    


    <!-- http://gtfs.org/Longitude -->


    <owl:Class rdf:about="http://gtfs.org/Longitude">
        <rdfs:subClassOf rdf:resource="http://gtfs.org/FieldType"/>
    </owl:Class>
    


    <!-- http://gtfs.org/MondayEnum -->


    <owl:Class rdf:about="http://gtfs.org/MondayEnum">
        <rdfs:subClassOf rdf:resource="http://gtfs.org/Enum"/>
    </owl:Class>
    


    <!-- http://gtfs.org/PathwayModeEnum -->


    <owl:Class rdf:about="http://gtfs.org/PathwayModeEnum">
        <rdfs:subClassOf rdf:resource="http://gtfs.org/Enum"/>
    </owl:Class>
    


    <!-- http://gtfs.org/PaymentMethodEnum -->


    <owl:Class rdf:about="http://gtfs.org/PaymentMethodEnum">
        <rdfs:subClassOf rdf:resource="http://gtfs.org/Enum"/>
    </owl:Class>
    


    <!-- http://gtfs.org/PhoneNumber -->


    <owl:Class rdf:about="http://gtfs.org/PhoneNumber">
        <rdfs:subClassOf rdf:resource="http://gtfs.org/FieldType"/>
    </owl:Class>
    


    <!-- http://gtfs.org/PickupTypeEnum -->


    <owl:Class rdf:about="http://gtfs.org/PickupTypeEnum">
        <rdfs:subClassOf rdf:resource="http://gtfs.org/Enum"/>
    </owl:Class>
    


    <!-- http://gtfs.org/PresenceCondition -->


    <owl:Class rdf:about="http://gtfs.org/PresenceCondition">
        <rdfs:subClassOf rdf:resource="http://schema.org/Enumeration"/>
        <rdfs:comment>The presence conditions applicable to  Files and Fields</rdfs:comment>
        <rdfs:label xml:lang="en">PresenceCondition</rdfs:label>
    </owl:Class>
    


    <!-- http://gtfs.org/Recommended -->


    <owl:Class rdf:about="http://gtfs.org/Recommended">
        <rdfs:subClassOf rdf:resource="http://gtfs.org/PresenceCondition"/>
    </owl:Class>
    


    <!-- http://gtfs.org/Record -->


    <owl:Class rdf:about="http://gtfs.org/Record">
        <rdfs:comment>A basic data structure comprised of a number of different field values describing a single entity (e.g. transit agency, stop, route, etc.). Represented, in a table, as a row.</rdfs:comment>
        <rdfs:label>Record</rdfs:label>
    </owl:Class>
    


    <!-- http://gtfs.org/RouteTypeEnum -->


    <owl:Class rdf:about="http://gtfs.org/RouteTypeEnum">
        <rdfs:subClassOf rdf:resource="http://gtfs.org/Enum"/>
    </owl:Class>
    


    <!-- http://gtfs.org/SaturdayEnum -->


    <owl:Class rdf:about="http://gtfs.org/SaturdayEnum">
        <rdfs:subClassOf rdf:resource="http://gtfs.org/Enum"/>
    </owl:Class>
    


    <!-- http://gtfs.org/ServiceDay -->


    <owl:Class rdf:about="http://gtfs.org/ServiceDay">
        <gtfs:hasExample>Service that runs from 08:00:00 on Friday to 02:00:00 on Saturday could be denoted as running from 08:00:00 to 26:00:00 on a single service day.</gtfs:hasExample>
        <rdfs:comment>A time period used to indicate route scheduling. Service days often do not correspond with calendar days and may exceed 24:00:00 if service begins on one day and ends on a following day.</rdfs:comment>
        <rdfs:label>ServiceDay</rdfs:label>
    </owl:Class>
    


    <!-- http://gtfs.org/Specification -->


    <owl:Class rdf:about="http://gtfs.org/Specification">
        <rdfs:subClassOf rdf:resource="http://schema.org/Intangible"/>
        <dc:language>en</dc:language>
        <rdfs:comment>The main class for the GTFS Specification. Can be used for GTFS-Static, GTFS-Realtime, GTFS-Flex, etc.</rdfs:comment>
        <rdfs:label>Specification</rdfs:label>
    </owl:Class>
    


    <!-- http://gtfs.org/SubJourney -->


    <owl:Class rdf:about="http://gtfs.org/SubJourney">
        <rdfs:comment>Two or more legs that comprise a subset of a journey.</rdfs:comment>
        <rdfs:label>SubJourney</rdfs:label>
    </owl:Class>
    


    <!-- http://gtfs.org/SundayEnum -->


    <owl:Class rdf:about="http://gtfs.org/SundayEnum">
        <rdfs:subClassOf rdf:resource="http://gtfs.org/Enum"/>
    </owl:Class>
    


    <!-- http://gtfs.org/TableNameEnum -->


    <owl:Class rdf:about="http://gtfs.org/TableNameEnum">
        <rdfs:subClassOf rdf:resource="http://gtfs.org/Enum"/>
    </owl:Class>
    


    <!-- http://gtfs.org/Text -->


    <owl:Class rdf:about="http://gtfs.org/Text">
        <rdfs:subClassOf rdf:resource="http://gtfs.org/FieldType"/>
    </owl:Class>
    


    <!-- http://gtfs.org/TextToSpeechField -->


    <owl:Class rdf:about="http://gtfs.org/TextToSpeechField">
        <rdfs:comment>A field that should contain the same information as its parent field. It is aimed to be read as text-to-speech, with abbreviations either removed or kept for proper pronunciation.</rdfs:comment>
        <rdfs:label>TextToSpeechField</rdfs:label>
    </owl:Class>
    


    <!-- http://gtfs.org/ThursdayEnum -->


    <owl:Class rdf:about="http://gtfs.org/ThursdayEnum">
        <rdfs:subClassOf rdf:resource="http://gtfs.org/Enum"/>
    </owl:Class>
    


    <!-- http://gtfs.org/Time -->


    <owl:Class rdf:about="http://gtfs.org/Time">
        <rdfs:subClassOf rdf:resource="http://gtfs.org/FieldType"/>
    </owl:Class>
    


    <!-- http://gtfs.org/TimeZone -->


    <owl:Class rdf:about="http://gtfs.org/TimeZone">
        <rdfs:subClassOf rdf:resource="http://gtfs.org/FieldType"/>
    </owl:Class>
    


    <!-- http://gtfs.org/TimepointEnum -->


    <owl:Class rdf:about="http://gtfs.org/TimepointEnum">
        <rdfs:subClassOf rdf:resource="http://gtfs.org/Enum"/>
    </owl:Class>
    


    <!-- http://gtfs.org/TransferTypeEnum -->


    <owl:Class rdf:about="http://gtfs.org/TransferTypeEnum">
        <rdfs:subClassOf rdf:resource="http://gtfs.org/Enum"/>
    </owl:Class>
    


    <!-- http://gtfs.org/TransfersEnum -->


    <owl:Class rdf:about="http://gtfs.org/TransfersEnum">
        <rdfs:subClassOf rdf:resource="http://gtfs.org/Enum"/>
    </owl:Class>
    


    <!-- http://gtfs.org/TuesdayEnum -->


    <owl:Class rdf:about="http://gtfs.org/TuesdayEnum">
        <rdfs:subClassOf rdf:resource="http://gtfs.org/Enum"/>
    </owl:Class>
    


    <!-- http://gtfs.org/URL -->


    <owl:Class rdf:about="http://gtfs.org/URL">
        <rdfs:subClassOf rdf:resource="http://gtfs.org/FieldType"/>
    </owl:Class>
    


    <!-- http://gtfs.org/WednesdayEnum -->


    <owl:Class rdf:about="http://gtfs.org/WednesdayEnum">
        <rdfs:subClassOf rdf:resource="http://gtfs.org/Enum"/>
    </owl:Class>
    


    <!-- http://gtfs.org/WheelchairAccessibleEnum -->


    <owl:Class rdf:about="http://gtfs.org/WheelchairAccessibleEnum">
        <rdfs:subClassOf rdf:resource="http://gtfs.org/Enum"/>
    </owl:Class>
    


    <!-- http://gtfs.org/WheelchairBoardingEnum -->


    <owl:Class rdf:about="http://gtfs.org/WheelchairBoardingEnum">
        <rdfs:subClassOf rdf:resource="http://gtfs.org/Enum"/>
    </owl:Class>
    


    <!-- http://schema.org/Enumeration -->


    <owl:Class rdf:about="http://schema.org/Enumeration">
        <rdfs:subClassOf rdf:resource="http://schema.org/Intangible"/>
        <rdfs:label xml:lang="en">Enumeration</rdfs:label>
    </owl:Class>
    


    <!-- http://schema.org/Intangible -->


    <owl:Class rdf:about="http://schema.org/Intangible">
        <rdfs:label xml:lang="en">Intangible</rdfs:label>
    </owl:Class>
    


    <!-- 
    ///////////////////////////////////////////////////////////////////////////////////////
    //
    // Individuals
    //
    ///////////////////////////////////////////////////////////////////////////////////////
     -->


    


    <!-- http://gtfs.org/BikesAllowedEnum -->


    <owl:NamedIndividual rdf:about="http://gtfs.org/BikesAllowedEnum"/>
    


    <!-- http://gtfs.org/Color -->


    <owl:NamedIndividual rdf:about="http://gtfs.org/Color"/>
    


    <!-- http://gtfs.org/ConditionallyRequired -->


    <owl:NamedIndividual rdf:about="http://gtfs.org/ConditionallyRequired"/>
    


    <!-- http://gtfs.org/ContinuousDropOffEnum -->


    <owl:NamedIndividual rdf:about="http://gtfs.org/ContinuousDropOffEnum"/>
    


    <!-- http://gtfs.org/ContinuousPickupEnum -->


    <owl:NamedIndividual rdf:about="http://gtfs.org/ContinuousPickupEnum"/>
    


    <!-- http://gtfs.org/CurrencyAmount -->


    <owl:NamedIndividual rdf:about="http://gtfs.org/CurrencyAmount"/>
    


    <!-- http://gtfs.org/CurrencyCode -->


    <owl:NamedIndividual rdf:about="http://gtfs.org/CurrencyCode"/>
    


    <!-- http://gtfs.org/Date -->


    <owl:NamedIndividual rdf:about="http://gtfs.org/Date"/>
    


    <!-- http://gtfs.org/DirectionIdEnum -->


    <owl:NamedIndividual rdf:about="http://gtfs.org/DirectionIdEnum"/>
    


    <!-- http://gtfs.org/DropOffTypeEnum -->


    <owl:NamedIndividual rdf:about="http://gtfs.org/DropOffTypeEnum"/>
    


    <!-- http://gtfs.org/DurationLimitTypeEnum -->


    <owl:NamedIndividual rdf:about="http://gtfs.org/DurationLimitTypeEnum"/>
    


    <!-- http://gtfs.org/Email -->


    <owl:NamedIndividual rdf:about="http://gtfs.org/Email"/>
    


    <!-- http://gtfs.org/ExactTimesEnum -->


    <owl:NamedIndividual rdf:about="http://gtfs.org/ExactTimesEnum"/>
    


    <!-- http://gtfs.org/ExceptionTypeEnum -->


    <owl:NamedIndividual rdf:about="http://gtfs.org/ExceptionTypeEnum"/>
    


    <!-- http://gtfs.org/FareMediaTypeEnum -->


    <owl:NamedIndividual rdf:about="http://gtfs.org/FareMediaTypeEnum"/>
    


    <!-- http://gtfs.org/FareTransferTypeEnum -->


    <owl:NamedIndividual rdf:about="http://gtfs.org/FareTransferTypeEnum"/>
    


    <!-- http://gtfs.org/Float -->


    <owl:NamedIndividual rdf:about="http://gtfs.org/Float"/>
    


    <!-- http://gtfs.org/FridayEnum -->


    <owl:NamedIndividual rdf:about="http://gtfs.org/FridayEnum"/>
    


    <!-- http://gtfs.org/GTFS_Static -->


    <owl:NamedIndividual rdf:about="http://gtfs.org/GTFS_Static">
        <rdf:type rdf:resource="http://gtfs.org/Specification"/>
        <gtfs:hasFile rdf:resource="http://gtfs.org/agency.txt"/>
        <gtfs:hasFile rdf:resource="http://gtfs.org/areas.txt"/>
        <gtfs:hasFile rdf:resource="http://gtfs.org/attributions.txt"/>
        <gtfs:hasFile rdf:resource="http://gtfs.org/calendar.txt"/>
        <gtfs:hasFile rdf:resource="http://gtfs.org/calendar_dates.txt"/>
        <gtfs:hasFile rdf:resource="http://gtfs.org/fare_attributes.txt"/>
        <gtfs:hasFile rdf:resource="http://gtfs.org/fare_leg_rules.txt"/>
        <gtfs:hasFile rdf:resource="http://gtfs.org/fare_media.txt"/>
        <gtfs:hasFile rdf:resource="http://gtfs.org/fare_products.txt"/>
        <gtfs:hasFile rdf:resource="http://gtfs.org/fare_rules.txt"/>
        <gtfs:hasFile rdf:resource="http://gtfs.org/fare_transfer_rules.txt"/>
        <gtfs:hasFile rdf:resource="http://gtfs.org/feed_info.txt"/>
        <gtfs:hasFile rdf:resource="http://gtfs.org/frequencies.txt"/>
        <gtfs:hasFile rdf:resource="http://gtfs.org/levels.txt"/>
        <gtfs:hasFile rdf:resource="http://gtfs.org/pathways.txt"/>
        <gtfs:hasFile rdf:resource="http://gtfs.org/routes.txt"/>
        <gtfs:hasFile rdf:resource="http://gtfs.org/shapes.txt"/>
        <gtfs:hasFile rdf:resource="http://gtfs.org/stop_areas.txt"/>
        <gtfs:hasFile rdf:resource="http://gtfs.org/stop_times.txt"/>
        <gtfs:hasFile rdf:resource="http://gtfs.org/stops.txt"/>
        <gtfs:hasFile rdf:resource="http://gtfs.org/timeframes.txt"/>
        <gtfs:hasFile rdf:resource="http://gtfs.org/transfers.txt"/>
        <gtfs:hasFile rdf:resource="http://gtfs.org/translations.txt"/>
        <gtfs:hasFile rdf:resource="http://gtfs.org/trips.txt"/>
        <rdfs:comment>GTFS Static contains information about routes, schedules, fares, and geographic transit details, and it is presented in simple text files. This straightforward format allows for easy creation and maintenance without relying on complex or proprietary software.</rdfs:comment>
        <rdfs:label>GTFS_Static</rdfs:label>
        <XML:namespacelang>en</XML:namespacelang>
    </owl:NamedIndividual>
    


    <!-- http://gtfs.org/ID -->


    <owl:NamedIndividual rdf:about="http://gtfs.org/ID"/>
    


    <!-- http://gtfs.org/Integer -->


    <owl:NamedIndividual rdf:about="http://gtfs.org/Integer"/>
    


    <!-- http://gtfs.org/IsAuthorityEnum -->


    <owl:NamedIndividual rdf:about="http://gtfs.org/IsAuthorityEnum"/>
    


    <!-- http://gtfs.org/IsBidirectionalEnum -->


    <owl:NamedIndividual rdf:about="http://gtfs.org/IsBidirectionalEnum"/>
    


    <!-- http://gtfs.org/IsOperatorEnum -->


    <owl:NamedIndividual rdf:about="http://gtfs.org/IsOperatorEnum"/>
    


    <!-- http://gtfs.org/IsProducerEnum -->


    <owl:NamedIndividual rdf:about="http://gtfs.org/IsProducerEnum"/>
    


    <!-- http://gtfs.org/LanguageCode -->


    <owl:NamedIndividual rdf:about="http://gtfs.org/LanguageCode"/>
    


    <!-- http://gtfs.org/Latitude -->


    <owl:NamedIndividual rdf:about="http://gtfs.org/Latitude"/>
    


    <!-- http://gtfs.org/LocationTypeEnum -->


    <owl:NamedIndividual rdf:about="http://gtfs.org/LocationTypeEnum"/>
    


    <!-- http://gtfs.org/Longitude -->


    <owl:NamedIndividual rdf:about="http://gtfs.org/Longitude"/>
    


    <!-- http://gtfs.org/MondayEnum -->


    <owl:NamedIndividual rdf:about="http://gtfs.org/MondayEnum"/>
    


    <!-- http://gtfs.org/Optional -->


    <owl:NamedIndividual rdf:about="http://gtfs.org/Optional"/>
    


    <!-- http://gtfs.org/PathwayModeEnum -->


    <owl:NamedIndividual rdf:about="http://gtfs.org/PathwayModeEnum"/>
    


    <!-- http://gtfs.org/PaymentMethodEnum -->


    <owl:NamedIndividual rdf:about="http://gtfs.org/PaymentMethodEnum"/>
    


    <!-- http://gtfs.org/PhoneNumber -->


    <owl:NamedIndividual rdf:about="http://gtfs.org/PhoneNumber"/>
    


    <!-- http://gtfs.org/PickupTypeEnum -->


    <owl:NamedIndividual rdf:about="http://gtfs.org/PickupTypeEnum"/>
    


    <!-- http://gtfs.org/Recommended -->


    <owl:NamedIndividual rdf:about="http://gtfs.org/Recommended"/>
    


    <!-- http://gtfs.org/Required -->


    <owl:NamedIndividual rdf:about="http://gtfs.org/Required"/>
    


    <!-- http://gtfs.org/RouteTypeEnum -->


    <owl:NamedIndividual rdf:about="http://gtfs.org/RouteTypeEnum"/>
    


    <!-- http://gtfs.org/SaturdayEnum -->


    <owl:NamedIndividual rdf:about="http://gtfs.org/SaturdayEnum"/>
    


    <!-- http://gtfs.org/SundayEnum -->


    <owl:NamedIndividual rdf:about="http://gtfs.org/SundayEnum"/>
    


    <!-- http://gtfs.org/TableNameEnum -->


    <owl:NamedIndividual rdf:about="http://gtfs.org/TableNameEnum"/>
    


    <!-- http://gtfs.org/Text -->


    <owl:NamedIndividual rdf:about="http://gtfs.org/Text"/>
    


    <!-- http://gtfs.org/ThursdayEnum -->


    <owl:NamedIndividual rdf:about="http://gtfs.org/ThursdayEnum"/>
    


    <!-- http://gtfs.org/Time -->


    <owl:NamedIndividual rdf:about="http://gtfs.org/Time"/>
    


    <!-- http://gtfs.org/TimeZone -->


    <owl:NamedIndividual rdf:about="http://gtfs.org/TimeZone"/>
    


    <!-- http://gtfs.org/TimepointEnum -->


    <owl:NamedIndividual rdf:about="http://gtfs.org/TimepointEnum"/>
    


    <!-- http://gtfs.org/TransferTypeEnum -->


    <owl:NamedIndividual rdf:about="http://gtfs.org/TransferTypeEnum"/>
    


    <!-- http://gtfs.org/TransfersEnum -->


    <owl:NamedIndividual rdf:about="http://gtfs.org/TransfersEnum"/>
    


    <!-- http://gtfs.org/TuesdayEnum -->


    <owl:NamedIndividual rdf:about="http://gtfs.org/TuesdayEnum"/>
    


    <!-- http://gtfs.org/URL -->


    <owl:NamedIndividual rdf:about="http://gtfs.org/URL"/>
    


    <!-- http://gtfs.org/WednesdayEnum -->


    <owl:NamedIndividual rdf:about="http://gtfs.org/WednesdayEnum"/>
    


    <!-- http://gtfs.org/WheelchairAccessibleEnum -->


    <owl:NamedIndividual rdf:about="http://gtfs.org/WheelchairAccessibleEnum"/>
    


    <!-- http://gtfs.org/WheelchairBoardingEnum -->


    <owl:NamedIndividual rdf:about="http://gtfs.org/WheelchairBoardingEnum"/>
    


    <!-- http://gtfs.org/agency.txt -->


    <owl:NamedIndividual rdf:about="http://gtfs.org/agency.txt">
        <rdf:type rdf:resource="http://gtfs.org/File"/>
        <gtfs:hasField rdf:resource="http://gtfs.org/agency_email"/>
        <gtfs:hasField rdf:resource="http://gtfs.org/agency_fare_url"/>
        <gtfs:hasField rdf:resource="http://gtfs.org/agency_id"/>
        <gtfs:hasField rdf:resource="http://gtfs.org/agency_lang"/>
        <gtfs:hasField rdf:resource="http://gtfs.org/agency_name"/>
        <gtfs:hasField rdf:resource="http://gtfs.org/agency_phone"/>
        <gtfs:hasField rdf:resource="http://gtfs.org/agency_timezone"/>
        <gtfs:hasField rdf:resource="http://gtfs.org/agency_url"/>
        <gtfs:isFileOf rdf:resource="http://gtfs.org/GTFS_Static"/>
        <gtfs:isRequiredIn rdf:resource="http://gtfs.org/GTFS_Static"/>
        <rdfs:comment>Transit agencies with service represented in this dataset.</rdfs:comment>
        <rdfs:label>agency.txt</rdfs:label>
    </owl:NamedIndividual>
    


    <!-- http://gtfs.org/agency_email -->


    <owl:NamedIndividual rdf:about="http://gtfs.org/agency_email">
        <rdf:type rdf:resource="http://gtfs.org/Field"/>
        <gtfs:isFieldOf rdf:resource="http://gtfs.org/agency.txt"/>
        <gtfs:isOptionalIn rdf:resource="http://gtfs.org/agency.txt"/>
        <gtfs:isType rdf:resource="http://gtfs.org/Email"/>
        <gtfs:hasAdditionalInfo>Email address actively monitored by the agency’s customer service department. This email address should be a direct contact point where transit riders can reach a customer service representative at the agency.</gtfs:hasAdditionalInfo>
        <rdfs:comment>Email address actively monitored by the agency’s customer service department. This email address should be a direct contact point where transit riders can reach a customer service representative at the agency.</rdfs:comment>
        <rdfs:label>agency_email</rdfs:label>
    </owl:NamedIndividual>
    


    <!-- http://gtfs.org/agency_fare_url -->


    <owl:NamedIndividual rdf:about="http://gtfs.org/agency_fare_url">
        <rdf:type rdf:resource="http://gtfs.org/Field"/>
        <gtfs:isFieldOf rdf:resource="http://gtfs.org/agency.txt"/>
        <gtfs:isOptionalIn rdf:resource="http://gtfs.org/agency.txt"/>
        <gtfs:isType rdf:resource="http://gtfs.org/URL"/>
        <gtfs:hasAdditionalInfo>Field Type: URL</gtfs:hasAdditionalInfo>
        <rdfs:comment>URL of a web page that allows a rider to purchase tickets or other fare instruments for that agency online.</rdfs:comment>
        <rdfs:label>agency_fare_url</rdfs:label>
    </owl:NamedIndividual>
    


    <!-- http://gtfs.org/agency_id -->


    <owl:NamedIndividual rdf:about="http://gtfs.org/agency_id">
        <rdf:type rdf:resource="http://gtfs.org/Field"/>
        <gtfs:isConditionallyRequiredIn rdf:resource="http://gtfs.org/agency.txt"/>
        <gtfs:isConditionallyRequiredIn rdf:resource="http://gtfs.org/fare_attributes.txt"/>
        <gtfs:isConditionallyRequiredIn rdf:resource="http://gtfs.org/routes.txt"/>
        <gtfs:isFieldOf rdf:resource="http://gtfs.org/agency.txt"/>
        <gtfs:isFieldOf rdf:resource="http://gtfs.org/attributions.txt"/>
        <gtfs:isFieldOf rdf:resource="http://gtfs.org/fare_attributes.txt"/>
        <gtfs:isFieldOf rdf:resource="http://gtfs.org/routes.txt"/>
        <gtfs:isOptionalIn rdf:resource="http://gtfs.org/attributions.txt"/>
        <gtfs:isType rdf:resource="http://gtfs.org/ID"/>
        <gtfs:hasAdditionalInfo>Foreign ID referencing agency.agency_id</gtfs:hasAdditionalInfo>
        <gtfs:hasAdditionalInfo>Unique ID</gtfs:hasAdditionalInfo>
        <gtfs:hasCondition>Required if multiple agencies are defined in agency.txt. Recommended otherwise.</gtfs:hasCondition>
        <gtfs:hasCondition>Required when the dataset contains data for multiple transit agencies. Recommended otherwise.</gtfs:hasCondition>
        <gtfs:isForeignID rdf:resource="http://gtfs.org/attributions.txt"/>
        <gtfs:isForeignID rdf:resource="http://gtfs.org/fare_attributes.txt"/>
        <gtfs:isForeignID rdf:resource="http://gtfs.org/routes.txt"/>
        <gtfs:isUniqueID rdf:resource="http://gtfs.org/agency.txt"/>
        <rdfs:comment>Agency for the specified route.</rdfs:comment>
        <rdfs:comment>Agency to which the attribution applies. If one agency_id, route_id, or trip_id attribution is defined, the other ones must be empty. If none of them is specified, the attribution will apply to the whole dataset.</rdfs:comment>
        <rdfs:comment>Identifies a transit brand which is often synonymous with a transit agency. Note that in some cases, such as when a single agency operates multiple separate services, agencies and brands are distinct. This document uses the term &apos;agency&apos; in place of &apos;brand&apos;. A dataset may contain data from multiple agencies.</rdfs:comment>
        <rdfs:comment>Identifies the relevant agency for a fare.</rdfs:comment>
        <rdfs:label>agency_id</rdfs:label>
    </owl:NamedIndividual>
    


    <!-- http://gtfs.org/agency_lang -->


    <owl:NamedIndividual rdf:about="http://gtfs.org/agency_lang">
        <rdf:type rdf:resource="http://gtfs.org/Field"/>
        <gtfs:isFieldOf rdf:resource="http://gtfs.org/agency.txt"/>
        <gtfs:isOptionalIn rdf:resource="http://gtfs.org/agency.txt"/>
        <gtfs:isType rdf:resource="http://gtfs.org/LanguageCode"/>
        <gtfs:hasAdditionalInfo>Language code</gtfs:hasAdditionalInfo>
        <rdfs:comment>Primary language used by this transit agency. Should be provided to help GTFS consumers choose capitalization rules and other language-specific settings for the dataset.</rdfs:comment>
        <rdfs:label>agency_lang</rdfs:label>
    </owl:NamedIndividual>
    


    <!-- http://gtfs.org/agency_name -->


    <owl:NamedIndividual rdf:about="http://gtfs.org/agency_name">
        <rdf:type rdf:resource="http://gtfs.org/Field"/>
        <gtfs:isFieldOf rdf:resource="http://gtfs.org/agency.txt"/>
        <gtfs:isRequiredIn rdf:resource="http://gtfs.org/agency.txt"/>
        <gtfs:isType rdf:resource="http://gtfs.org/Text"/>
        <gtfs:hasAdditionalInfo>Type: Text</gtfs:hasAdditionalInfo>
        <rdfs:comment>Full name of the transit agency.</rdfs:comment>
        <rdfs:label>agency_name</rdfs:label>
    </owl:NamedIndividual>
    


    <!-- http://gtfs.org/agency_phone -->


    <owl:NamedIndividual rdf:about="http://gtfs.org/agency_phone">
        <rdf:type rdf:resource="http://gtfs.org/Field"/>
        <gtfs:isFieldOf rdf:resource="http://gtfs.org/agency.txt"/>
        <gtfs:isOptionalIn rdf:resource="http://gtfs.org/agency.txt"/>
        <gtfs:isType rdf:resource="http://gtfs.org/PhoneNumber"/>
        <gtfs:hasAdditionalInfo>Phone number should be in a standard format without any descriptive text.</gtfs:hasAdditionalInfo>
        <rdfs:comment>A voice telephone number for the specified agency. This field is a string value that presents the telephone number as typical for the agency&apos;s service area. It may contain punctuation marks to group the digits of the number. Dialable text (for example, TriMet&apos;s &quot;503-238-RIDE&quot;) is permitted, but the field must not contain any other descriptive text.</rdfs:comment>
        <rdfs:label>agency_phone</rdfs:label>
    </owl:NamedIndividual>
    


    <!-- http://gtfs.org/agency_timezone -->


    <owl:NamedIndividual rdf:about="http://gtfs.org/agency_timezone">
        <rdf:type rdf:resource="http://gtfs.org/Field"/>
        <gtfs:isFieldOf rdf:resource="http://gtfs.org/agency.txt"/>
        <gtfs:isRequiredIn rdf:resource="http://gtfs.org/agency.txt"/>
        <gtfs:isType rdf:resource="http://gtfs.org/TimeZone"/>
        <gtfs:hasAdditionalInfo>Timezone where the transit agency is located. If multiple agencies are specified in the dataset, each must have the same `agency_timezone`.</gtfs:hasAdditionalInfo>
        <rdfs:comment>Timezone where the transit agency is located. If multiple agencies are specified in the dataset, each must have the same `agency_timezone`.</rdfs:comment>
        <rdfs:label>agency_timezone</rdfs:label>
    </owl:NamedIndividual>
    


    <!-- http://gtfs.org/agency_url -->


    <owl:NamedIndividual rdf:about="http://gtfs.org/agency_url">
        <rdf:type rdf:resource="http://gtfs.org/Field"/>
        <gtfs:isFieldOf rdf:resource="http://gtfs.org/agency.txt"/>
        <gtfs:isRequiredIn rdf:resource="http://gtfs.org/agency.txt"/>
        <gtfs:isType rdf:resource="http://gtfs.org/URL"/>
        <gtfs:hasAdditionalInfo>URL</gtfs:hasAdditionalInfo>
        <rdfs:comment>URL of the transit agency.</rdfs:comment>
        <rdfs:label>agency_url</rdfs:label>
    </owl:NamedIndividual>
    


    <!-- http://gtfs.org/amount -->


    <owl:NamedIndividual rdf:about="http://gtfs.org/amount">
        <rdf:type rdf:resource="http://gtfs.org/Field"/>
        <gtfs:isFieldOf rdf:resource="http://gtfs.org/fare_products.txt"/>
        <gtfs:isRequiredIn rdf:resource="http://gtfs.org/fare_products.txt"/>
        <gtfs:isType rdf:resource="http://gtfs.org/CurrencyAmount"/>
        <gtfs:hasAdditionalInfo>Currency amount</gtfs:hasAdditionalInfo>
        <rdfs:comment>The cost of the fare product. May be negative to represent transfer discounts. May be zero to represent a fare product that is free.</rdfs:comment>
        <rdfs:label>amount</rdfs:label>
    </owl:NamedIndividual>
    


    <!-- http://gtfs.org/area_id -->


    <owl:NamedIndividual rdf:about="http://gtfs.org/area_id">
        <rdf:type rdf:resource="http://gtfs.org/Field"/>
        <gtfs:isFieldOf rdf:resource="http://gtfs.org/areas.txt"/>
        <gtfs:isFieldOf rdf:resource="http://gtfs.org/stop_areas.txt"/>
        <gtfs:isRequiredIn rdf:resource="http://gtfs.org/areas.txt"/>
        <gtfs:isRequiredIn rdf:resource="http://gtfs.org/stop_areas.txt"/>
        <gtfs:isType rdf:resource="http://gtfs.org/ID"/>
        <gtfs:hasAdditionalInfo>Foreign ID referencing `areas.area_id`</gtfs:hasAdditionalInfo>
        <gtfs:hasAdditionalInfo>Unique ID</gtfs:hasAdditionalInfo>
        <gtfs:isForeignID rdf:resource="http://gtfs.org/stop_areas.txt"/>
        <gtfs:isUniqueID rdf:resource="http://gtfs.org/areas.txt"/>
        <rdfs:comment>Identifies an area to which one or multiple `stop_id`s belong. The same `stop_id` may be defined in many `area_id`s.</rdfs:comment>
        <rdfs:comment>Identifies an area. Must be unique in areas.txt.</rdfs:comment>
        <rdfs:label>area_id</rdfs:label>
    </owl:NamedIndividual>
    


    <!-- http://gtfs.org/area_name -->


    <owl:NamedIndividual rdf:about="http://gtfs.org/area_name">
        <rdf:type rdf:resource="http://gtfs.org/Field"/>
        <gtfs:isFieldOf rdf:resource="http://gtfs.org/areas.txt"/>
        <gtfs:isOptionalIn rdf:resource="http://gtfs.org/areas.txt"/>
        <gtfs:isType rdf:resource="http://gtfs.org/Text"/>
        <gtfs:hasAdditionalInfo>Field Type: Text</gtfs:hasAdditionalInfo>
        <rdfs:comment>The name of the area as displayed to the rider.</rdfs:comment>
        <rdfs:label>area_name</rdfs:label>
    </owl:NamedIndividual>
    


    <!-- http://gtfs.org/areas.txt -->


    <owl:NamedIndividual rdf:about="http://gtfs.org/areas.txt">
        <rdf:type rdf:resource="http://gtfs.org/File"/>
        <gtfs:hasField rdf:resource="http://gtfs.org/area_id"/>
        <gtfs:hasField rdf:resource="http://gtfs.org/area_name"/>
        <gtfs:isFileOf rdf:resource="http://gtfs.org/GTFS_Static"/>
        <gtfs:isOptionalIn rdf:resource="http://gtfs.org/GTFS_Static"/>
        <rdfs:comment>Area grouping of locations.</rdfs:comment>
        <rdfs:label>areas.txt</rdfs:label>
    </owl:NamedIndividual>
    


    <!-- http://gtfs.org/arrival_time -->


    <owl:NamedIndividual rdf:about="http://gtfs.org/arrival_time">
        <rdf:type rdf:resource="http://gtfs.org/Field"/>
        <gtfs:isConditionallyRequiredIn rdf:resource="http://gtfs.org/stop_times.txt"/>
        <gtfs:isFieldOf rdf:resource="http://gtfs.org/stop_times.txt"/>
        <gtfs:isType rdf:resource="http://gtfs.org/Time"/>
        <gtfs:hasAdditionalInfo>The arrival time should be provided in the time zone specified by the agency. If exact arrival and departure times are not available, estimated or interpolated times should be provided.</gtfs:hasAdditionalInfo>
        <gtfs:hasCondition>Required for the first and last stop in a trip (defined by `stop_times.stop_sequence`). Required for `timepoint=1`. Optional otherwise.</gtfs:hasCondition>
        <rdfs:comment>Arrival time at the stop (defined by `stop_times.stop_id`) for a specific trip (defined by `stop_times.trip_id`) in the time zone specified by `agency.agency_timezone`, not `stops.stop_timezone`. If there are not separate times for arrival and departure at a stop, `arrival_time` and `departure_time` should be the same. For times occurring after midnight on the service day, enter the time as a value greater than 24:00:00 in HH:MM:SS. If exact arrival and departure times (`timepoint=1` or empty) are not available, estimated or interpolated arrival and departure times (`timepoint=0`) should be provided.</rdfs:comment>
        <rdfs:label>arrival_time</rdfs:label>
    </owl:NamedIndividual>
    


    <!-- http://gtfs.org/attribution_email -->


    <owl:NamedIndividual rdf:about="http://gtfs.org/attribution_email">
        <rdf:type rdf:resource="http://gtfs.org/Field"/>
        <gtfs:isFieldOf rdf:resource="http://gtfs.org/attributions.txt"/>
        <gtfs:isOptionalIn rdf:resource="http://gtfs.org/attributions.txt"/>
        <gtfs:isType rdf:resource="http://gtfs.org/Email"/>
        <gtfs:hasAdditionalInfo>Email of the organization.</gtfs:hasAdditionalInfo>
        <rdfs:comment>Email of the organization.</rdfs:comment>
        <rdfs:label>attribution_email</rdfs:label>
    </owl:NamedIndividual>
    


    <!-- http://gtfs.org/attribution_id -->


    <owl:NamedIndividual rdf:about="http://gtfs.org/attribution_id">
        <rdf:type rdf:resource="http://gtfs.org/Field"/>
        <gtfs:isFieldOf rdf:resource="http://gtfs.org/attributions.txt"/>
        <gtfs:isOptionalIn rdf:resource="http://gtfs.org/attributions.txt"/>
        <gtfs:isType rdf:resource="http://gtfs.org/ID"/>
        <gtfs:hasAdditionalInfo>Unique ID</gtfs:hasAdditionalInfo>
        <gtfs:isUniqueID rdf:resource="http://gtfs.org/attributions.txt"/>
        <rdfs:comment>Identifies an attribution for the dataset or a subset of it. This is mostly useful for translations.</rdfs:comment>
        <rdfs:label>attribution_id</rdfs:label>
    </owl:NamedIndividual>
    


    <!-- http://gtfs.org/attribution_phone -->


    <owl:NamedIndividual rdf:about="http://gtfs.org/attribution_phone">
        <rdf:type rdf:resource="http://gtfs.org/Field"/>
        <gtfs:isFieldOf rdf:resource="http://gtfs.org/attributions.txt"/>
        <gtfs:isOptionalIn rdf:resource="http://gtfs.org/attributions.txt"/>
        <gtfs:isType rdf:resource="http://gtfs.org/PhoneNumber"/>
        <gtfs:hasAdditionalInfo>Phone number of the organization.</gtfs:hasAdditionalInfo>
        <rdfs:comment>Phone number of the organization.</rdfs:comment>
        <rdfs:label>attribution_phone</rdfs:label>
    </owl:NamedIndividual>
    


    <!-- http://gtfs.org/attribution_url -->


    <owl:NamedIndividual rdf:about="http://gtfs.org/attribution_url">
        <rdf:type rdf:resource="http://gtfs.org/Field"/>
        <gtfs:isFieldOf rdf:resource="http://gtfs.org/attributions.txt"/>
        <gtfs:isOptionalIn rdf:resource="http://gtfs.org/attributions.txt"/>
        <gtfs:isType rdf:resource="http://gtfs.org/URL"/>
        <gtfs:hasAdditionalInfo>URL</gtfs:hasAdditionalInfo>
        <rdfs:comment>URL of the organization.</rdfs:comment>
        <rdfs:label>attribution_url</rdfs:label>
    </owl:NamedIndividual>
    


    <!-- http://gtfs.org/attributions.txt -->


    <owl:NamedIndividual rdf:about="http://gtfs.org/attributions.txt">
        <rdf:type rdf:resource="http://gtfs.org/File"/>
        <gtfs:hasField rdf:resource="http://gtfs.org/agency_id"/>
        <gtfs:hasField rdf:resource="http://gtfs.org/attribution_email"/>
        <gtfs:hasField rdf:resource="http://gtfs.org/attribution_id"/>
        <gtfs:hasField rdf:resource="http://gtfs.org/attribution_phone"/>
        <gtfs:hasField rdf:resource="http://gtfs.org/attribution_url"/>
        <gtfs:hasField rdf:resource="http://gtfs.org/is_authority"/>
        <gtfs:hasField rdf:resource="http://gtfs.org/is_operator"/>
        <gtfs:hasField rdf:resource="http://gtfs.org/is_producer"/>
        <gtfs:hasField rdf:resource="http://gtfs.org/organization_name"/>
        <gtfs:hasField rdf:resource="http://gtfs.org/route_id"/>
        <gtfs:hasField rdf:resource="http://gtfs.org/trip_id"/>
        <gtfs:isFileOf rdf:resource="http://gtfs.org/GTFS_Static"/>
        <gtfs:isOptionalIn rdf:resource="http://gtfs.org/GTFS_Static"/>
        <rdfs:comment>Dataset attributions.</rdfs:comment>
        <rdfs:label>attributions.txt</rdfs:label>
    </owl:NamedIndividual>
    


    <!-- http://gtfs.org/bikes_allowed -->


    <owl:NamedIndividual rdf:about="http://gtfs.org/bikes_allowed">
        <rdf:type rdf:resource="http://gtfs.org/Field"/>
        <gtfs:isFieldOf rdf:resource="http://gtfs.org/trips.txt"/>
        <gtfs:isOptionalIn rdf:resource="http://gtfs.org/trips.txt"/>
        <gtfs:isPresence rdf:resource="http://gtfs.org/Optional"/>
        <gtfs:isType rdf:resource="http://gtfs.org/BikesAllowedEnum"/>
        <gtfs:hasAdditionalInfo>Enum field with options 0, 1, 2</gtfs:hasAdditionalInfo>
        <rdfs:comment>Indicates whether bikes are allowed. Valid options are: 0 or empty - No bike information for the trip. 1 - Vehicle being used on this particular trip can accommodate at least one bicycle. 2 - No bicycles are allowed on this trip.</rdfs:comment>
        <rdfs:label>bikes_allowed</rdfs:label>
    </owl:NamedIndividual>
    


    <!-- http://gtfs.org/bikes_allowed_0 -->


    <owl:NamedIndividual rdf:about="http://gtfs.org/bikes_allowed_0">
        <rdf:type rdf:resource="http://gtfs.org/BikesAllowedEnum"/>
        <gtfs:hasEnumValue>0</gtfs:hasEnumValue>
        <rdfs:comment>No bike information for the trip</rdfs:comment>
        <rdfs:label>bikes_allowed:0</rdfs:label>
    </owl:NamedIndividual>
    


    <!-- http://gtfs.org/bikes_allowed_1 -->


    <owl:NamedIndividual rdf:about="http://gtfs.org/bikes_allowed_1">
        <rdf:type rdf:resource="http://gtfs.org/BikesAllowedEnum"/>
        <gtfs:hasEnumValue>1</gtfs:hasEnumValue>
        <rdfs:comment>Vehicle being used on this particular trip can accommodate at least one bicycle</rdfs:comment>
        <rdfs:label>bikes_allowed:1</rdfs:label>
    </owl:NamedIndividual>
    


    <!-- http://gtfs.org/bikes_allowed_2 -->


    <owl:NamedIndividual rdf:about="http://gtfs.org/bikes_allowed_2">
        <rdf:type rdf:resource="http://gtfs.org/BikesAllowedEnum"/>
        <gtfs:hasEnumValue>2</gtfs:hasEnumValue>
        <rdfs:comment>No bicycles are allowed on this trip</rdfs:comment>
        <rdfs:label>bikes_allowed:2</rdfs:label>
    </owl:NamedIndividual>
    


    <!-- http://gtfs.org/block_id -->


    <owl:NamedIndividual rdf:about="http://gtfs.org/block_id">
        <rdf:type rdf:resource="http://gtfs.org/Field"/>
        <gtfs:isFieldOf rdf:resource="http://gtfs.org/trips.txt"/>
        <gtfs:isOptionalIn rdf:resource="http://gtfs.org/trips.txt"/>
        <gtfs:isType rdf:resource="http://gtfs.org/ID"/>
        <gtfs:hasAdditionalInfo>A block consists of a single trip or many sequential trips made using the same vehicle, defined by shared service days and `block_id`.</gtfs:hasAdditionalInfo>
        <rdfs:comment>Identifies the block to which the trip belongs. A block consists of a single trip or many sequential trips made using the same vehicle, defined by shared service days and `block_id`. A `block_id` may have trips with different service days, making distinct blocks. See the example below. To provide in-seat transfers information, transfers of `transfer_type` `4` should be provided instead.</rdfs:comment>
        <rdfs:label>block_id</rdfs:label>
    </owl:NamedIndividual>
    


    <!-- http://gtfs.org/calendar.txt -->


    <owl:NamedIndividual rdf:about="http://gtfs.org/calendar.txt">
        <rdf:type rdf:resource="http://gtfs.org/File"/>
        <gtfs:hasField rdf:resource="http://gtfs.org/end_date"/>
        <gtfs:hasField rdf:resource="http://gtfs.org/friday"/>
        <gtfs:hasField rdf:resource="http://gtfs.org/monday"/>
        <gtfs:hasField rdf:resource="http://gtfs.org/saturday"/>
        <gtfs:hasField rdf:resource="http://gtfs.org/service_id"/>
        <gtfs:hasField rdf:resource="http://gtfs.org/start_date"/>
        <gtfs:hasField rdf:resource="http://gtfs.org/sunday"/>
        <gtfs:hasField rdf:resource="http://gtfs.org/thursday"/>
        <gtfs:hasField rdf:resource="http://gtfs.org/tuesday"/>
        <gtfs:hasField rdf:resource="http://gtfs.org/wednesday"/>
        <gtfs:isConditionallyRequiredIn rdf:resource="http://gtfs.org/GTFS_Static"/>
        <gtfs:isFileOf rdf:resource="http://gtfs.org/GTFS_Static"/>
        <gtfs:hasCondition>- Required unless all dates of service are defined in calendar_dates.txt. - Optional otherwise.</gtfs:hasCondition>
        <rdfs:comment>Service dates specified using a weekly schedule with start and end dates.</rdfs:comment>
        <rdfs:label>calendar.txt</rdfs:label>
    </owl:NamedIndividual>
    


    <!-- http://gtfs.org/calendar_dates.txt -->


    <owl:NamedIndividual rdf:about="http://gtfs.org/calendar_dates.txt">
        <rdf:type rdf:resource="http://gtfs.org/File"/>
        <gtfs:hasField rdf:resource="http://gtfs.org/date"/>
        <gtfs:hasField rdf:resource="http://gtfs.org/exception_type"/>
        <gtfs:hasField rdf:resource="http://gtfs.org/service_id"/>
        <gtfs:isConditionallyRequiredIn rdf:resource="http://gtfs.org/GTFS_Static"/>
        <gtfs:isFileOf rdf:resource="http://gtfs.org/GTFS_Static"/>
        <gtfs:hasCondition>- Required if calendar.txt is omitted. In which case calendar_dates.txt must contain all dates of service. - Optional otherwise.</gtfs:hasCondition>
        <rdfs:comment>Exceptions for the services defined in the calendar.txt.</rdfs:comment>
        <rdfs:label>calendar_dates.txt</rdfs:label>
    </owl:NamedIndividual>
    


    <!-- http://gtfs.org/contains_id -->


    <owl:NamedIndividual rdf:about="http://gtfs.org/contains_id">
        <rdf:type rdf:resource="http://gtfs.org/Field"/>
        <gtfs:isFieldOf rdf:resource="http://gtfs.org/fare_rules.txt"/>
        <gtfs:isOptionalIn rdf:resource="http://gtfs.org/fare_rules.txt"/>
        <gtfs:isType rdf:resource="http://gtfs.org/ID"/>
        <gtfs:hasAdditionalInfo>Because all `contains_id` zones must be matched for the fare to apply, an itinerary that passes through zones 5 and 6 but not zone 7 would not have fare class &quot;c&quot;. For more detail, see [https://code.google.com/p/googletransitdatafeed/wiki/FareExamples](https://code.google.com/p/googletransitdatafeed/wiki/FareExamples) in the GoogleTransitDataFeed project wiki.</gtfs:hasAdditionalInfo>
        <gtfs:hasExample>fare_id,route_id,...,contains_id
c,GRT,...,5
c,GRT,...,6
c,GRT,...,7</gtfs:hasExample>
        <gtfs:isForeignID rdf:resource="http://gtfs.org/fare_rules.txt"/>
        <rdfs:comment>Identifies the zones that a rider will enter while using a given fare class. Used in some systems to calculate correct fare class.</rdfs:comment>
        <rdfs:label>contains_id</rdfs:label>
    </owl:NamedIndividual>
    


    <!-- http://gtfs.org/continuous_drop_off -->


    <owl:NamedIndividual rdf:about="http://gtfs.org/continuous_drop_off">
        <rdf:type rdf:resource="http://gtfs.org/Field"/>
        <gtfs:isFieldOf rdf:resource="http://gtfs.org/routes.txt"/>
        <gtfs:isFieldOf rdf:resource="http://gtfs.org/stop_times.txt"/>
        <gtfs:isOptionalIn rdf:resource="http://gtfs.org/routes.txt"/>
        <gtfs:isOptionalIn rdf:resource="http://gtfs.org/stop_times.txt"/>
        <gtfs:isPresence rdf:resource="http://gtfs.org/Optional"/>
        <gtfs:isType rdf:resource="http://gtfs.org/ContinuousDropOffEnum"/>
        <gtfs:hasAdditionalInfo>Valid options are: 0 - Continuous stopping drop off, 1 or empty - No continuous stopping drop off, 2 - Must phone agency to arrange continuous stopping drop off, 3 - Must coordinate with driver to arrange continuous stopping drop off. Values for routes.continuous_drop_off may be overridden by defining values in stop_times.continuous_drop_off for specific stop_times along the route.</gtfs:hasAdditionalInfo>
        <rdfs:comment>Indicates that the rider can alight from the transit vehicle at any point along the vehicle’s travel path as described by `shapes.txt`, from this `stop_time` to the next `stop_time` in the trip’s `stop_sequence`. Valid options are: `0` - Continuous stopping drop off. `1` or empty - No continuous stopping drop off. `2` - Must phone agency to arrange continuous stopping drop off. `3` - Must coordinate with driver to arrange continuous stopping drop off. If this field is populated, it overrides any continuous drop-off behavior defined in `routes.txt`. If this field is empty, the `stop_time` inherits any continuous drop-off behavior defined in `routes.txt`.</rdfs:comment>
        <rdfs:comment>Indicates that the rider can alight from the transit vehicle at any point along the vehicle’s travel path as described by shapes.txt, on every trip of the route.</rdfs:comment>
        <rdfs:label>continuous_drop_off</rdfs:label>
    </owl:NamedIndividual>
    


    <!-- http://gtfs.org/continuous_drop_off_0 -->


    <owl:NamedIndividual rdf:about="http://gtfs.org/continuous_drop_off_0">
        <rdf:type rdf:resource="http://gtfs.org/ContinuousDropOffEnum"/>
        <gtfs:hasEnumValue>0</gtfs:hasEnumValue>
        <rdfs:comment>Continuous stopping drop off</rdfs:comment>
        <rdfs:label>continuous_drop_off:0</rdfs:label>
    </owl:NamedIndividual>
    


    <!-- http://gtfs.org/continuous_drop_off_1 -->


    <owl:NamedIndividual rdf:about="http://gtfs.org/continuous_drop_off_1">
        <rdf:type rdf:resource="http://gtfs.org/ContinuousDropOffEnum"/>
        <gtfs:hasEnumValue>1</gtfs:hasEnumValue>
        <rdfs:comment>No continuous stopping drop off</rdfs:comment>
        <rdfs:label>continuous_drop_off:1</rdfs:label>
    </owl:NamedIndividual>
    


    <!-- http://gtfs.org/continuous_drop_off_2 -->


    <owl:NamedIndividual rdf:about="http://gtfs.org/continuous_drop_off_2">
        <rdf:type rdf:resource="http://gtfs.org/ContinuousDropOffEnum"/>
        <gtfs:hasEnumValue>2</gtfs:hasEnumValue>
        <rdfs:comment>Must phone agency to arrange continuous stopping drop off</rdfs:comment>
        <rdfs:label>continuous_drop_off:2</rdfs:label>
    </owl:NamedIndividual>
    


    <!-- http://gtfs.org/continuous_drop_off_3 -->


    <owl:NamedIndividual rdf:about="http://gtfs.org/continuous_drop_off_3">
        <rdf:type rdf:resource="http://gtfs.org/ContinuousDropOffEnum"/>
        <gtfs:hasEnumValue>3</gtfs:hasEnumValue>
        <rdfs:comment>Must coordinate with driver to arrange continuous stopping drop off</rdfs:comment>
        <rdfs:label>continuous_drop_off:3</rdfs:label>
    </owl:NamedIndividual>
    


    <!-- http://gtfs.org/continuous_pickup -->


    <owl:NamedIndividual rdf:about="http://gtfs.org/continuous_pickup">
        <rdf:type rdf:resource="http://gtfs.org/Field"/>
        <gtfs:isFieldOf rdf:resource="http://gtfs.org/routes.txt"/>
        <gtfs:isFieldOf rdf:resource="http://gtfs.org/stop_times.txt"/>
        <gtfs:isOptionalIn rdf:resource="http://gtfs.org/routes.txt"/>
        <gtfs:isOptionalIn rdf:resource="http://gtfs.org/stop_times.txt"/>
        <gtfs:isPresence rdf:resource="http://gtfs.org/Optional"/>
        <gtfs:isType rdf:resource="http://gtfs.org/ContinuousPickupEnum"/>
        <gtfs:hasAdditionalInfo>Valid options are: 0 - Continuous stopping pickup, 1 or empty - No continuous stopping pickup, 2 - Must phone agency to arrange continuous stopping pickup, 3 - Must coordinate with driver to arrange continuous stopping pickup.</gtfs:hasAdditionalInfo>
        <gtfs:hasAdditionalInfo>Valid options are: 0 - Continuous stopping pickup, 1 or empty - No continuous stopping pickup, 2 - Must phone agency to arrange continuous stopping pickup, 3 - Must coordinate with driver to arrange continuous stopping pickup. Values for `routes.continuous_pickup` may be overridden by defining values in `stop_times.continuous_pickup` for specific `stop_time`s along the route.</gtfs:hasAdditionalInfo>
        <rdfs:comment>Indicates that the rider can board the transit vehicle at any point along the vehicle’s travel path as described by `shapes.txt`, from this `stop_time` to the next `stop_time` in the trip’s `stop_sequence`. If this field is populated, it overrides any continuous pickup behavior defined in `routes.txt`. If this field is empty, the `stop_time` inherits any continuous pickup behavior defined in `routes.txt`.</rdfs:comment>
        <rdfs:comment>Indicates that the rider can board the transit vehicle at any point along the vehicle’s travel path as described by `shapes.txt`, on every trip of the route.</rdfs:comment>
        <rdfs:label>continuous_pickup</rdfs:label>
    </owl:NamedIndividual>
    


    <!-- http://gtfs.org/continuous_pickup_0 -->


    <owl:NamedIndividual rdf:about="http://gtfs.org/continuous_pickup_0">
        <rdf:type rdf:resource="http://gtfs.org/ContinuousPickupEnum"/>
        <gtfs:hasEnumValue>0</gtfs:hasEnumValue>
        <rdfs:comment>Continuous stopping pickup</rdfs:comment>
        <rdfs:label>continuous_pickup:0</rdfs:label>
    </owl:NamedIndividual>
    


    <!-- http://gtfs.org/continuous_pickup_1 -->


    <owl:NamedIndividual rdf:about="http://gtfs.org/continuous_pickup_1">
        <rdf:type rdf:resource="http://gtfs.org/ContinuousPickupEnum"/>
        <gtfs:hasEnumValue>1</gtfs:hasEnumValue>
        <rdfs:comment>No continuous stopping pickup</rdfs:comment>
        <rdfs:label>continuous_pickup:1</rdfs:label>
    </owl:NamedIndividual>
    


    <!-- http://gtfs.org/continuous_pickup_2 -->


    <owl:NamedIndividual rdf:about="http://gtfs.org/continuous_pickup_2">
        <rdf:type rdf:resource="http://gtfs.org/ContinuousPickupEnum"/>
        <gtfs:hasEnumValue>2</gtfs:hasEnumValue>
        <rdfs:comment>Must phone agency to arrange continuous stopping pickup</rdfs:comment>
        <rdfs:label>continuous_pickup:2</rdfs:label>
    </owl:NamedIndividual>
    


    <!-- http://gtfs.org/continuous_pickup_3 -->


    <owl:NamedIndividual rdf:about="http://gtfs.org/continuous_pickup_3">
        <rdf:type rdf:resource="http://gtfs.org/ContinuousPickupEnum"/>
        <gtfs:hasEnumValue>3</gtfs:hasEnumValue>
        <rdfs:comment>Must coordinate with driver to arrange continuous stopping pickup</rdfs:comment>
        <rdfs:label>continuous_pickup:3</rdfs:label>
    </owl:NamedIndividual>
    


    <!-- http://gtfs.org/currency -->


    <owl:NamedIndividual rdf:about="http://gtfs.org/currency">
        <rdf:type rdf:resource="http://gtfs.org/Field"/>
        <gtfs:isFieldOf rdf:resource="http://gtfs.org/fare_products.txt"/>
        <gtfs:isRequiredIn rdf:resource="http://gtfs.org/fare_products.txt"/>
        <gtfs:isType rdf:resource="http://gtfs.org/CurrencyCode"/>
        <gtfs:hasAdditionalInfo>Currency code</gtfs:hasAdditionalInfo>
        <rdfs:comment>The currency of the cost of the fare product.</rdfs:comment>
        <rdfs:label>currency</rdfs:label>
    </owl:NamedIndividual>
    


    <!-- http://gtfs.org/currency_type -->


    <owl:NamedIndividual rdf:about="http://gtfs.org/currency_type">
        <rdf:type rdf:resource="http://gtfs.org/Field"/>
        <gtfs:isFieldOf rdf:resource="http://gtfs.org/fare_attributes.txt"/>
        <gtfs:isRequiredIn rdf:resource="http://gtfs.org/fare_attributes.txt"/>
        <gtfs:isType rdf:resource="http://gtfs.org/CurrencyCode"/>
        <gtfs:hasAdditionalInfo>Currency code</gtfs:hasAdditionalInfo>
        <rdfs:comment>Currency used to pay the fare.</rdfs:comment>
        <rdfs:label>currency_type</rdfs:label>
    </owl:NamedIndividual>
    


    <!-- http://gtfs.org/date -->


    <owl:NamedIndividual rdf:about="http://gtfs.org/date">
        <rdf:type rdf:resource="http://gtfs.org/Field"/>
        <gtfs:isFieldOf rdf:resource="http://gtfs.org/calendar_dates.txt"/>
        <gtfs:isRequiredIn rdf:resource="http://gtfs.org/calendar_dates.txt"/>
        <gtfs:isType rdf:resource="http://gtfs.org/Date"/>
        <gtfs:hasAdditionalInfo>Field Type: Date</gtfs:hasAdditionalInfo>
        <rdfs:comment>Date when service exception occurs.</rdfs:comment>
        <rdfs:label>date</rdfs:label>
    </owl:NamedIndividual>
    


    <!-- http://gtfs.org/default_lang -->


    <owl:NamedIndividual rdf:about="http://gtfs.org/default_lang">
        <rdf:type rdf:resource="http://gtfs.org/Field"/>
        <gtfs:isFieldOf rdf:resource="http://gtfs.org/feed_info.txt"/>
        <gtfs:isOptionalIn rdf:resource="http://gtfs.org/feed_info.txt"/>
        <gtfs:isType rdf:resource="http://gtfs.org/LanguageCode"/>
        <gtfs:hasAdditionalInfo>Language code</gtfs:hasAdditionalInfo>
        <rdfs:comment>Defines the language that should be used when the data consumer doesn’t know the language of the rider. It will often be `en` (English).</rdfs:comment>
        <rdfs:label>default_lang</rdfs:label>
    </owl:NamedIndividual>
    


    <!-- http://gtfs.org/departure_time -->


    <owl:NamedIndividual rdf:about="http://gtfs.org/departure_time">
        <rdf:type rdf:resource="http://gtfs.org/Field"/>
        <gtfs:isConditionallyRequiredIn rdf:resource="http://gtfs.org/stop_times.txt"/>
        <gtfs:isFieldOf rdf:resource="http://gtfs.org/stop_times.txt"/>
        <gtfs:isType rdf:resource="http://gtfs.org/Time"/>
        <gtfs:hasAdditionalInfo>Conditionally Required: Required for `timepoint=1`. Optional otherwise</gtfs:hasAdditionalInfo>
        <gtfs:hasCondition>Required for `timepoint=1`. Optional otherwise</gtfs:hasCondition>
        <rdfs:comment>Departure time from the stop (defined by `stop_times.stop_id`) for a specific trip (defined by `stop_times.trip_id`) in the time zone specified by `agency.agency_timezone`, not `stops.stop_timezone`.

If there are not separate times for arrival and departure at a stop, `arrival_time` and `departure_time` should be the same. 

For times occurring after midnight on the service day, enter the time as a value greater than 24:00:00 in HH:MM:SS.

 If exact arrival and departure times (`timepoint=1` or empty) are not available, estimated or interpolated arrival and departure times (`timepoint=0`) should be provided.</rdfs:comment>
        <rdfs:label>departure_time</rdfs:label>
    </owl:NamedIndividual>
    


    <!-- http://gtfs.org/destination_id -->


    <owl:NamedIndividual rdf:about="http://gtfs.org/destination_id">
        <rdf:type rdf:resource="http://gtfs.org/Field"/>
        <gtfs:isFieldOf rdf:resource="http://gtfs.org/fare_rules.txt"/>
        <gtfs:isOptionalIn rdf:resource="http://gtfs.org/fare_rules.txt"/>
        <gtfs:isType rdf:resource="http://gtfs.org/ID"/>
        <gtfs:hasAdditionalInfo>Foreign ID referencing stops.zone_id</gtfs:hasAdditionalInfo>
        <gtfs:hasExample>The origin_id and destination_id fields could be used together to specify that fare class &apos;b&apos; is valid for travel between zones 3 and 4, and for travel between zones 3 and 5, the fare_rules.txt file would contain these records for the fare class: fare_id,...,origin_id,destination_id b,...,3,4 b,...,3,5</gtfs:hasExample>
        <gtfs:isForeignID rdf:resource="http://gtfs.org/fare_rules.txt"/>
        <rdfs:comment>Identifies a destination zone. If a fare class has multiple destination zones, create a record in fare_rules.txt for each destination_id.</rdfs:comment>
        <rdfs:label>destination_id</rdfs:label>
    </owl:NamedIndividual>
    


    <!-- http://gtfs.org/direction_id -->


    <owl:NamedIndividual rdf:about="http://gtfs.org/direction_id">
        <rdf:type rdf:resource="http://gtfs.org/Field"/>
        <gtfs:isFieldOf rdf:resource="http://gtfs.org/trips.txt"/>
        <gtfs:isOptionalIn rdf:resource="http://gtfs.org/trips.txt"/>
        <gtfs:isPresence rdf:resource="http://gtfs.org/Optional"/>
        <gtfs:isType rdf:resource="http://gtfs.org/DirectionIdEnum"/>
        <gtfs:hasAdditionalInfo>Valid options are: 0 - Travel in one direction (e.g. outbound travel). 1 - Travel in the opposite direction (e.g. inbound travel).</gtfs:hasAdditionalInfo>
        <rdfs:comment>Indicates the direction of travel for a trip. This field should not be used in routing; it provides a way to separate trips by direction when publishing time tables.</rdfs:comment>
        <rdfs:label>direction_id</rdfs:label>
    </owl:NamedIndividual>
    


    <!-- http://gtfs.org/direction_id_0 -->


    <owl:NamedIndividual rdf:about="http://gtfs.org/direction_id_0">
        <rdf:type rdf:resource="http://gtfs.org/DirectionIdEnum"/>
        <gtfs:hasEnumValue>0</gtfs:hasEnumValue>
        <rdfs:comment>Travel in one direction (e.g. outbound travel)</rdfs:comment>
        <rdfs:label>direction_id:0</rdfs:label>
    </owl:NamedIndividual>
    


    <!-- http://gtfs.org/direction_id_1 -->


    <owl:NamedIndividual rdf:about="http://gtfs.org/direction_id_1">
        <rdf:type rdf:resource="http://gtfs.org/DirectionIdEnum"/>
        <gtfs:hasEnumValue>1</gtfs:hasEnumValue>
        <rdfs:comment>Travel in the opposite direction (e.g. inbound travel)</rdfs:comment>
        <rdfs:label>direction_id:1</rdfs:label>
    </owl:NamedIndividual>
    


    <!-- http://gtfs.org/drop_off_type -->


    <owl:NamedIndividual rdf:about="http://gtfs.org/drop_off_type">
        <rdf:type rdf:resource="http://gtfs.org/Field"/>
        <gtfs:isFieldOf rdf:resource="http://gtfs.org/stop_times.txt"/>
        <gtfs:isOptionalIn rdf:resource="http://gtfs.org/stop_times.txt"/>
        <gtfs:isPresence rdf:resource="http://gtfs.org/Optional"/>
        <gtfs:isType rdf:resource="http://gtfs.org/DropOffTypeEnum"/>
        <gtfs:hasAdditionalInfo>Enum field with options 0, 1, 2, 3</gtfs:hasAdditionalInfo>
        <rdfs:comment>Indicates drop off method. Valid options are: 0 or empty - Regularly scheduled drop off. 1 - No drop off available. 2 - Must phone agency to arrange drop off. 3 - Must coordinate with driver to arrange drop off.</rdfs:comment>
        <rdfs:label>drop_off_type</rdfs:label>
    </owl:NamedIndividual>
    


    <!-- http://gtfs.org/drop_off_type_0 -->


    <owl:NamedIndividual rdf:about="http://gtfs.org/drop_off_type_0">
        <rdf:type rdf:resource="http://gtfs.org/DropOffTypeEnum"/>
        <gtfs:hasEnumValue>0</gtfs:hasEnumValue>
        <rdfs:comment>Regularly scheduled drop off</rdfs:comment>
        <rdfs:label>drop_off_type:0</rdfs:label>
    </owl:NamedIndividual>
    


    <!-- http://gtfs.org/drop_off_type_1 -->


    <owl:NamedIndividual rdf:about="http://gtfs.org/drop_off_type_1">
        <rdf:type rdf:resource="http://gtfs.org/DropOffTypeEnum"/>
        <gtfs:hasEnumValue>1</gtfs:hasEnumValue>
        <rdfs:comment>No drop off available</rdfs:comment>
        <rdfs:label>drop_off_type:1</rdfs:label>
    </owl:NamedIndividual>
    


    <!-- http://gtfs.org/drop_off_type_2 -->


    <owl:NamedIndividual rdf:about="http://gtfs.org/drop_off_type_2">
        <rdf:type rdf:resource="http://gtfs.org/DropOffTypeEnum"/>
        <gtfs:hasEnumValue>2</gtfs:hasEnumValue>
        <rdfs:comment>Must phone agency to arrange drop off</rdfs:comment>
        <rdfs:label>drop_off_type:2</rdfs:label>
    </owl:NamedIndividual>
    


    <!-- http://gtfs.org/drop_off_type_3 -->


    <owl:NamedIndividual rdf:about="http://gtfs.org/drop_off_type_3">
        <rdf:type rdf:resource="http://gtfs.org/DropOffTypeEnum"/>
        <gtfs:hasEnumValue>3</gtfs:hasEnumValue>
        <rdfs:comment>Must coordinate with driver to arrange drop off</rdfs:comment>
        <rdfs:label>drop_off_type:3</rdfs:label>
    </owl:NamedIndividual>
    


    <!-- http://gtfs.org/duration_limit -->


    <owl:NamedIndividual rdf:about="http://gtfs.org/duration_limit">
        <rdf:type rdf:resource="http://gtfs.org/Field"/>
        <gtfs:isFieldOf rdf:resource="http://gtfs.org/fare_transfer_rules.txt"/>
        <gtfs:isOptionalIn rdf:resource="http://gtfs.org/fare_transfer_rules.txt"/>
        <gtfs:isType rdf:resource="http://gtfs.org/Integer"/>
        <gtfs:hasAdditionalInfo>Positive integer</gtfs:hasAdditionalInfo>
        <rdfs:comment>Defines the duration limit of the transfer.

Must be expressed in integer increments of seconds.

If there is no duration limit, `fare_transfer_rules.duration_limit` must be empty.</rdfs:comment>
        <rdfs:label>duration_limit</rdfs:label>
    </owl:NamedIndividual>
    


    <!-- http://gtfs.org/duration_limit_type -->


    <owl:NamedIndividual rdf:about="http://gtfs.org/duration_limit_type">
        <rdf:type rdf:resource="http://gtfs.org/Field"/>
        <gtfs:isConditionallyRequiredIn rdf:resource="http://gtfs.org/fare_transfer_rules.txt"/>
        <gtfs:isFieldOf rdf:resource="http://gtfs.org/fare_transfer_rules.txt"/>
        <gtfs:isPresence rdf:resource="http://gtfs.org/ConditionallyRequired"/>
        <gtfs:isType rdf:resource="http://gtfs.org/DurationLimitTypeEnum"/>
        <gtfs:hasAdditionalInfo>Defines the relative start and end of `fare_transfer_rules.duration_limit`.</gtfs:hasAdditionalInfo>
        <gtfs:hasCondition>Required if `fare_transfer_rules.duration_limit` is defined. Forbidden if `fare_transfer_rules.duration_limit` is empty.</gtfs:hasCondition>
        <rdfs:comment>Defines the relative start and end of `fare_transfer_rules.duration_limit`. Valid options are: `0` - Between the departure fare validation of the current leg and the arrival fare validation of the next leg. `1` - Between the departure fare validation of the current leg and the departure fare validation of the next leg. `2` - Between the arrival fare validation of the current leg and the departure fare validation of the next leg. `3` - Between the arrival fare validation of the current leg and the arrival fare validation of the next leg.</rdfs:comment>
        <rdfs:label>duration_limit_type</rdfs:label>
    </owl:NamedIndividual>
    


    <!-- http://gtfs.org/duration_limit_type_0 -->


    <owl:NamedIndividual rdf:about="http://gtfs.org/duration_limit_type_0">
        <rdf:type rdf:resource="http://gtfs.org/DurationLimitTypeEnum"/>
        <gtfs:hasEnumValue>0</gtfs:hasEnumValue>
        <rdfs:comment>Between the departure fare validation of the current leg and the arrival fare validation of the next leg</rdfs:comment>
        <rdfs:label>duration_limit_type:0</rdfs:label>
    </owl:NamedIndividual>
    


    <!-- http://gtfs.org/duration_limit_type_1 -->


    <owl:NamedIndividual rdf:about="http://gtfs.org/duration_limit_type_1">
        <rdf:type rdf:resource="http://gtfs.org/DurationLimitTypeEnum"/>
        <gtfs:hasEnumValue>1</gtfs:hasEnumValue>
        <rdfs:comment>Between the departure fare validation of the current leg and the departure fare validation of the next leg</rdfs:comment>
        <rdfs:label>duration_limit_type:1</rdfs:label>
    </owl:NamedIndividual>
    


    <!-- http://gtfs.org/duration_limit_type_2 -->


    <owl:NamedIndividual rdf:about="http://gtfs.org/duration_limit_type_2">
        <rdf:type rdf:resource="http://gtfs.org/DurationLimitTypeEnum"/>
        <gtfs:hasEnumValue>2</gtfs:hasEnumValue>
        <rdfs:comment>Between the arrival fare validation of the current leg and the departure fare validation of the next leg</rdfs:comment>
        <rdfs:label>duration_limit_type:2</rdfs:label>
    </owl:NamedIndividual>
    


    <!-- http://gtfs.org/duration_limit_type_3 -->


    <owl:NamedIndividual rdf:about="http://gtfs.org/duration_limit_type_3">
        <rdf:type rdf:resource="http://gtfs.org/DurationLimitTypeEnum"/>
        <gtfs:hasEnumValue>3</gtfs:hasEnumValue>
        <rdfs:comment>Between the arrival fare validation of the current leg and the arrival fare validation of the next leg</rdfs:comment>
        <rdfs:label>duration_limit_type:3</rdfs:label>
    </owl:NamedIndividual>
    


    <!-- http://gtfs.org/end_date -->


    <owl:NamedIndividual rdf:about="http://gtfs.org/end_date">
        <rdf:type rdf:resource="http://gtfs.org/Field"/>
        <gtfs:isFieldOf rdf:resource="http://gtfs.org/calendar.txt"/>
        <gtfs:isRequiredIn rdf:resource="http://gtfs.org/calendar.txt"/>
        <gtfs:isType rdf:resource="http://gtfs.org/Date"/>
        <gtfs:hasAdditionalInfo>The end_date field specifies the end service day for the service interval.</gtfs:hasAdditionalInfo>
        <rdfs:comment>End service day for the service interval. This service day is included in the interval.</rdfs:comment>
        <rdfs:label>end_date</rdfs:label>
    </owl:NamedIndividual>
    


    <!-- http://gtfs.org/end_time -->


    <owl:NamedIndividual rdf:about="http://gtfs.org/end_time">
        <rdf:type rdf:resource="http://gtfs.org/Field"/>
        <gtfs:isConditionallyRequiredIn rdf:resource="http://gtfs.org/timeframes.txt"/>
        <gtfs:isFieldOf rdf:resource="http://gtfs.org/frequencies.txt"/>
        <gtfs:isFieldOf rdf:resource="http://gtfs.org/timeframes.txt"/>
        <gtfs:isRequiredIn rdf:resource="http://gtfs.org/frequencies.txt"/>
        <gtfs:isType rdf:resource="http://gtfs.org/Time"/>
        <gtfs:hasAdditionalInfo>Time at which service changes to a different headway (or ceases) at the first stop in the trip.</gtfs:hasAdditionalInfo>
        <gtfs:hasAdditionalInfo>Values greater than 24:00:00 are forbidden. An empty value in end_time is considered 24:00:00.</gtfs:hasAdditionalInfo>
        <gtfs:hasCondition>Required if timeframes.start_time is defined. Forbidden otherwise</gtfs:hasCondition>
        <rdfs:comment>Defines the end of a timeframe. The interval does not include the end time. Values greater than 24:00:00 are forbidden. An empty value in end_time is considered 24:00:00.</rdfs:comment>
        <rdfs:comment>Time at which service changes to a different headway (or ceases) at the first stop in the trip.</rdfs:comment>
        <rdfs:label>end_time</rdfs:label>
    </owl:NamedIndividual>
    


    <!-- http://gtfs.org/exact_times -->


    <owl:NamedIndividual rdf:about="http://gtfs.org/exact_times">
        <rdf:type rdf:resource="http://gtfs.org/Field"/>
        <gtfs:isFieldOf rdf:resource="http://gtfs.org/frequencies.txt"/>
        <gtfs:isOptionalIn rdf:resource="http://gtfs.org/frequencies.txt"/>
        <gtfs:isPresence rdf:resource="http://gtfs.org/Optional"/>
        <gtfs:isType rdf:resource="http://gtfs.org/ExactTimesEnum"/>
        <gtfs:hasAdditionalInfo>Enum field with options 0 or 1</gtfs:hasAdditionalInfo>
        <rdfs:comment>Indicates the type of service for a trip. See the file description for more information. Valid options are: 0 or empty - Frequency-based trips. 1 - Schedule-based trips with the exact same headway throughout the day. In this case the end_time value must be greater than the last desired trip start_time but less than the last desired trip start_time + headway_secs.</rdfs:comment>
        <rdfs:label>exact_times</rdfs:label>
    </owl:NamedIndividual>
    


    <!-- http://gtfs.org/exact_times_0 -->


    <owl:NamedIndividual rdf:about="http://gtfs.org/exact_times_0">
        <rdf:type rdf:resource="http://gtfs.org/ExactTimesEnum"/>
        <gtfs:hasEnumValue>0</gtfs:hasEnumValue>
        <rdfs:comment>Frequency-based trips</rdfs:comment>
        <rdfs:label>exact_times:0</rdfs:label>
    </owl:NamedIndividual>
    


    <!-- http://gtfs.org/exact_times_1 -->


    <owl:NamedIndividual rdf:about="http://gtfs.org/exact_times_1">
        <rdf:type rdf:resource="http://gtfs.org/ExactTimesEnum"/>
        <gtfs:hasEnumValue>1</gtfs:hasEnumValue>
        <rdfs:comment>Schedule-based trips with exact same headway throughout the day</rdfs:comment>
        <rdfs:label>exact_times:1</rdfs:label>
    </owl:NamedIndividual>
    


    <!-- http://gtfs.org/exception_type -->


    <owl:NamedIndividual rdf:about="http://gtfs.org/exception_type">
        <rdf:type rdf:resource="http://gtfs.org/Field"/>
        <gtfs:isFieldOf rdf:resource="http://gtfs.org/calendar_dates.txt"/>
        <gtfs:isPresence rdf:resource="http://gtfs.org/Required"/>
        <gtfs:isRequiredIn rdf:resource="http://gtfs.org/calendar_dates.txt"/>
        <gtfs:isType rdf:resource="http://gtfs.org/ExceptionTypeEnum"/>
        <gtfs:hasAdditionalInfo>Suppose a route has one set of trips available on holidays and another set of trips available on all other days. One service_id could correspond to the regular service schedule and another service_id could correspond to the holiday schedule. For a particular holiday, the calendar_dates.txt file could be used to add the holiday to the holiday service_id and to remove the holiday from the regular service_id schedule.</gtfs:hasAdditionalInfo>
        <rdfs:comment>Indicates whether service is available on the date specified in the date field. Valid options are: 1 - Service has been added for the specified date. 2 - Service has been removed for the specified date.</rdfs:comment>
        <rdfs:label>exception_type</rdfs:label>
    </owl:NamedIndividual>
    


    <!-- http://gtfs.org/exception_type_1 -->


    <owl:NamedIndividual rdf:about="http://gtfs.org/exception_type_1">
        <rdf:type rdf:resource="http://gtfs.org/ExceptionTypeEnum"/>
        <gtfs:hasEnumValue>1</gtfs:hasEnumValue>
        <rdfs:comment>Service has been added for the specified date</rdfs:comment>
        <rdfs:label>exception_type:1</rdfs:label>
    </owl:NamedIndividual>
    


    <!-- http://gtfs.org/exception_type_2 -->


    <owl:NamedIndividual rdf:about="http://gtfs.org/exception_type_2">
        <rdf:type rdf:resource="http://gtfs.org/ExceptionTypeEnum"/>
        <gtfs:hasEnumValue>2</gtfs:hasEnumValue>
        <rdfs:comment>Service has been removed for the specified date</rdfs:comment>
        <rdfs:label>exception_type:2</rdfs:label>
    </owl:NamedIndividual>
    


    <!-- http://gtfs.org/fare_attributes.txt -->


    <owl:NamedIndividual rdf:about="http://gtfs.org/fare_attributes.txt">
        <rdf:type rdf:resource="http://gtfs.org/File"/>
        <gtfs:hasField rdf:resource="http://gtfs.org/agency_id"/>
        <gtfs:hasField rdf:resource="http://gtfs.org/currency_type"/>
        <gtfs:hasField rdf:resource="http://gtfs.org/fare_id"/>
        <gtfs:hasField rdf:resource="http://gtfs.org/payment_method"/>
        <gtfs:hasField rdf:resource="http://gtfs.org/price"/>
        <gtfs:hasField rdf:resource="http://gtfs.org/transfer_duration"/>
        <gtfs:hasField rdf:resource="http://gtfs.org/transfers"/>
        <gtfs:isFileOf rdf:resource="http://gtfs.org/GTFS_Static"/>
        <gtfs:isOptionalIn rdf:resource="http://gtfs.org/GTFS_Static"/>
        <rdfs:comment>Fare information for a transit agency&apos;s routes.</rdfs:comment>
        <rdfs:label>fare_attributes.txt</rdfs:label>
    </owl:NamedIndividual>
    


    <!-- http://gtfs.org/fare_id -->


    <owl:NamedIndividual rdf:about="http://gtfs.org/fare_id">
        <rdf:type rdf:resource="http://gtfs.org/Field"/>
        <gtfs:isFieldOf rdf:resource="http://gtfs.org/fare_attributes.txt"/>
        <gtfs:isFieldOf rdf:resource="http://gtfs.org/fare_rules.txt"/>
        <gtfs:isRequiredIn rdf:resource="http://gtfs.org/fare_attributes.txt"/>
        <gtfs:isRequiredIn rdf:resource="http://gtfs.org/fare_rules.txt"/>
        <gtfs:isType rdf:resource="http://gtfs.org/ID"/>
        <gtfs:hasAdditionalInfo>Foreign ID referencing fare_attributes.fare_id</gtfs:hasAdditionalInfo>
        <gtfs:hasAdditionalInfo>Unique ID</gtfs:hasAdditionalInfo>
        <gtfs:isForeignID rdf:resource="http://gtfs.org/fare_rules.txt"/>
        <gtfs:isUniqueID rdf:resource="http://gtfs.org/fare_attributes.txt"/>
        <rdfs:comment>Identifies a fare class.</rdfs:comment>
        <rdfs:label>fare_id</rdfs:label>
    </owl:NamedIndividual>
    


    <!-- http://gtfs.org/fare_leg_rules.txt -->


    <owl:NamedIndividual rdf:about="http://gtfs.org/fare_leg_rules.txt">
        <rdf:type rdf:resource="http://gtfs.org/File"/>
        <gtfs:hasField rdf:resource="http://gtfs.org/fare_product_id"/>
        <gtfs:hasField rdf:resource="http://gtfs.org/from_area_id"/>
        <gtfs:hasField rdf:resource="http://gtfs.org/from_timeframe_group_id"/>
        <gtfs:hasField rdf:resource="http://gtfs.org/leg_group_id"/>
        <gtfs:hasField rdf:resource="http://gtfs.org/network_id"/>
        <gtfs:hasField rdf:resource="http://gtfs.org/to_area_id"/>
        <gtfs:hasField rdf:resource="http://gtfs.org/to_timeframe_group_id"/>
        <gtfs:isFileOf rdf:resource="http://gtfs.org/GTFS_Static"/>
        <gtfs:isOptionalIn rdf:resource="http://gtfs.org/GTFS_Static"/>
        <gtfs:hasAdditionalInfo>File provides a more detailed method for modeling fare structures.</gtfs:hasAdditionalInfo>
        <rdfs:comment>Fare rules for individual legs of travel.</rdfs:comment>
        <rdfs:label>fare_leg_rules.txt</rdfs:label>
    </owl:NamedIndividual>
    


    <!-- http://gtfs.org/fare_media.txt -->


    <owl:NamedIndividual rdf:about="http://gtfs.org/fare_media.txt">
        <rdf:type rdf:resource="http://gtfs.org/File"/>
        <gtfs:hasField rdf:resource="http://gtfs.org/fare_media_id"/>
        <gtfs:hasField rdf:resource="http://gtfs.org/fare_media_name"/>
        <gtfs:hasField rdf:resource="http://gtfs.org/fare_media_type"/>
        <gtfs:isFileOf rdf:resource="http://gtfs.org/GTFS_Static"/>
        <gtfs:isOptionalIn rdf:resource="http://gtfs.org/GTFS_Static"/>
        <gtfs:hasAdditionalInfo>File describes concepts not represented in fare_attributes.txt and fare_rules.txt.</gtfs:hasAdditionalInfo>
        <rdfs:comment>To describe the fare media that can be employed to use fare products.</rdfs:comment>
        <rdfs:label>fare_media.txt</rdfs:label>
    </owl:NamedIndividual>
    


    <!-- http://gtfs.org/fare_media_id -->


    <owl:NamedIndividual rdf:about="http://gtfs.org/fare_media_id">
        <rdf:type rdf:resource="http://gtfs.org/Field"/>
        <gtfs:isFieldOf rdf:resource="http://gtfs.org/fare_media.txt"/>
        <gtfs:isFieldOf rdf:resource="http://gtfs.org/fare_products.txt"/>
        <gtfs:isOptionalIn rdf:resource="http://gtfs.org/fare_products.txt"/>
        <gtfs:isRequiredIn rdf:resource="http://gtfs.org/fare_media.txt"/>
        <gtfs:isType rdf:resource="http://gtfs.org/ID"/>
        <gtfs:hasAdditionalInfo>Foreign ID referencing `fare_media.fare_media_id`</gtfs:hasAdditionalInfo>
        <gtfs:hasAdditionalInfo>Unique ID</gtfs:hasAdditionalInfo>
        <gtfs:isForeignID rdf:resource="http://gtfs.org/fare_products.txt"/>
        <gtfs:isUniqueID rdf:resource="http://gtfs.org/fare_media.txt"/>
        <rdfs:comment>Identifies a fare media that can be employed to use the fare product during the trip. When `fare_media_id` is empty, it is considered that the fare media is unknown.</rdfs:comment>
        <rdfs:comment>Identifies a fare media.</rdfs:comment>
        <rdfs:label>fare_media_id</rdfs:label>
    </owl:NamedIndividual>
    


    <!-- http://gtfs.org/fare_media_name -->


    <owl:NamedIndividual rdf:about="http://gtfs.org/fare_media_name">
        <rdf:type rdf:resource="http://gtfs.org/Field"/>
        <gtfs:isFieldOf rdf:resource="http://gtfs.org/fare_media.txt"/>
        <gtfs:isOptionalIn rdf:resource="http://gtfs.org/fare_media.txt"/>
        <gtfs:isType rdf:resource="http://gtfs.org/Text"/>
        <gtfs:hasAdditionalInfo>None</gtfs:hasAdditionalInfo>
        <rdfs:comment>Name of the fare media.

For fare media which are transit cards (`fare_media_type =2`) or mobile apps (`fare_media_type =4`), the `fare_media_name` should be included and should match the rider-facing name used by the organizations delivering them.</rdfs:comment>
        <rdfs:label>fare_media_name</rdfs:label>
    </owl:NamedIndividual>
    


    <!-- http://gtfs.org/fare_media_type -->


    <owl:NamedIndividual rdf:about="http://gtfs.org/fare_media_type">
        <rdf:type rdf:resource="http://gtfs.org/Field"/>
        <gtfs:isFieldOf rdf:resource="http://gtfs.org/fare_media.txt"/>
        <gtfs:isPresence rdf:resource="http://gtfs.org/Required"/>
        <gtfs:isRequiredIn rdf:resource="http://gtfs.org/fare_media.txt"/>
        <gtfs:isType rdf:resource="http://gtfs.org/FareMediaTypeEnum"/>
        <gtfs:hasAdditionalInfo>Enum field with options: 0 - None, 1 - Physical paper ticket, 2 - Physical transit card, 3 - cEMV, 4 - Mobile app</gtfs:hasAdditionalInfo>
        <rdfs:comment>The type of fare media. Valid options are: 0 - None. Used when there is no fare media involved in purchasing or validating a fare product, such as paying cash to a driver or conductor with no physical ticket provided. 1 - Physical paper ticket that allows a passenger to take either a certain number of pre-purchased trips or unlimited trips within a fixed period of time. 2 - Physical transit card that has stored tickets, passes or monetary value. 3 - cEMV (contactless Europay, Mastercard and Visa) as an open-loop token container for account-based ticketing. 4 - Mobile app that have stored virtual transit cards, tickets, passes, or monetary value.</rdfs:comment>
        <rdfs:label>fare_media_type</rdfs:label>
    </owl:NamedIndividual>
    


    <!-- http://gtfs.org/fare_media_type_0 -->


    <owl:NamedIndividual rdf:about="http://gtfs.org/fare_media_type_0">
        <rdf:type rdf:resource="http://gtfs.org/FareMediaTypeEnum"/>
        <gtfs:hasEnumValue>0</gtfs:hasEnumValue>
        <rdfs:comment>None</rdfs:comment>
        <rdfs:label>fare_media_type:0</rdfs:label>
    </owl:NamedIndividual>
    


    <!-- http://gtfs.org/fare_media_type_1 -->


    <owl:NamedIndividual rdf:about="http://gtfs.org/fare_media_type_1">
        <rdf:type rdf:resource="http://gtfs.org/FareMediaTypeEnum"/>
        <gtfs:hasEnumValue>1</gtfs:hasEnumValue>
        <rdfs:comment>Physical paper ticket</rdfs:comment>
        <rdfs:label>fare_media_type:1</rdfs:label>
    </owl:NamedIndividual>
    


    <!-- http://gtfs.org/fare_media_type_2 -->


    <owl:NamedIndividual rdf:about="http://gtfs.org/fare_media_type_2">
        <rdf:type rdf:resource="http://gtfs.org/FareMediaTypeEnum"/>
        <gtfs:hasEnumValue>2</gtfs:hasEnumValue>
        <rdfs:comment>Physical transit card</rdfs:comment>
        <rdfs:label>fare_media_type:2</rdfs:label>
    </owl:NamedIndividual>
    


    <!-- http://gtfs.org/fare_media_type_3 -->


    <owl:NamedIndividual rdf:about="http://gtfs.org/fare_media_type_3">
        <rdf:type rdf:resource="http://gtfs.org/FareMediaTypeEnum"/>
        <gtfs:hasEnumValue>3</gtfs:hasEnumValue>
        <rdfs:comment>cEMV</rdfs:comment>
        <rdfs:label>fare_media_type:3</rdfs:label>
    </owl:NamedIndividual>
    


    <!-- http://gtfs.org/fare_media_type_4 -->


    <owl:NamedIndividual rdf:about="http://gtfs.org/fare_media_type_4">
        <rdf:type rdf:resource="http://gtfs.org/FareMediaTypeEnum"/>
        <gtfs:hasEnumValue>4</gtfs:hasEnumValue>
        <rdfs:comment>Mobile app</rdfs:comment>
        <rdfs:label>fare_media_type:4</rdfs:label>
    </owl:NamedIndividual>
    


    <!-- http://gtfs.org/fare_product_id -->


    <owl:NamedIndividual rdf:about="http://gtfs.org/fare_product_id">
        <rdf:type rdf:resource="http://gtfs.org/Field"/>
        <gtfs:isFieldOf rdf:resource="http://gtfs.org/fare_leg_rules.txt"/>
        <gtfs:isFieldOf rdf:resource="http://gtfs.org/fare_products.txt"/>
        <gtfs:isFieldOf rdf:resource="http://gtfs.org/fare_transfer_rules.txt"/>
        <gtfs:isOptionalIn rdf:resource="http://gtfs.org/fare_transfer_rules.txt"/>
        <gtfs:isRequiredIn rdf:resource="http://gtfs.org/fare_leg_rules.txt"/>
        <gtfs:isRequiredIn rdf:resource="http://gtfs.org/fare_products.txt"/>
        <gtfs:isType rdf:resource="http://gtfs.org/ID"/>
        <gtfs:hasAdditionalInfo>Foreign ID referencing fare_products.fare_product_id</gtfs:hasAdditionalInfo>
        <gtfs:hasAdditionalInfo>This field is used to uniquely identify a fare product.</gtfs:hasAdditionalInfo>
        <gtfs:isForeignID rdf:resource="http://gtfs.org/fare_leg_rules.txt"/>
        <gtfs:isUniqueID rdf:resource="http://gtfs.org/fare_products.txt"/>
        <rdfs:comment>Identifies a fare product.</rdfs:comment>
        <rdfs:comment>The fare product required to transfer between two fare legs. If empty, the cost of the transfer rule is 0.</rdfs:comment>
        <rdfs:comment>The fare product required to travel the leg.</rdfs:comment>
        <rdfs:label>fare_product_id</rdfs:label>
    </owl:NamedIndividual>
    


    <!-- http://gtfs.org/fare_product_name -->


    <owl:NamedIndividual rdf:about="http://gtfs.org/fare_product_name">
        <rdf:type rdf:resource="http://gtfs.org/Field"/>
        <gtfs:isFieldOf rdf:resource="http://gtfs.org/fare_products.txt"/>
        <gtfs:isOptionalIn rdf:resource="http://gtfs.org/fare_products.txt"/>
        <gtfs:isType rdf:resource="http://gtfs.org/Text"/>
        <gtfs:hasAdditionalInfo>Type: Text</gtfs:hasAdditionalInfo>
        <rdfs:comment>The name of the fare product as displayed to riders.</rdfs:comment>
        <rdfs:label>fare_product_name</rdfs:label>
    </owl:NamedIndividual>
    


    <!-- http://gtfs.org/fare_products.txt -->


    <owl:NamedIndividual rdf:about="http://gtfs.org/fare_products.txt">
        <rdf:type rdf:resource="http://gtfs.org/File"/>
        <gtfs:hasField rdf:resource="http://gtfs.org/amount"/>
        <gtfs:hasField rdf:resource="http://gtfs.org/currency"/>
        <gtfs:hasField rdf:resource="http://gtfs.org/fare_media_id"/>
        <gtfs:hasField rdf:resource="http://gtfs.org/fare_product_id"/>
        <gtfs:hasField rdf:resource="http://gtfs.org/fare_product_name"/>
        <gtfs:isFileOf rdf:resource="http://gtfs.org/GTFS_Static"/>
        <gtfs:isOptionalIn rdf:resource="http://gtfs.org/GTFS_Static"/>
        <gtfs:hasAdditionalInfo>File describes fare products not represented in fare_attributes.txt and fare_rules.txt.</gtfs:hasAdditionalInfo>
        <rdfs:comment>To describe the different types of tickets or fares that can be purchased by riders.</rdfs:comment>
        <rdfs:label>fare_products.txt</rdfs:label>
    </owl:NamedIndividual>
    


    <!-- http://gtfs.org/fare_rules.txt -->


    <owl:NamedIndividual rdf:about="http://gtfs.org/fare_rules.txt">
        <rdf:type rdf:resource="http://gtfs.org/File"/>
        <gtfs:hasField rdf:resource="http://gtfs.org/contains_id"/>
        <gtfs:hasField rdf:resource="http://gtfs.org/destination_id"/>
        <gtfs:hasField rdf:resource="http://gtfs.org/fare_id"/>
        <gtfs:hasField rdf:resource="http://gtfs.org/origin_id"/>
        <gtfs:hasField rdf:resource="http://gtfs.org/route_id"/>
        <gtfs:isFileOf rdf:resource="http://gtfs.org/GTFS_Static"/>
        <gtfs:isOptionalIn rdf:resource="http://gtfs.org/GTFS_Static"/>
        <rdfs:comment>Rules to apply fares for itineraries.</rdfs:comment>
        <rdfs:label>fare_rules.txt</rdfs:label>
    </owl:NamedIndividual>
    


    <!-- http://gtfs.org/fare_transfer_rules.txt -->


    <owl:NamedIndividual rdf:about="http://gtfs.org/fare_transfer_rules.txt">
        <rdf:type rdf:resource="http://gtfs.org/File"/>
        <gtfs:hasField rdf:resource="http://gtfs.org/duration_limit"/>
        <gtfs:hasField rdf:resource="http://gtfs.org/duration_limit_type"/>
        <gtfs:hasField rdf:resource="http://gtfs.org/fare_product_id"/>
        <gtfs:hasField rdf:resource="http://gtfs.org/fare_transfer_type"/>
        <gtfs:hasField rdf:resource="http://gtfs.org/from_leg_group_id"/>
        <gtfs:hasField rdf:resource="http://gtfs.org/to_leg_group_id"/>
        <gtfs:hasField rdf:resource="http://gtfs.org/transfer_count"/>
        <gtfs:isFileOf rdf:resource="http://gtfs.org/GTFS_Static"/>
        <gtfs:isOptionalIn rdf:resource="http://gtfs.org/GTFS_Static"/>
        <gtfs:hasAdditionalInfo>File provides a more detailed method for modeling fare structures.</gtfs:hasAdditionalInfo>
        <rdfs:comment>Fare rules for transfers between legs of travel.</rdfs:comment>
        <rdfs:label>fare_transfer_rules.txt</rdfs:label>
    </owl:NamedIndividual>
    


    <!-- http://gtfs.org/fare_transfer_type -->


    <owl:NamedIndividual rdf:about="http://gtfs.org/fare_transfer_type">
        <rdf:type rdf:resource="http://gtfs.org/Field"/>
        <gtfs:isFieldOf rdf:resource="http://gtfs.org/fare_transfer_rules.txt"/>
        <gtfs:isPresence rdf:resource="http://gtfs.org/Required"/>
        <gtfs:isRequiredIn rdf:resource="http://gtfs.org/fare_transfer_rules.txt"/>
        <gtfs:isType rdf:resource="http://gtfs.org/FareTransferTypeEnum"/>
        <gtfs:hasAdditionalInfo>Valid options are: 0 - From-leg fare_leg_rules.fare_product_id plus fare_transfer_rules.fare_product_id; A + AB. 1 - From-leg fare_leg_rules.fare_product_id plus fare_transfer_rules.fare_product_id plus to-leg fare_leg_rules.fare_product_id; A + AB + B. 2 - fare_transfer_rules.fare_product_id; AB. Cost processing interactions between multiple transfers in a journey: Where S indicates the total processed cost of the preceding leg(s) and transfer(s.</gtfs:hasAdditionalInfo>
        <rdfs:comment>Indicates the cost processing method of transferring between legs in a journey</rdfs:comment>
        <rdfs:label>fare_transfer_type</rdfs:label>
    </owl:NamedIndividual>
    


    <!-- http://gtfs.org/fare_transfer_type_0 -->


    <owl:NamedIndividual rdf:about="http://gtfs.org/fare_transfer_type_0">
        <rdf:type rdf:resource="http://gtfs.org/FareTransferTypeEnum"/>
        <gtfs:hasEnumValue>0</gtfs:hasEnumValue>
        <rdfs:comment>From-leg fare_leg_rules.fare_product_id plus fare_transfer_rules.fare_product_id; A + AB</rdfs:comment>
        <rdfs:label>fare_transfer_type:0</rdfs:label>
    </owl:NamedIndividual>
    


    <!-- http://gtfs.org/fare_transfer_type_1 -->


    <owl:NamedIndividual rdf:about="http://gtfs.org/fare_transfer_type_1">
        <rdf:type rdf:resource="http://gtfs.org/FareTransferTypeEnum"/>
        <gtfs:hasEnumValue>1</gtfs:hasEnumValue>
        <rdfs:comment>From-leg fare_leg_rules.fare_product_id plus fare_transfer_rules.fare_product_id plus to-leg fare_leg_rules.fare_product_id; A + AB + B</rdfs:comment>
        <rdfs:label>fare_transfer_type:1</rdfs:label>
    </owl:NamedIndividual>
    


    <!-- http://gtfs.org/fare_transfer_type_2 -->


    <owl:NamedIndividual rdf:about="http://gtfs.org/fare_transfer_type_2">
        <rdf:type rdf:resource="http://gtfs.org/FareTransferTypeEnum"/>
        <gtfs:hasEnumValue>2</gtfs:hasEnumValue>
        <rdfs:comment>fare_transfer_rules.fare_product_id; AB</rdfs:comment>
        <rdfs:label>fare_transfer_type:2</rdfs:label>
    </owl:NamedIndividual>
    


    <!-- http://gtfs.org/feed_contact_email -->


    <owl:NamedIndividual rdf:about="http://gtfs.org/feed_contact_email">
        <rdf:type rdf:resource="http://gtfs.org/Field"/>
        <gtfs:isFieldOf rdf:resource="http://gtfs.org/feed_info.txt"/>
        <gtfs:isOptionalIn rdf:resource="http://gtfs.org/feed_info.txt"/>
        <gtfs:isType rdf:resource="http://gtfs.org/Email"/>
        <gtfs:hasAdditionalInfo>Email address for communication regarding the GTFS dataset and data publishing practices. `feed_contact_email` is a technical contact for GTFS-consuming applications. Provide customer service contact information through [agency.txt](#agencytxt). It&apos;s recommended that at least one of `feed_contact_email` or `feed_contact_url` are provided.</gtfs:hasAdditionalInfo>
        <rdfs:comment>Email address for communication regarding the GTFS dataset and data publishing practices. `feed_contact_email` is a technical contact for GTFS-consuming applications. Provide customer service contact information through [agency.txt](#agencytxt). It&apos;s recommended that at least one of `feed_contact_email` or `feed_contact_url` are provided.</rdfs:comment>
        <rdfs:label>feed_contact_email</rdfs:label>
    </owl:NamedIndividual>
    


    <!-- http://gtfs.org/feed_contact_url -->


    <owl:NamedIndividual rdf:about="http://gtfs.org/feed_contact_url">
        <rdf:type rdf:resource="http://gtfs.org/Field"/>
        <gtfs:isFieldOf rdf:resource="http://gtfs.org/feed_info.txt"/>
        <gtfs:isOptionalIn rdf:resource="http://gtfs.org/feed_info.txt"/>
        <gtfs:isType rdf:resource="http://gtfs.org/URL"/>
        <gtfs:hasAdditionalInfo>URL for contact information</gtfs:hasAdditionalInfo>
        <rdfs:comment>URL for contact information, a web-form, support desk, or other tools for communication regarding the GTFS dataset and data publishing practices. `feed_contact_url` is a technical contact for GTFS-consuming applications. Provide customer service contact information through agency.txt. It&apos;s recommended that at least one of `feed_contact_url` or `feed_contact_email` are provided.</rdfs:comment>
        <rdfs:label>feed_contact_url</rdfs:label>
    </owl:NamedIndividual>
    


    <!-- http://gtfs.org/feed_end_date -->


    <owl:NamedIndividual rdf:about="http://gtfs.org/feed_end_date">
        <rdf:type rdf:resource="http://gtfs.org/Field"/>
        <gtfs:isFieldOf rdf:resource="http://gtfs.org/feed_info.txt"/>
        <gtfs:isRecommendedIn rdf:resource="http://gtfs.org/feed_info.txt"/>
        <gtfs:isType rdf:resource="http://gtfs.org/Date"/>
        <gtfs:hasAdditionalInfo>The end date for the feed</gtfs:hasAdditionalInfo>
        <rdfs:comment>(see above)</rdfs:comment>
        <rdfs:label>feed_end_date</rdfs:label>
    </owl:NamedIndividual>
    


    <!-- http://gtfs.org/feed_info.txt -->


    <owl:NamedIndividual rdf:about="http://gtfs.org/feed_info.txt">
        <rdf:type rdf:resource="http://gtfs.org/File"/>
        <gtfs:hasField rdf:resource="http://gtfs.org/default_lang"/>
        <gtfs:hasField rdf:resource="http://gtfs.org/feed_contact_email"/>
        <gtfs:hasField rdf:resource="http://gtfs.org/feed_contact_url"/>
        <gtfs:hasField rdf:resource="http://gtfs.org/feed_end_date"/>
        <gtfs:hasField rdf:resource="http://gtfs.org/feed_lang"/>
        <gtfs:hasField rdf:resource="http://gtfs.org/feed_publisher_name"/>
        <gtfs:hasField rdf:resource="http://gtfs.org/feed_publisher_url"/>
        <gtfs:hasField rdf:resource="http://gtfs.org/feed_start_date"/>
        <gtfs:hasField rdf:resource="http://gtfs.org/feed_version"/>
        <gtfs:isFileOf rdf:resource="http://gtfs.org/GTFS_Static"/>
        <gtfs:isOptionalIn rdf:resource="http://gtfs.org/GTFS_Static"/>
        <rdfs:comment>Dataset metadata, including publisher, version, and expiration information.</rdfs:comment>
        <rdfs:label>feed_info.txt</rdfs:label>
    </owl:NamedIndividual>
    


    <!-- http://gtfs.org/feed_lang -->


    <owl:NamedIndividual rdf:about="http://gtfs.org/feed_lang">
        <rdf:type rdf:resource="http://gtfs.org/Field"/>
        <gtfs:isFieldOf rdf:resource="http://gtfs.org/feed_info.txt"/>
        <gtfs:isRequiredIn rdf:resource="http://gtfs.org/feed_info.txt"/>
        <gtfs:isType rdf:resource="http://gtfs.org/LanguageCode"/>
        <gtfs:hasAdditionalInfo>The `feed_lang` field is crucial for specifying the default language used in the dataset and providing translations for multilingual datasets.</gtfs:hasAdditionalInfo>
        <gtfs:hasExample>None</gtfs:hasExample>
        <rdfs:comment>Default language used for the text in this dataset. This setting helps GTFS consumers choose capitalization rules and other language-specific settings for the dataset. The file `translations.txt` can be used if the text needs to be translated into languages other than the default one. The default language may be multilingual for datasets with the original text in multiple languages. In such cases, the `feed_lang` field should contain the language code `mul` defined by the norm ISO 639-2, and a translation for each language used in the dataset should be provided in `translations.txt`. If all the original text in the dataset is in the same language, then `mul` should not be used.</rdfs:comment>
        <rdfs:label>feed_lang</rdfs:label>
    </owl:NamedIndividual>
    


    <!-- http://gtfs.org/feed_publisher_name -->


    <owl:NamedIndividual rdf:about="http://gtfs.org/feed_publisher_name">
        <rdf:type rdf:resource="http://gtfs.org/Field"/>
        <gtfs:isFieldOf rdf:resource="http://gtfs.org/feed_info.txt"/>
        <gtfs:isRequiredIn rdf:resource="http://gtfs.org/feed_info.txt"/>
        <gtfs:isType rdf:resource="http://gtfs.org/Text"/>
        <gtfs:hasAdditionalInfo>Type: Text</gtfs:hasAdditionalInfo>
        <rdfs:comment>Full name of the organization that publishes the dataset. This may be the same as one of the agency.agency_name values.</rdfs:comment>
        <rdfs:label>feed_publisher_name</rdfs:label>
    </owl:NamedIndividual>
    


    <!-- http://gtfs.org/feed_publisher_url -->


    <owl:NamedIndividual rdf:about="http://gtfs.org/feed_publisher_url">
        <rdf:type rdf:resource="http://gtfs.org/Field"/>
        <gtfs:isFieldOf rdf:resource="http://gtfs.org/feed_info.txt"/>
        <gtfs:isRequiredIn rdf:resource="http://gtfs.org/feed_info.txt"/>
        <gtfs:isType rdf:resource="http://gtfs.org/URL"/>
        <gtfs:hasAdditionalInfo>URL of the dataset publishing organization&apos;s website.</gtfs:hasAdditionalInfo>
        <rdfs:comment>URL of the dataset publishing organization&apos;s website. This may be the same as one of the agency.agency_url values.</rdfs:comment>
        <rdfs:label>feed_publisher_url</rdfs:label>
    </owl:NamedIndividual>
    


    <!-- http://gtfs.org/feed_start_date -->


    <owl:NamedIndividual rdf:about="http://gtfs.org/feed_start_date">
        <rdf:type rdf:resource="http://gtfs.org/Field"/>
        <gtfs:isFieldOf rdf:resource="http://gtfs.org/feed_info.txt"/>
        <gtfs:isRecommendedIn rdf:resource="http://gtfs.org/feed_info.txt"/>
        <gtfs:isType rdf:resource="http://gtfs.org/Date"/>
        <rdfs:comment>The dataset provides complete and reliable schedule information for service in the period from the beginning of the `feed_start_date` day to the end of the `feed_end_date` day. Both days may be left empty if unavailable. The `feed_end_date` date must not precede the `feed_start_date` date if both are given. It is recommended that dataset providers give schedule data outside this period to advise of likely future service, but dataset consumers should treat it mindful of its non-authoritative status. If `feed_start_date` or `feed_end_date` extend beyond the active calendar dates defined in calendar.txt and calendar_dates.txt, the dataset is making an explicit assertion that there is no service for dates within the `feed_start_date` or `feed_end_date` range but not included in the active calendar dates.</rdfs:comment>
        <rdfs:label>feed_start_date</rdfs:label>
    </owl:NamedIndividual>
    


    <!-- http://gtfs.org/feed_version -->


    <owl:NamedIndividual rdf:about="http://gtfs.org/feed_version">
        <rdf:type rdf:resource="http://gtfs.org/Field"/>
        <gtfs:isFieldOf rdf:resource="http://gtfs.org/feed_info.txt"/>
        <gtfs:isRecommendedIn rdf:resource="http://gtfs.org/feed_info.txt"/>
        <gtfs:isType rdf:resource="http://gtfs.org/Text"/>
        <gtfs:hasAdditionalInfo>Recommended field to indicate the version of the GTFS dataset.</gtfs:hasAdditionalInfo>
        <rdfs:comment>String that indicates the current version of their GTFS dataset. GTFS-consuming applications can display this value to help dataset publishers determine whether the latest dataset has been incorporated.</rdfs:comment>
        <rdfs:label>feed_version</rdfs:label>
    </owl:NamedIndividual>
    


    <!-- http://gtfs.org/field_name -->


    <owl:NamedIndividual rdf:about="http://gtfs.org/field_name">
        <rdf:type rdf:resource="http://gtfs.org/Field"/>
        <gtfs:isFieldOf rdf:resource="http://gtfs.org/translations.txt"/>
        <gtfs:isRequiredIn rdf:resource="http://gtfs.org/translations.txt"/>
        <gtfs:isType rdf:resource="http://gtfs.org/Text"/>
        <gtfs:hasAdditionalInfo>Fields with type `Text` may be translated, fields with type `URL`, `Email` and `Phone number` may also be “translated” to provide resources in the correct language. Fields with other types should not be translated.</gtfs:hasAdditionalInfo>
        <gtfs:isUniqueID rdf:resource="http://gtfs.org/translations.txt"/>
        <rdfs:comment>Name of the field to be translated. Fields with type `Text` may be translated, fields with type `URL`, `Email` and `Phone number` may also be “translated” to provide resources in the correct language. Fields with other types should not be translated.</rdfs:comment>
        <rdfs:label>field_name</rdfs:label>
    </owl:NamedIndividual>
    


    <!-- http://gtfs.org/field_value -->


    <owl:NamedIndividual rdf:about="http://gtfs.org/field_value">
        <rdf:type rdf:resource="http://gtfs.org/Field"/>
        <gtfs:isConditionallyRequiredIn rdf:resource="http://gtfs.org/translations.txt"/>
        <gtfs:isFieldOf rdf:resource="http://gtfs.org/translations.txt"/>
        <gtfs:isType rdf:resource="http://gtfs.org/Text"/>
        <gtfs:hasAdditionalInfo>Instead of defining which record should be translated by using `record_id` and `record_sub_id`, this field can be used to define the value which should be translated. When used, the translation will be applied when the fields identified by `table_name` and `field_name` contains the exact same value defined in field_value.

The field must have exactly the value defined in `field_value`. If only a subset of the value matches `field_value`, the translation won’t be applied.

If two translation rules match the same record (one with `field_value`, and the other one with `record_id`), the rule with `record_id` takes precedence.</gtfs:hasAdditionalInfo>
        <gtfs:hasCondition>- **Forbidden** if `table_name` is `feed_info`.
- **Forbidden** if `record_id` is defined.
- **Required** if `record_id` is empty.</gtfs:hasCondition>
        <gtfs:isUniqueID rdf:resource="http://gtfs.org/translations.txt"/>
        <rdfs:comment>Instead of defining which record should be translated by using `record_id` and `record_sub_id`, this field can be used to define the value which should be translated. When used, the translation will be applied when the fields identified by `table_name` and `field_name` contains the exact same value defined in field_value.

The field must have exactly the value defined in `field_value`. If only a subset of the value matches `field_value`, the translation won’t be applied.

If two translation rules match the same record (one with `field_value`, and the other one with `record_id`), the rule with `record_id` takes precedence.</rdfs:comment>
        <rdfs:label>field_value</rdfs:label>
    </owl:NamedIndividual>
    


    <!-- http://gtfs.org/frequencies.txt -->


    <owl:NamedIndividual rdf:about="http://gtfs.org/frequencies.txt">
        <rdf:type rdf:resource="http://gtfs.org/File"/>
        <gtfs:hasField rdf:resource="http://gtfs.org/end_time"/>
        <gtfs:hasField rdf:resource="http://gtfs.org/exact_times"/>
        <gtfs:hasField rdf:resource="http://gtfs.org/headway_secs"/>
        <gtfs:hasField rdf:resource="http://gtfs.org/start_time"/>
        <gtfs:hasField rdf:resource="http://gtfs.org/trip_id"/>
        <gtfs:isFileOf rdf:resource="http://gtfs.org/GTFS_Static"/>
        <gtfs:isOptionalIn rdf:resource="http://gtfs.org/GTFS_Static"/>
        <rdfs:comment>Headway (time between trips) for headway-based service or a compressed representation of fixed-schedule service.</rdfs:comment>
        <rdfs:label>frequencies.txt</rdfs:label>
    </owl:NamedIndividual>
    


    <!-- http://gtfs.org/friday -->


    <owl:NamedIndividual rdf:about="http://gtfs.org/friday">
        <rdf:type rdf:resource="http://gtfs.org/Field"/>
        <gtfs:isFieldOf rdf:resource="http://gtfs.org/calendar.txt"/>
        <gtfs:isPresence rdf:resource="http://gtfs.org/Required"/>
        <gtfs:isRequiredIn rdf:resource="http://gtfs.org/calendar.txt"/>
        <gtfs:isType rdf:resource="http://gtfs.org/FridayEnum"/>
        <gtfs:hasAdditionalInfo>Enum field representing the behavior on Fridays</gtfs:hasAdditionalInfo>
        <rdfs:comment>Functions in the same way as `monday` except applies to Fridays</rdfs:comment>
        <rdfs:label>friday</rdfs:label>
    </owl:NamedIndividual>
    


    <!-- http://gtfs.org/friday_0 -->


    <owl:NamedIndividual rdf:about="http://gtfs.org/friday_0">
        <rdf:type rdf:resource="http://gtfs.org/FridayEnum"/>
        <gtfs:hasEnumValue>0</gtfs:hasEnumValue>
        <rdfs:comment>No</rdfs:comment>
        <rdfs:label>friday:0</rdfs:label>
    </owl:NamedIndividual>
    


    <!-- http://gtfs.org/friday_1 -->


    <owl:NamedIndividual rdf:about="http://gtfs.org/friday_1">
        <rdf:type rdf:resource="http://gtfs.org/FridayEnum"/>
        <gtfs:hasEnumValue>1</gtfs:hasEnumValue>
        <rdfs:comment>Yes</rdfs:comment>
        <rdfs:label>friday:1</rdfs:label>
    </owl:NamedIndividual>
    


    <!-- http://gtfs.org/from_area_id -->


    <owl:NamedIndividual rdf:about="http://gtfs.org/from_area_id">
        <rdf:type rdf:resource="http://gtfs.org/Field"/>
        <gtfs:isFieldOf rdf:resource="http://gtfs.org/fare_leg_rules.txt"/>
        <gtfs:isOptionalIn rdf:resource="http://gtfs.org/fare_leg_rules.txt"/>
        <gtfs:isType rdf:resource="http://gtfs.org/ID"/>
        <gtfs:hasAdditionalInfo>If there are no matching fare_leg_rules.from_area_id values to the area_id being filtered, empty fare_leg_rules.from_area_id will be matched by default. An empty entry in fare_leg_rules.from_area_id corresponds to all areas defined in areas.area_id excluding the ones listed under fare_leg_rules.from_area_id</gtfs:hasAdditionalInfo>
        <gtfs:isForeignID rdf:resource="http://gtfs.org/fare_leg_rules.txt"/>
        <rdfs:comment>Identifies a departure area.</rdfs:comment>
        <rdfs:label>from_area_id</rdfs:label>
    </owl:NamedIndividual>
    


    <!-- http://gtfs.org/from_leg_group_id -->


    <owl:NamedIndividual rdf:about="http://gtfs.org/from_leg_group_id">
        <rdf:type rdf:resource="http://gtfs.org/Field"/>
        <gtfs:isFieldOf rdf:resource="http://gtfs.org/fare_transfer_rules.txt"/>
        <gtfs:isOptionalIn rdf:resource="http://gtfs.org/fare_transfer_rules.txt"/>
        <gtfs:isType rdf:resource="http://gtfs.org/ID"/>
        <gtfs:hasAdditionalInfo>Foreign ID referencing fare_leg_rules.leg_group_id</gtfs:hasAdditionalInfo>
        <gtfs:isForeignID rdf:resource="http://gtfs.org/fare_transfer_rules.txt"/>
        <rdfs:comment>Identifies a group of pre-transfer fare leg rules.

If there are no matching fare_transfer_rules.from_leg_group_id values to the leg_group_id being filtered, empty fare_transfer_rules.from_leg_group_id will be matched by default. 

An empty entry in fare_transfer_rules.from_leg_group_id corresponds to all leg groups defined under fare_leg_rules.leg_group_id excluding the ones listed under fare_transfer_rules.from_leg_group_id</rdfs:comment>
        <rdfs:label>from_leg_group_id</rdfs:label>
    </owl:NamedIndividual>
    


    <!-- http://gtfs.org/from_route_id -->


    <owl:NamedIndividual rdf:about="http://gtfs.org/from_route_id">
        <rdf:type rdf:resource="http://gtfs.org/Field"/>
        <gtfs:isFieldOf rdf:resource="http://gtfs.org/transfers.txt"/>
        <gtfs:isOptionalIn rdf:resource="http://gtfs.org/transfers.txt"/>
        <gtfs:isType rdf:resource="http://gtfs.org/ID"/>
        <gtfs:hasAdditionalInfo>Foreign ID referencing `routes.route_id`</gtfs:hasAdditionalInfo>
        <gtfs:isForeignID rdf:resource="http://gtfs.org/transfers.txt"/>
        <rdfs:comment>Identifies a route where a connection begins. If `from_route_id` is defined, the transfer will apply to the arriving trip on the route for the given `from_stop_id`. If both `from_trip_id` and `from_route_id` are defined, the `trip_id` must belong to the `route_id`, and `from_trip_id` will take precedence.</rdfs:comment>
        <rdfs:label>from_route_id</rdfs:label>
    </owl:NamedIndividual>
    


    <!-- http://gtfs.org/from_stop_id -->


    <owl:NamedIndividual rdf:about="http://gtfs.org/from_stop_id">
        <rdf:type rdf:resource="http://gtfs.org/Field"/>
        <gtfs:isConditionallyRequiredIn rdf:resource="http://gtfs.org/transfers.txt"/>
        <gtfs:isFieldOf rdf:resource="http://gtfs.org/pathways.txt"/>
        <gtfs:isFieldOf rdf:resource="http://gtfs.org/transfers.txt"/>
        <gtfs:isRequiredIn rdf:resource="http://gtfs.org/pathways.txt"/>
        <gtfs:isType rdf:resource="http://gtfs.org/ID"/>
        <gtfs:hasAdditionalInfo>Foreign ID referencing stops.stop_id</gtfs:hasAdditionalInfo>
        <gtfs:hasCondition>If this field refers to a station, the transfer rule applies to all its child stops. Referring to a station is forbidden for transfer_types 4 and 5.</gtfs:hasCondition>
        <gtfs:isForeignID rdf:resource="http://gtfs.org/pathways.txt"/>
        <gtfs:isForeignID rdf:resource="http://gtfs.org/transfers.txt"/>
        <rdfs:comment>Identifies a stop or station where a connection between routes begins. If this field refers to a station, the transfer rule applies to all its child stops. Referring to a station is forbidden for transfer_types 4 and 5.</rdfs:comment>
        <rdfs:comment>Location at which the pathway begins. Must contain a stop_id that identifies a platform (location_type=0 or empty), entrance/exit (location_type=2), generic node (location_type=3) or boarding area (location_type=4). Values for stop_id that identify stations (location_type=1) are forbidden.</rdfs:comment>
        <rdfs:label>from_stop_id</rdfs:label>
    </owl:NamedIndividual>
    


    <!-- http://gtfs.org/from_timeframe_group_id -->


    <owl:NamedIndividual rdf:about="http://gtfs.org/from_timeframe_group_id">
        <rdf:type rdf:resource="http://gtfs.org/Field"/>
        <gtfs:isFieldOf rdf:resource="http://gtfs.org/fare_leg_rules.txt"/>
        <gtfs:isOptionalIn rdf:resource="http://gtfs.org/fare_leg_rules.txt"/>
        <gtfs:isType rdf:resource="http://gtfs.org/ID"/>
        <gtfs:hasAdditionalInfo>Foreign ID referencing timeframes.timeframe_group_id</gtfs:hasAdditionalInfo>
        <gtfs:isForeignID rdf:resource="http://gtfs.org/fare_leg_rules.txt"/>
        <rdfs:comment>Defines the timeframe for the fare validation event at the start of the fare leg. The “start time” of the fare leg is the time at which the event is scheduled to occur. For example, the time could be the scheduled departure time of a bus at the start of a fare leg where the rider boards and validates their fare. For the rule matching semantics below, the start time is computed in local time, as determined by Local Time Semantics of timeframes.txt. The stop or station of the fare leg’s departure event should be used for timezone resolution, where appropriate. For a fare leg rule that specifies a from_timeframe_group_id, that rule will match a particular leg if there exists at least one record in timeframes.txt where all of the following conditions are true: - The value of timeframe_group_id is equal to the from_timeframe_group_id value. - The set of days identified by the record’s service_id contains the “current day” of the fare leg’s start time. - The “time-of-day” of the fare leg&apos;s start time is greater than or equal to the record’s timeframes.start_time value and less than the timeframes.end_time value. An empty fare_leg_rules.from_timeframe_group_id indicates that the start time of the leg does not affect the matching of this rule.</rdfs:comment>
        <rdfs:label>from_timeframe_group_id</rdfs:label>
    </owl:NamedIndividual>
    


    <!-- http://gtfs.org/from_trip_id -->


    <owl:NamedIndividual rdf:about="http://gtfs.org/from_trip_id">
        <rdf:type rdf:resource="http://gtfs.org/Field"/>
        <gtfs:isConditionallyRequiredIn rdf:resource="http://gtfs.org/transfers.txt"/>
        <gtfs:isFieldOf rdf:resource="http://gtfs.org/transfers.txt"/>
        <gtfs:isType rdf:resource="http://gtfs.org/ID"/>
        <gtfs:hasAdditionalInfo>Foreign ID referencing `trips.trip_id`</gtfs:hasAdditionalInfo>
        <gtfs:hasCondition>REQUIRED if `transfer_type` is `4` or `5`.</gtfs:hasCondition>
        <gtfs:isForeignID rdf:resource="http://gtfs.org/transfers.txt"/>
        <rdfs:comment>Identifies a trip where a connection between routes begins. If `from_trip_id` is defined, the transfer will apply to the arriving trip for the given `from_stop_id`. If both `from_trip_id` and `from_route_id` are defined, the `trip_id` must belong to the `route_id`, and `from_trip_id` will take precedence. REQUIRED if `transfer_type` is `4` or `5`.</rdfs:comment>
        <rdfs:label>from_trip_id</rdfs:label>
    </owl:NamedIndividual>
    


    <!-- http://gtfs.org/headway_secs -->


    <owl:NamedIndividual rdf:about="http://gtfs.org/headway_secs">
        <rdf:type rdf:resource="http://gtfs.org/Field"/>
        <gtfs:isFieldOf rdf:resource="http://gtfs.org/frequencies.txt"/>
        <gtfs:isRequiredIn rdf:resource="http://gtfs.org/frequencies.txt"/>
        <gtfs:isType rdf:resource="http://gtfs.org/Integer"/>
        <gtfs:hasAdditionalInfo>Positive integer</gtfs:hasAdditionalInfo>
        <rdfs:comment>Time, in seconds, between departures from the same stop (headway) for the trip, during the time interval specified by `start_time` and `end_time`. Multiple headways may be defined for the same trip, but must not overlap. New headways may start at the exact time the previous headway ends.</rdfs:comment>
        <rdfs:label>headway_secs</rdfs:label>
    </owl:NamedIndividual>
    


    <!-- http://gtfs.org/is_authority -->


    <owl:NamedIndividual rdf:about="http://gtfs.org/is_authority">
        <rdf:type rdf:resource="http://gtfs.org/Field"/>
        <gtfs:isFieldOf rdf:resource="http://gtfs.org/attributions.txt"/>
        <gtfs:isOptionalIn rdf:resource="http://gtfs.org/attributions.txt"/>
        <gtfs:isPresence rdf:resource="http://gtfs.org/Optional"/>
        <gtfs:isType rdf:resource="http://gtfs.org/IsAuthorityEnum"/>
        <gtfs:hasAdditionalInfo>Enum field representing the role of the organization as an authority.</gtfs:hasAdditionalInfo>
        <rdfs:comment>Functions in the same way as `is_producer` except the role of the organization is authority.</rdfs:comment>
        <rdfs:label>is_authority</rdfs:label>
    </owl:NamedIndividual>
    


    <!-- http://gtfs.org/is_authority_0 -->


    <owl:NamedIndividual rdf:about="http://gtfs.org/is_authority_0">
        <rdf:type rdf:resource="http://gtfs.org/IsAuthorityEnum"/>
        <gtfs:hasEnumValue>0</gtfs:hasEnumValue>
        <rdfs:comment>False</rdfs:comment>
        <rdfs:label>is_authority:0</rdfs:label>
    </owl:NamedIndividual>
    


    <!-- http://gtfs.org/is_authority_1 -->


    <owl:NamedIndividual rdf:about="http://gtfs.org/is_authority_1">
        <rdf:type rdf:resource="http://gtfs.org/IsAuthorityEnum"/>
        <gtfs:hasEnumValue>1</gtfs:hasEnumValue>
        <rdfs:comment>True</rdfs:comment>
        <rdfs:label>is_authority:1</rdfs:label>
    </owl:NamedIndividual>
    


    <!-- http://gtfs.org/is_bidirectional -->


    <owl:NamedIndividual rdf:about="http://gtfs.org/is_bidirectional">
        <rdf:type rdf:resource="http://gtfs.org/Field"/>
        <gtfs:isFieldOf rdf:resource="http://gtfs.org/pathways.txt"/>
        <gtfs:isPresence rdf:resource="http://gtfs.org/Required"/>
        <gtfs:isRequiredIn rdf:resource="http://gtfs.org/pathways.txt"/>
        <gtfs:isType rdf:resource="http://gtfs.org/IsBidirectionalEnum"/>
        <gtfs:hasAdditionalInfo>Exit gates (pathway_mode=7) must not be bidirectional.</gtfs:hasAdditionalInfo>
        <rdfs:comment>Indicates the direction that the pathway can be taken</rdfs:comment>
        <rdfs:label>is_bidirectional</rdfs:label>
    </owl:NamedIndividual>
    


    <!-- http://gtfs.org/is_bidirectional_0 -->


    <owl:NamedIndividual rdf:about="http://gtfs.org/is_bidirectional_0">
        <rdf:type rdf:resource="http://gtfs.org/IsBidirectionalEnum"/>
        <gtfs:hasEnumValue>0</gtfs:hasEnumValue>
        <rdfs:comment>Unidirectional pathway that can only be used from from_stop_id to to_stop_id.</rdfs:comment>
        <rdfs:label>is_bidirectional:0</rdfs:label>
    </owl:NamedIndividual>
    


    <!-- http://gtfs.org/is_bidirectional_1 -->


    <owl:NamedIndividual rdf:about="http://gtfs.org/is_bidirectional_1">
        <rdf:type rdf:resource="http://gtfs.org/IsBidirectionalEnum"/>
        <gtfs:hasEnumValue>1</gtfs:hasEnumValue>
        <rdfs:comment>Bidirectional pathway that can be used in both directions.</rdfs:comment>
        <rdfs:label>is_bidirectional:1</rdfs:label>
    </owl:NamedIndividual>
    


    <!-- http://gtfs.org/is_operator -->


    <owl:NamedIndividual rdf:about="http://gtfs.org/is_operator">
        <rdf:type rdf:resource="http://gtfs.org/Field"/>
        <gtfs:isFieldOf rdf:resource="http://gtfs.org/attributions.txt"/>
        <gtfs:isOptionalIn rdf:resource="http://gtfs.org/attributions.txt"/>
        <gtfs:isPresence rdf:resource="http://gtfs.org/Optional"/>
        <gtfs:isType rdf:resource="http://gtfs.org/IsOperatorEnum"/>
        <gtfs:hasAdditionalInfo>Enum type field</gtfs:hasAdditionalInfo>
        <rdfs:comment>Functions in the same way as `is_producer` except the role of the organization is operator.</rdfs:comment>
        <rdfs:label>is_operator</rdfs:label>
    </owl:NamedIndividual>
    


    <!-- http://gtfs.org/is_operator_0 -->


    <owl:NamedIndividual rdf:about="http://gtfs.org/is_operator_0">
        <rdf:type rdf:resource="http://gtfs.org/IsOperatorEnum"/>
        <gtfs:hasEnumValue>0</gtfs:hasEnumValue>
        <rdfs:comment>False</rdfs:comment>
        <rdfs:label>is_operator:0</rdfs:label>
    </owl:NamedIndividual>
    


    <!-- http://gtfs.org/is_operator_1 -->


    <owl:NamedIndividual rdf:about="http://gtfs.org/is_operator_1">
        <rdf:type rdf:resource="http://gtfs.org/IsOperatorEnum"/>
        <gtfs:hasEnumValue>1</gtfs:hasEnumValue>
        <rdfs:comment>True</rdfs:comment>
        <rdfs:label>is_operator:1</rdfs:label>
    </owl:NamedIndividual>
    


    <!-- http://gtfs.org/is_producer -->


    <owl:NamedIndividual rdf:about="http://gtfs.org/is_producer">
        <rdf:type rdf:resource="http://gtfs.org/Field"/>
        <gtfs:isFieldOf rdf:resource="http://gtfs.org/attributions.txt"/>
        <gtfs:isOptionalIn rdf:resource="http://gtfs.org/attributions.txt"/>
        <gtfs:isPresence rdf:resource="http://gtfs.org/Optional"/>
        <gtfs:isType rdf:resource="http://gtfs.org/IsProducerEnum"/>
        <gtfs:hasAdditionalInfo>Valid options are: 0 or empty - Organization doesn’t have this role. 1 - Organization does have this role.</gtfs:hasAdditionalInfo>
        <rdfs:comment>The role of the organization is producer. At least one of the fields is_producer, is_operator, or is_authority should be set at 1.</rdfs:comment>
        <rdfs:label>is_producer</rdfs:label>
    </owl:NamedIndividual>
    


    <!-- http://gtfs.org/is_producer_0 -->


    <owl:NamedIndividual rdf:about="http://gtfs.org/is_producer_0">
        <rdf:type rdf:resource="http://gtfs.org/IsProducerEnum"/>
        <gtfs:hasEnumValue>0</gtfs:hasEnumValue>
        <rdfs:comment>Organization doesn’t have this role</rdfs:comment>
        <rdfs:label>is_producer:0</rdfs:label>
    </owl:NamedIndividual>
    


    <!-- http://gtfs.org/is_producer_1 -->


    <owl:NamedIndividual rdf:about="http://gtfs.org/is_producer_1">
        <rdf:type rdf:resource="http://gtfs.org/IsProducerEnum"/>
        <gtfs:hasEnumValue>1</gtfs:hasEnumValue>
        <rdfs:comment>Organization does have this role</rdfs:comment>
        <rdfs:label>is_producer:1</rdfs:label>
    </owl:NamedIndividual>
    


    <!-- http://gtfs.org/language -->


    <owl:NamedIndividual rdf:about="http://gtfs.org/language">
        <rdf:type rdf:resource="http://gtfs.org/Field"/>
        <gtfs:isFieldOf rdf:resource="http://gtfs.org/translations.txt"/>
        <gtfs:isRequiredIn rdf:resource="http://gtfs.org/translations.txt"/>
        <gtfs:isType rdf:resource="http://gtfs.org/LanguageCode"/>
        <gtfs:hasAdditionalInfo>If the language is the same as in `feed_info.feed_lang`, the original value of the field will be assumed to be the default value to use in languages without specific translations (if `default_lang` doesn&apos;t specify otherwise).</gtfs:hasAdditionalInfo>
        <gtfs:isUniqueID rdf:resource="http://gtfs.org/translations.txt"/>
        <rdfs:comment>Language of translation.

If the language is the same as in `feed_info.feed_lang`, the original value of the field will be assumed to be the default value to use in languages without specific translations (if `default_lang` doesn&apos;t specify otherwise).

Example: In Switzerland, a city in an officially bilingual canton is officially called “Biel/Bienne”, but would simply be called “Bienne” in French and “Biel” in German.</rdfs:comment>
        <rdfs:label>language</rdfs:label>
    </owl:NamedIndividual>
    


    <!-- http://gtfs.org/leg_group_id -->


    <owl:NamedIndividual rdf:about="http://gtfs.org/leg_group_id">
        <rdf:type rdf:resource="http://gtfs.org/Field"/>
        <gtfs:isFieldOf rdf:resource="http://gtfs.org/fare_leg_rules.txt"/>
        <gtfs:isOptionalIn rdf:resource="http://gtfs.org/fare_leg_rules.txt"/>
        <gtfs:isType rdf:resource="http://gtfs.org/ID"/>
        <gtfs:hasAdditionalInfo>This field is an ID type that identifies a group of entries in fare_leg_rules.txt.</gtfs:hasAdditionalInfo>
        <rdfs:comment>Identifies a group of entries in fare_leg_rules.txt. Used to describe fare transfer rules between fare_transfer_rules.from_leg_group_id and fare_transfer_rules.to_leg_group_id. Multiple entries in fare_leg_rules.txt may belong to the same fare_leg_rules.leg_group_id. The same entry in fare_leg_rules.txt (not including fare_leg_rules.leg_group_id) must not belong to multiple fare_leg_rules.leg_group_id.</rdfs:comment>
        <rdfs:label>leg_group_id</rdfs:label>
    </owl:NamedIndividual>
    


    <!-- http://gtfs.org/length -->


    <owl:NamedIndividual rdf:about="http://gtfs.org/length">
        <rdf:type rdf:resource="http://gtfs.org/Field"/>
        <gtfs:isFieldOf rdf:resource="http://gtfs.org/pathways.txt"/>
        <gtfs:isOptionalIn rdf:resource="http://gtfs.org/pathways.txt"/>
        <gtfs:isType rdf:resource="http://gtfs.org/Float"/>
        <gtfs:hasAdditionalInfo>Non-negative float</gtfs:hasAdditionalInfo>
        <rdfs:comment>Horizontal length in meters of the pathway from the origin location (defined in `from_stop_id`) to the destination location (defined in `to_stop_id`). This field is recommended for walkways (`pathway_mode=1`), fare gates (`pathway_mode=6`) and exit gates (`pathway_mode=7`).</rdfs:comment>
        <rdfs:label>length</rdfs:label>
    </owl:NamedIndividual>
    


    <!-- http://gtfs.org/level_id -->


    <owl:NamedIndividual rdf:about="http://gtfs.org/level_id">
        <rdf:type rdf:resource="http://gtfs.org/Field"/>
        <gtfs:isFieldOf rdf:resource="http://gtfs.org/levels.txt"/>
        <gtfs:isFieldOf rdf:resource="http://gtfs.org/stops.txt"/>
        <gtfs:isOptionalIn rdf:resource="http://gtfs.org/stops.txt"/>
        <gtfs:isRequiredIn rdf:resource="http://gtfs.org/levels.txt"/>
        <gtfs:isType rdf:resource="http://gtfs.org/ID"/>
        <gtfs:hasAdditionalInfo>Foreign ID referencing `levels.level_id`</gtfs:hasAdditionalInfo>
        <gtfs:hasAdditionalInfo>Unique ID</gtfs:hasAdditionalInfo>
        <gtfs:isForeignID rdf:resource="http://gtfs.org/stops.txt"/>
        <gtfs:isUniqueID rdf:resource="http://gtfs.org/levels.txt"/>
        <rdfs:comment>Identifies a level in a station.</rdfs:comment>
        <rdfs:comment>Level of the location. The same level may be used by multiple unlinked stations.</rdfs:comment>
        <rdfs:label>level_id</rdfs:label>
    </owl:NamedIndividual>
    


    <!-- http://gtfs.org/level_index -->


    <owl:NamedIndividual rdf:about="http://gtfs.org/level_index">
        <rdf:type rdf:resource="http://gtfs.org/Field"/>
        <gtfs:isFieldOf rdf:resource="http://gtfs.org/levels.txt"/>
        <gtfs:isRequiredIn rdf:resource="http://gtfs.org/levels.txt"/>
        <gtfs:isType rdf:resource="http://gtfs.org/Float"/>
        <gtfs:hasAdditionalInfo>The level index is a float value.</gtfs:hasAdditionalInfo>
        <rdfs:comment>Numeric index of the level that indicates its relative position. Ground level should have index `0`, with levels above ground indicated by positive indices and levels below ground by negative indices.</rdfs:comment>
        <rdfs:label>level_index</rdfs:label>
    </owl:NamedIndividual>
    


    <!-- http://gtfs.org/level_name -->


    <owl:NamedIndividual rdf:about="http://gtfs.org/level_name">
        <rdf:type rdf:resource="http://gtfs.org/Field"/>
        <gtfs:isFieldOf rdf:resource="http://gtfs.org/levels.txt"/>
        <gtfs:isOptionalIn rdf:resource="http://gtfs.org/levels.txt"/>
        <gtfs:isType rdf:resource="http://gtfs.org/Text"/>
        <gtfs:hasAdditionalInfo>This field represents the name of the level within a building or station.</gtfs:hasAdditionalInfo>
        <gtfs:hasExample>Take the elevator to &quot;Mezzanine&quot; or &quot;Platform&quot; or &quot;-1&quot;.</gtfs:hasExample>
        <rdfs:comment>Name of the level as seen by the rider inside the building or station.</rdfs:comment>
        <rdfs:label>level_name</rdfs:label>
    </owl:NamedIndividual>
    


    <!-- http://gtfs.org/levels.txt -->


    <owl:NamedIndividual rdf:about="http://gtfs.org/levels.txt">
        <rdf:type rdf:resource="http://gtfs.org/File"/>
        <gtfs:hasField rdf:resource="http://gtfs.org/level_id"/>
        <gtfs:hasField rdf:resource="http://gtfs.org/level_index"/>
        <gtfs:hasField rdf:resource="http://gtfs.org/level_name"/>
        <gtfs:isConditionallyRequiredIn rdf:resource="http://gtfs.org/GTFS_Static"/>
        <gtfs:isFileOf rdf:resource="http://gtfs.org/GTFS_Static"/>
        <gtfs:hasCondition>- Required when describing pathways with elevators (pathway_mode=5). - Optional otherwise.</gtfs:hasCondition>
        <rdfs:comment>Levels within stations.</rdfs:comment>
        <rdfs:label>levels.txt</rdfs:label>
    </owl:NamedIndividual>
    


    <!-- http://gtfs.org/location_type -->


    <owl:NamedIndividual rdf:about="http://gtfs.org/location_type">
        <rdf:type rdf:resource="http://gtfs.org/Field"/>
        <gtfs:isFieldOf rdf:resource="http://gtfs.org/stops.txt"/>
        <gtfs:isOptionalIn rdf:resource="http://gtfs.org/stops.txt"/>
        <gtfs:isPresence rdf:resource="http://gtfs.org/Optional"/>
        <gtfs:isType rdf:resource="http://gtfs.org/LocationTypeEnum"/>
        <gtfs:hasAdditionalInfo>Valid options are: 0 (or blank) - Stop (or Platform), 1 - Station, 2 - Entrance/Exit, 3 - Generic Node, 4 - Boarding Area</gtfs:hasAdditionalInfo>
        <rdfs:comment>Location type. Valid options are: 0 (or blank) - Stop (or Platform). A location where passengers board or disembark from a transit vehicle. Is called a platform when defined within a parent_station. 1 - Station. A physical structure or area that contains one or more platform. 2 - Entrance/Exit. A location where passengers can enter or exit a station from the street. If an entrance/exit belongs to multiple stations, it may be linked by pathways to both, but the data provider must pick one of them as parent. 3 - Generic Node. A location within a station, not matching any other location_type, that may be used to link together pathways define in pathways.txt. 4 - Boarding Area. A specific location on a platform, where passengers can board and/or alight vehicles.</rdfs:comment>
        <rdfs:label>location_type</rdfs:label>
    </owl:NamedIndividual>
    


    <!-- http://gtfs.org/location_type_0 -->


    <owl:NamedIndividual rdf:about="http://gtfs.org/location_type_0">
        <rdf:type rdf:resource="http://gtfs.org/LocationTypeEnum"/>
        <gtfs:hasEnumValue>0</gtfs:hasEnumValue>
        <rdfs:comment>Stop (or Platform)</rdfs:comment>
        <rdfs:label>location_type:0</rdfs:label>
    </owl:NamedIndividual>
    


    <!-- http://gtfs.org/location_type_1 -->


    <owl:NamedIndividual rdf:about="http://gtfs.org/location_type_1">
        <rdf:type rdf:resource="http://gtfs.org/LocationTypeEnum"/>
        <gtfs:hasEnumValue>1</gtfs:hasEnumValue>
        <rdfs:comment>Station</rdfs:comment>
        <rdfs:label>location_type:1</rdfs:label>
    </owl:NamedIndividual>
    


    <!-- http://gtfs.org/location_type_2 -->


    <owl:NamedIndividual rdf:about="http://gtfs.org/location_type_2">
        <rdf:type rdf:resource="http://gtfs.org/LocationTypeEnum"/>
        <gtfs:hasEnumValue>2</gtfs:hasEnumValue>
        <rdfs:comment>Entrance/Exit</rdfs:comment>
        <rdfs:label>location_type:2</rdfs:label>
    </owl:NamedIndividual>
    


    <!-- http://gtfs.org/location_type_3 -->


    <owl:NamedIndividual rdf:about="http://gtfs.org/location_type_3">
        <rdf:type rdf:resource="http://gtfs.org/LocationTypeEnum"/>
        <gtfs:hasEnumValue>3</gtfs:hasEnumValue>
        <rdfs:comment>Generic Node</rdfs:comment>
        <rdfs:label>location_type:3</rdfs:label>
    </owl:NamedIndividual>
    


    <!-- http://gtfs.org/location_type_4 -->


    <owl:NamedIndividual rdf:about="http://gtfs.org/location_type_4">
        <rdf:type rdf:resource="http://gtfs.org/LocationTypeEnum"/>
        <gtfs:hasEnumValue>4</gtfs:hasEnumValue>
        <rdfs:comment>Boarding Area</rdfs:comment>
        <rdfs:label>location_type:4</rdfs:label>
    </owl:NamedIndividual>
    


    <!-- http://gtfs.org/max_slope -->


    <owl:NamedIndividual rdf:about="http://gtfs.org/max_slope">
        <rdf:type rdf:resource="http://gtfs.org/Field"/>
        <gtfs:isFieldOf rdf:resource="http://gtfs.org/pathways.txt"/>
        <gtfs:isOptionalIn rdf:resource="http://gtfs.org/pathways.txt"/>
        <gtfs:isType rdf:resource="http://gtfs.org/Float"/>
        <gtfs:hasAdditionalInfo>Valid options are: 0 or empty - No slope. Float - Slope ratio of the pathway, positive for upwards, negative for downwards. This field should only be used with walkways (pathway_mode=1) and moving sidewalks (pathway_mode=3). Example: In the US, 0.083 (also written 8.3%) is the maximum slope ratio for hand-propelled wheelchair, which means an increase of 0.083m (so 8.3cm) for each 1m.</gtfs:hasAdditionalInfo>
        <rdfs:comment>Maximum slope ratio of the pathway. Valid options are: 0 or empty - No slope. Float - Slope ratio of the pathway, positive for upwards, negative for downwards. This field should only be used with walkways (pathway_mode=1) and moving sidewalks (pathway_mode=3). Example: In the US, 0.083 (also written 8.3%) is the maximum slope ratio for hand-propelled wheelchair, which means an increase of 0.083m (so 8.3cm) for each 1m.</rdfs:comment>
        <rdfs:label>max_slope</rdfs:label>
    </owl:NamedIndividual>
    


    <!-- http://gtfs.org/min_transfer_time -->


    <owl:NamedIndividual rdf:about="http://gtfs.org/min_transfer_time">
        <rdf:type rdf:resource="http://gtfs.org/Field"/>
        <gtfs:isFieldOf rdf:resource="http://gtfs.org/transfers.txt"/>
        <gtfs:isOptionalIn rdf:resource="http://gtfs.org/transfers.txt"/>
        <gtfs:isType rdf:resource="http://gtfs.org/Integer"/>
        <gtfs:hasAdditionalInfo>Non-negative integer</gtfs:hasAdditionalInfo>
        <rdfs:comment>Amount of time, in seconds, that must be available to permit a transfer between routes at the specified stops. The `min_transfer_time` should be sufficient to permit a typical rider to move between the two stops, including buffer time to allow for schedule variance on each route.</rdfs:comment>
        <rdfs:label>min_transfer_time</rdfs:label>
    </owl:NamedIndividual>
    


    <!-- http://gtfs.org/min_width -->


    <owl:NamedIndividual rdf:about="http://gtfs.org/min_width">
        <rdf:type rdf:resource="http://gtfs.org/Field"/>
        <gtfs:isFieldOf rdf:resource="http://gtfs.org/pathways.txt"/>
        <gtfs:isOptionalIn rdf:resource="http://gtfs.org/pathways.txt"/>
        <gtfs:isType rdf:resource="http://gtfs.org/Float"/>
        <gtfs:hasAdditionalInfo>This field is recommended if the minimum width is less than 1 meter.</gtfs:hasAdditionalInfo>
        <rdfs:comment>Minimum width of the pathway in meters.</rdfs:comment>
        <rdfs:label>min_width</rdfs:label>
    </owl:NamedIndividual>
    


    <!-- http://gtfs.org/monday -->


    <owl:NamedIndividual rdf:about="http://gtfs.org/monday">
        <rdf:type rdf:resource="http://gtfs.org/Field"/>
        <gtfs:isFieldOf rdf:resource="http://gtfs.org/calendar.txt"/>
        <gtfs:isPresence rdf:resource="http://gtfs.org/Required"/>
        <gtfs:isRequiredIn rdf:resource="http://gtfs.org/calendar.txt"/>
        <gtfs:isType rdf:resource="http://gtfs.org/MondayEnum"/>
        <gtfs:hasAdditionalInfo>Valid options are: 1 - Service is available for all Mondays in the date range. 0 - Service is not available for Mondays in the date range.</gtfs:hasAdditionalInfo>
        <rdfs:comment>Indicates whether the service operates on all Mondays in the date range specified by the `start_date` and `end_date` fields. Note that exceptions for particular dates may be listed in [calendar_dates.txt](#calendar_datestxt). Valid options are: 1 - Service is available for all Mondays in the date range. 0 - Service is not available for Mondays in the date range.</rdfs:comment>
        <rdfs:label>monday</rdfs:label>
    </owl:NamedIndividual>
    


    <!-- http://gtfs.org/monday_0 -->


    <owl:NamedIndividual rdf:about="http://gtfs.org/monday_0">
        <rdf:type rdf:resource="http://gtfs.org/MondayEnum"/>
        <gtfs:hasEnumValue>0</gtfs:hasEnumValue>
        <rdfs:comment>Service is not available for Mondays in the date range</rdfs:comment>
        <rdfs:label>monday:0</rdfs:label>
    </owl:NamedIndividual>
    


    <!-- http://gtfs.org/monday_1 -->


    <owl:NamedIndividual rdf:about="http://gtfs.org/monday_1">
        <rdf:type rdf:resource="http://gtfs.org/MondayEnum"/>
        <gtfs:hasEnumValue>1</gtfs:hasEnumValue>
        <rdfs:comment>Service is available for all Mondays in the date range</rdfs:comment>
        <rdfs:label>monday:1</rdfs:label>
    </owl:NamedIndividual>
    


    <!-- http://gtfs.org/network_id -->


    <owl:NamedIndividual rdf:about="http://gtfs.org/network_id">
        <rdf:type rdf:resource="http://gtfs.org/Field"/>
        <gtfs:isFieldOf rdf:resource="http://gtfs.org/fare_leg_rules.txt"/>
        <gtfs:isFieldOf rdf:resource="http://gtfs.org/routes.txt"/>
        <gtfs:isOptionalIn rdf:resource="http://gtfs.org/fare_leg_rules.txt"/>
        <gtfs:isOptionalIn rdf:resource="http://gtfs.org/routes.txt"/>
        <gtfs:isType rdf:resource="http://gtfs.org/ID"/>
        <gtfs:hasAdditionalInfo>Foreign ID referencing routes.network_id</gtfs:hasAdditionalInfo>
        <gtfs:hasAdditionalInfo>This field is an ID type that is used to group routes together.</gtfs:hasAdditionalInfo>
        <gtfs:isForeignID rdf:resource="http://gtfs.org/fare_leg_rules.txt"/>
        <rdfs:comment>Identifies a group of routes. Multiple rows in routes.txt may have the same network_id.</rdfs:comment>
        <rdfs:comment>Identifies a route network that applies for the fare leg rule. If there are no matching fare_leg_rules.network_id values to the network_id being filtered, empty fare_leg_rules.network_id will be matched by default. An empty entry in fare_leg_rules.network_id corresponds to all networks defined in routes.txt excluding the ones listed under fare_leg_rules.network_id</rdfs:comment>
        <rdfs:label>network_id</rdfs:label>
    </owl:NamedIndividual>
    


    <!-- http://gtfs.org/organization_name -->


    <owl:NamedIndividual rdf:about="http://gtfs.org/organization_name">
        <rdf:type rdf:resource="http://gtfs.org/Field"/>
        <gtfs:isFieldOf rdf:resource="http://gtfs.org/attributions.txt"/>
        <gtfs:isRequiredIn rdf:resource="http://gtfs.org/attributions.txt"/>
        <gtfs:isType rdf:resource="http://gtfs.org/Text"/>
        <gtfs:hasAdditionalInfo>This field stores the name of the organization associated with the dataset.</gtfs:hasAdditionalInfo>
        <rdfs:comment>Name of the organization that the dataset is attributed to.</rdfs:comment>
        <rdfs:label>organization_name</rdfs:label>
    </owl:NamedIndividual>
    


    <!-- http://gtfs.org/origin_id -->


    <owl:NamedIndividual rdf:about="http://gtfs.org/origin_id">
        <rdf:type rdf:resource="http://gtfs.org/Field"/>
        <gtfs:isFieldOf rdf:resource="http://gtfs.org/fare_rules.txt"/>
        <gtfs:isOptionalIn rdf:resource="http://gtfs.org/fare_rules.txt"/>
        <gtfs:isType rdf:resource="http://gtfs.org/ID"/>
        <gtfs:hasAdditionalInfo>Foreign ID referencing stops.zone_id</gtfs:hasAdditionalInfo>
        <gtfs:isForeignID rdf:resource="http://gtfs.org/fare_rules.txt"/>
        <rdfs:comment>Identifies an origin zone. If a fare class has multiple origin zones, create a record in fare_rules.txt for each origin_id.</rdfs:comment>
        <rdfs:label>origin_id</rdfs:label>
    </owl:NamedIndividual>
    


    <!-- http://gtfs.org/parent_station -->


    <owl:NamedIndividual rdf:about="http://gtfs.org/parent_station">
        <rdf:type rdf:resource="http://gtfs.org/Field"/>
        <gtfs:isConditionallyRequiredIn rdf:resource="http://gtfs.org/stops.txt"/>
        <gtfs:isFieldOf rdf:resource="http://gtfs.org/stops.txt"/>
        <gtfs:isType rdf:resource="http://gtfs.org/ID"/>
        <gtfs:hasAdditionalInfo>Foreign ID referencing stops.stop_id</gtfs:hasAdditionalInfo>
        <gtfs:hasCondition>Required for locations which are entrances (location_type=2), generic nodes (location_type=3) or boarding areas (location_type=4). Optional for stops/platforms (location_type=0). Forbidden for stations (location_type=1).</gtfs:hasCondition>
        <gtfs:isForeignID rdf:resource="http://gtfs.org/stops.txt"/>
        <rdfs:comment>Defines hierarchy between the different locations defined in stops.txt. It contains the ID of the parent location.</rdfs:comment>
        <rdfs:label>parent_station</rdfs:label>
    </owl:NamedIndividual>
    


    <!-- http://gtfs.org/pathway_id -->


    <owl:NamedIndividual rdf:about="http://gtfs.org/pathway_id">
        <rdf:type rdf:resource="http://gtfs.org/Field"/>
        <gtfs:isFieldOf rdf:resource="http://gtfs.org/pathways.txt"/>
        <gtfs:isRequiredIn rdf:resource="http://gtfs.org/pathways.txt"/>
        <gtfs:isType rdf:resource="http://gtfs.org/ID"/>
        <gtfs:hasAdditionalInfo>Unique ID</gtfs:hasAdditionalInfo>
        <gtfs:isUniqueID rdf:resource="http://gtfs.org/pathways.txt"/>
        <rdfs:comment>Identifies a pathway. Used by systems as an internal identifier for the record. Must be unique in the dataset. Different pathways may have the same values for `from_stop_id` and `to_stop_id`. Example: When two escalators are side-by-side in opposite directions, or when a stair set and elevator go from the same place to the same place, different `pathway_id` may have the same `from_stop_id` and `to_stop_id` values.</rdfs:comment>
        <rdfs:label>pathway_id</rdfs:label>
    </owl:NamedIndividual>
    


    <!-- http://gtfs.org/pathway_mode -->


    <owl:NamedIndividual rdf:about="http://gtfs.org/pathway_mode">
        <rdf:type rdf:resource="http://gtfs.org/Field"/>
        <gtfs:isFieldOf rdf:resource="http://gtfs.org/pathways.txt"/>
        <gtfs:isPresence rdf:resource="http://gtfs.org/Required"/>
        <gtfs:isRequiredIn rdf:resource="http://gtfs.org/pathways.txt"/>
        <gtfs:isType rdf:resource="http://gtfs.org/PathwayModeEnum"/>
        <gtfs:hasAdditionalInfo>Valid options are: 1 - Walkway, 2 - Stairs, 3 - Moving sidewalk/travelator, 4 - Escalator, 5 - Elevator, 6 - Fare gate, 7 - Exit gate</gtfs:hasAdditionalInfo>
        <rdfs:comment>Type of pathway between the specified (from_stop_id, to_stop_id) pair. Valid options are: 1 - Walkway. 2 - Stairs. 3 - Moving sidewalk/travelator. 4 - Escalator. 5 - Elevator. 6 - Fare gate (or payment gate): A pathway that crosses into an area of the station where proof of payment is required to cross. Fare gates may separate paid areas of the station from unpaid ones, or separate different payment areas within the same station from each other. This information can be used to avoid routing passengers through stations using shortcuts that would require passengers to make unnecessary payments, like directing a passenger to walk through a subway platform to reach a busway. 7- Exit gate: A pathway exiting a paid area into an unpaid area where proof of payment is not required to cross.</rdfs:comment>
        <rdfs:label>pathway_mode</rdfs:label>
    </owl:NamedIndividual>
    


    <!-- http://gtfs.org/pathway_mode_1 -->


    <owl:NamedIndividual rdf:about="http://gtfs.org/pathway_mode_1">
        <rdf:type rdf:resource="http://gtfs.org/PathwayModeEnum"/>
        <gtfs:hasEnumValue>1</gtfs:hasEnumValue>
        <rdfs:comment>Walkway</rdfs:comment>
        <rdfs:label>pathway_mode:1</rdfs:label>
    </owl:NamedIndividual>
    


    <!-- http://gtfs.org/pathway_mode_2 -->


    <owl:NamedIndividual rdf:about="http://gtfs.org/pathway_mode_2">
        <rdf:type rdf:resource="http://gtfs.org/PathwayModeEnum"/>
        <gtfs:hasEnumValue>2</gtfs:hasEnumValue>
        <rdfs:comment>Stairs</rdfs:comment>
        <rdfs:label>pathway_mode:2</rdfs:label>
    </owl:NamedIndividual>
    


    <!-- http://gtfs.org/pathway_mode_3 -->


    <owl:NamedIndividual rdf:about="http://gtfs.org/pathway_mode_3">
        <rdf:type rdf:resource="http://gtfs.org/PathwayModeEnum"/>
        <gtfs:hasEnumValue>3</gtfs:hasEnumValue>
        <rdfs:comment>Moving sidewalk/travelator</rdfs:comment>
        <rdfs:label>pathway_mode:3</rdfs:label>
    </owl:NamedIndividual>
    


    <!-- http://gtfs.org/pathway_mode_4 -->


    <owl:NamedIndividual rdf:about="http://gtfs.org/pathway_mode_4">
        <rdf:type rdf:resource="http://gtfs.org/PathwayModeEnum"/>
        <gtfs:hasEnumValue>4</gtfs:hasEnumValue>
        <rdfs:comment>Escalator</rdfs:comment>
        <rdfs:label>pathway_mode:4</rdfs:label>
    </owl:NamedIndividual>
    


    <!-- http://gtfs.org/pathway_mode_5 -->


    <owl:NamedIndividual rdf:about="http://gtfs.org/pathway_mode_5">
        <rdf:type rdf:resource="http://gtfs.org/PathwayModeEnum"/>
        <gtfs:hasEnumValue>5</gtfs:hasEnumValue>
        <rdfs:comment>Elevator</rdfs:comment>
        <rdfs:label>pathway_mode:5</rdfs:label>
    </owl:NamedIndividual>
    


    <!-- http://gtfs.org/pathway_mode_6 -->


    <owl:NamedIndividual rdf:about="http://gtfs.org/pathway_mode_6">
        <rdf:type rdf:resource="http://gtfs.org/PathwayModeEnum"/>
        <gtfs:hasEnumValue>6</gtfs:hasEnumValue>
        <rdfs:comment>Fare gate</rdfs:comment>
        <rdfs:label>pathway_mode:6</rdfs:label>
    </owl:NamedIndividual>
    


    <!-- http://gtfs.org/pathway_mode_7 -->


    <owl:NamedIndividual rdf:about="http://gtfs.org/pathway_mode_7">
        <rdf:type rdf:resource="http://gtfs.org/PathwayModeEnum"/>
        <gtfs:hasEnumValue>7</gtfs:hasEnumValue>
        <rdfs:comment>Exit gate</rdfs:comment>
        <rdfs:label>pathway_mode:7</rdfs:label>
    </owl:NamedIndividual>
    


    <!-- http://gtfs.org/pathways.txt -->


    <owl:NamedIndividual rdf:about="http://gtfs.org/pathways.txt">
        <rdf:type rdf:resource="http://gtfs.org/File"/>
        <gtfs:hasField rdf:resource="http://gtfs.org/from_stop_id"/>
        <gtfs:hasField rdf:resource="http://gtfs.org/is_bidirectional"/>
        <gtfs:hasField rdf:resource="http://gtfs.org/length"/>
        <gtfs:hasField rdf:resource="http://gtfs.org/max_slope"/>
        <gtfs:hasField rdf:resource="http://gtfs.org/min_width"/>
        <gtfs:hasField rdf:resource="http://gtfs.org/pathway_id"/>
        <gtfs:hasField rdf:resource="http://gtfs.org/pathway_mode"/>
        <gtfs:hasField rdf:resource="http://gtfs.org/reversed_signposted_as"/>
        <gtfs:hasField rdf:resource="http://gtfs.org/signposted_as"/>
        <gtfs:hasField rdf:resource="http://gtfs.org/stair_count"/>
        <gtfs:hasField rdf:resource="http://gtfs.org/to_stop_id"/>
        <gtfs:hasField rdf:resource="http://gtfs.org/traversal_time"/>
        <gtfs:isFileOf rdf:resource="http://gtfs.org/GTFS_Static"/>
        <gtfs:isOptionalIn rdf:resource="http://gtfs.org/GTFS_Static"/>
        <rdfs:comment>Pathways linking together locations within stations.</rdfs:comment>
        <rdfs:label>pathways.txt</rdfs:label>
    </owl:NamedIndividual>
    


    <!-- http://gtfs.org/payment_method -->


    <owl:NamedIndividual rdf:about="http://gtfs.org/payment_method">
        <rdf:type rdf:resource="http://gtfs.org/Field"/>
        <gtfs:isFieldOf rdf:resource="http://gtfs.org/fare_attributes.txt"/>
        <gtfs:isPresence rdf:resource="http://gtfs.org/Required"/>
        <gtfs:isRequiredIn rdf:resource="http://gtfs.org/fare_attributes.txt"/>
        <gtfs:isType rdf:resource="http://gtfs.org/PaymentMethodEnum"/>
        <gtfs:hasAdditionalInfo>Valid options are: 0 - Fare is paid on board. 1 - Fare must be paid before boarding.</gtfs:hasAdditionalInfo>
        <rdfs:comment>Indicates when the fare must be paid. Valid options are: 0 - Fare is paid on board. 1 - Fare must be paid before boarding.</rdfs:comment>
        <rdfs:label>payment_method</rdfs:label>
    </owl:NamedIndividual>
    


    <!-- http://gtfs.org/payment_method_0 -->


    <owl:NamedIndividual rdf:about="http://gtfs.org/payment_method_0">
        <rdf:type rdf:resource="http://gtfs.org/PaymentMethodEnum"/>
        <gtfs:hasEnumValue>0</gtfs:hasEnumValue>
        <rdfs:comment>Fare is paid on board</rdfs:comment>
        <rdfs:label>payment_method:0</rdfs:label>
    </owl:NamedIndividual>
    


    <!-- http://gtfs.org/payment_method_1 -->


    <owl:NamedIndividual rdf:about="http://gtfs.org/payment_method_1">
        <rdf:type rdf:resource="http://gtfs.org/PaymentMethodEnum"/>
        <gtfs:hasEnumValue>1</gtfs:hasEnumValue>
        <rdfs:comment>Fare must be paid before boarding</rdfs:comment>
        <rdfs:label>payment_method:1</rdfs:label>
    </owl:NamedIndividual>
    


    <!-- http://gtfs.org/pickup_type -->


    <owl:NamedIndividual rdf:about="http://gtfs.org/pickup_type">
        <rdf:type rdf:resource="http://gtfs.org/Field"/>
        <gtfs:isFieldOf rdf:resource="http://gtfs.org/stop_times.txt"/>
        <gtfs:isOptionalIn rdf:resource="http://gtfs.org/stop_times.txt"/>
        <gtfs:isPresence rdf:resource="http://gtfs.org/Optional"/>
        <gtfs:isType rdf:resource="http://gtfs.org/PickupTypeEnum"/>
        <gtfs:hasAdditionalInfo>Enum field with options 0, 1, 2, 3</gtfs:hasAdditionalInfo>
        <rdfs:comment>Indicates pickup method. Valid options are: 0 or empty - Regularly scheduled pickup. 1 - No pickup available. 2 - Must phone agency to arrange pickup. 3 - Must coordinate with driver to arrange pickup.</rdfs:comment>
        <rdfs:label>pickup_type</rdfs:label>
    </owl:NamedIndividual>
    


    <!-- http://gtfs.org/pickup_type_0 -->


    <owl:NamedIndividual rdf:about="http://gtfs.org/pickup_type_0">
        <rdf:type rdf:resource="http://gtfs.org/PickupTypeEnum"/>
        <gtfs:hasEnumValue>0</gtfs:hasEnumValue>
        <rdfs:comment>Regularly scheduled pickup</rdfs:comment>
        <rdfs:label>pickup_type:0</rdfs:label>
    </owl:NamedIndividual>
    


    <!-- http://gtfs.org/pickup_type_1 -->


    <owl:NamedIndividual rdf:about="http://gtfs.org/pickup_type_1">
        <rdf:type rdf:resource="http://gtfs.org/PickupTypeEnum"/>
        <gtfs:hasEnumValue>1</gtfs:hasEnumValue>
        <rdfs:comment>No pickup available</rdfs:comment>
        <rdfs:label>pickup_type:1</rdfs:label>
    </owl:NamedIndividual>
    


    <!-- http://gtfs.org/pickup_type_2 -->


    <owl:NamedIndividual rdf:about="http://gtfs.org/pickup_type_2">
        <rdf:type rdf:resource="http://gtfs.org/PickupTypeEnum"/>
        <gtfs:hasEnumValue>2</gtfs:hasEnumValue>
        <rdfs:comment>Must phone agency to arrange pickup</rdfs:comment>
        <rdfs:label>pickup_type:2</rdfs:label>
    </owl:NamedIndividual>
    


    <!-- http://gtfs.org/pickup_type_3 -->


    <owl:NamedIndividual rdf:about="http://gtfs.org/pickup_type_3">
        <rdf:type rdf:resource="http://gtfs.org/PickupTypeEnum"/>
        <gtfs:hasEnumValue>3</gtfs:hasEnumValue>
        <rdfs:comment>Must coordinate with driver to arrange pickup</rdfs:comment>
        <rdfs:label>pickup_type:3</rdfs:label>
    </owl:NamedIndividual>
    


    <!-- http://gtfs.org/platform_code -->


    <owl:NamedIndividual rdf:about="http://gtfs.org/platform_code">
        <rdf:type rdf:resource="http://gtfs.org/Field"/>
        <gtfs:isFieldOf rdf:resource="http://gtfs.org/stops.txt"/>
        <gtfs:isOptionalIn rdf:resource="http://gtfs.org/stops.txt"/>
        <gtfs:isType rdf:resource="http://gtfs.org/Text"/>
        <gtfs:hasAdditionalInfo>Platform identifier should be a text value without including words like “platform” or &quot;track&quot;</gtfs:hasAdditionalInfo>
        <rdfs:comment>Platform identifier for a platform stop (a stop belonging to a station). This should be just the platform identifier (eg. &quot;G&quot; or &quot;3&quot;). Words like “platform” or &quot;track&quot; (or the feed’s language-specific equivalent) should not be included. This allows feed consumers to more easily internationalize and localize the platform identifier into other languages.</rdfs:comment>
        <rdfs:label>platform_code</rdfs:label>
    </owl:NamedIndividual>
    


    <!-- http://gtfs.org/price -->


    <owl:NamedIndividual rdf:about="http://gtfs.org/price">
        <rdf:type rdf:resource="http://gtfs.org/Field"/>
        <gtfs:isFieldOf rdf:resource="http://gtfs.org/fare_attributes.txt"/>
        <gtfs:isRequiredIn rdf:resource="http://gtfs.org/fare_attributes.txt"/>
        <gtfs:isType rdf:resource="http://gtfs.org/Float"/>
        <gtfs:hasAdditionalInfo>Non-negative float</gtfs:hasAdditionalInfo>
        <rdfs:comment>Fare price, in the unit specified by currency_type.</rdfs:comment>
        <rdfs:label>price</rdfs:label>
    </owl:NamedIndividual>
    


    <!-- http://gtfs.org/record_id -->


    <owl:NamedIndividual rdf:about="http://gtfs.org/record_id">
        <rdf:type rdf:resource="http://gtfs.org/Field"/>
        <gtfs:isConditionallyRequiredIn rdf:resource="http://gtfs.org/translations.txt"/>
        <gtfs:isFieldOf rdf:resource="http://gtfs.org/translations.txt"/>
        <gtfs:isType rdf:resource="http://gtfs.org/ID"/>
        <gtfs:hasAdditionalInfo>Foreign ID</gtfs:hasAdditionalInfo>
        <gtfs:hasCondition>Forbidden if `table_name` is `feed_info`. Forbidden if `field_value` is defined. Required if `field_value` is empty.</gtfs:hasCondition>
        <gtfs:isForeignID rdf:resource="http://gtfs.org/translations.txt"/>
        <rdfs:comment>Defines the record that corresponds to the field to be translated. The value in `record_id` must be the first or only field of a table&apos;s primary key, as defined in the primary key attribute for each table and below:

- `agency_id` for `agency.txt`
- `stop_id` for `stops.txt`
- `route_id` for `routes.txt`
- `trip_id` for `trips.txt`
- `trip_id` for `stop_times.txt`
- `pathway_id` for `pathways.txt`
- `level_id` for `levels.txt`
- `attribution_id` for `attribution.txt`

Fields in tables not defined above should not be translated. However producers sometimes add extra fields that are outside the official specification and these unofficial fields may be translated. Below is the recommended way to use `record_id` for those tables:

- `service_id` for `calendar.txt`
- `service_id` for `calendar_dates.txt`
- `fare_id` for `fare_attributes.txt`
- `fare_id` for `fare_rules.txt`
- `shape_id` for `shapes.txt`
- `trip_id` for `frequencies.txt`
- `from_stop_id` for `transfers.txt`</rdfs:comment>
        <rdfs:label>record_id</rdfs:label>
    </owl:NamedIndividual>
    


    <!-- http://gtfs.org/record_sub_id -->


    <owl:NamedIndividual rdf:about="http://gtfs.org/record_sub_id">
        <rdf:type rdf:resource="http://gtfs.org/Field"/>
        <gtfs:isConditionallyRequiredIn rdf:resource="http://gtfs.org/translations.txt"/>
        <gtfs:isFieldOf rdf:resource="http://gtfs.org/translations.txt"/>
        <gtfs:isType rdf:resource="http://gtfs.org/ID"/>
        <gtfs:hasCondition>Forbidden if `table_name` is `feed_info` or if `field_value` is defined. Required if `table_name=stop_times` and `record_id` is defined.</gtfs:hasCondition>
        <gtfs:isForeignID rdf:resource="http://gtfs.org/translations.txt"/>
        <rdfs:comment>Helps the record that contains the field to be translated when the table doesn’t have a unique ID. Therefore, the value in `record_sub_id` is the secondary ID of the table, as defined by the table below:

- None for `agency.txt`;
- None for `stops.txt`;
- None for `routes.txt`;
- None for `trips.txt`;
- `stop_sequence` for `stop_times.txt`;
- None for `pathways.txt`;
- None for `levels.txt`;
- None for `attributions.txt`.

Fields in tables not defined above should not be translated. However producers sometimes add extra fields that are outside the official specification and these unofficial fields may be translated. Below is the recommended way to use `record_sub_id` for those tables:

- None for `calendar.txt`;
- `date` for `calendar_dates.txt`;
- None for `fare_attributes.txt`;
- `route_id` for `fare_rules.txt`;
- None for `shapes.txt`;
- `start_time` for `frequencies.txt`;
- `to_stop_id` for `transfers.txt`.

Conditionally Required:
- **Forbidden** if `table_name` is `feed_info`.
- **Forbidden** if `field_value` is defined.
- **Required** if `table_name=stop_times` and `record_id` is defined.</rdfs:comment>
        <rdfs:label>record_sub_id</rdfs:label>
    </owl:NamedIndividual>
    


    <!-- http://gtfs.org/reversed_signposted_as -->


    <owl:NamedIndividual rdf:about="http://gtfs.org/reversed_signposted_as">
        <rdf:type rdf:resource="http://gtfs.org/Field"/>
        <gtfs:isFieldOf rdf:resource="http://gtfs.org/pathways.txt"/>
        <gtfs:isOptionalIn rdf:resource="http://gtfs.org/pathways.txt"/>
        <gtfs:isType rdf:resource="http://gtfs.org/Text"/>
        <gtfs:hasAdditionalInfo>Text field to store the reversed signposted information.</gtfs:hasAdditionalInfo>
        <rdfs:comment>Same as `signposted_as`, but when the pathway is used from the `to_stop_id` to the `from_stop_id`.</rdfs:comment>
        <rdfs:label>reversed_signposted_as</rdfs:label>
    </owl:NamedIndividual>
    


    <!-- http://gtfs.org/route_color -->


    <owl:NamedIndividual rdf:about="http://gtfs.org/route_color">
        <rdf:type rdf:resource="http://gtfs.org/Field"/>
        <gtfs:isFieldOf rdf:resource="http://gtfs.org/routes.txt"/>
        <gtfs:isOptionalIn rdf:resource="http://gtfs.org/routes.txt"/>
        <gtfs:isType rdf:resource="http://gtfs.org/Color"/>
        <gtfs:hasAdditionalInfo>The color difference between `route_color` and `route_text_color` should provide sufficient contrast when viewed on a black and white screen.</gtfs:hasAdditionalInfo>
        <rdfs:comment>Route color designation that matches public facing material. Defaults to white (`FFFFFF`) when omitted or left empty. The color difference between `route_color` and `route_text_color` should provide sufficient contrast when viewed on a black and white screen.</rdfs:comment>
        <rdfs:label>route_color</rdfs:label>
    </owl:NamedIndividual>
    


    <!-- http://gtfs.org/route_desc -->


    <owl:NamedIndividual rdf:about="http://gtfs.org/route_desc">
        <rdf:type rdf:resource="http://gtfs.org/Field"/>
        <gtfs:isFieldOf rdf:resource="http://gtfs.org/routes.txt"/>
        <gtfs:isOptionalIn rdf:resource="http://gtfs.org/routes.txt"/>
        <gtfs:isType rdf:resource="http://gtfs.org/Text"/>
        <gtfs:hasAdditionalInfo>This field should contain detailed information about the route.</gtfs:hasAdditionalInfo>
        <gtfs:hasExample>&quot;A&quot; trains operate between Inwood-207 St, Manhattan and Far Rockaway-Mott Avenue, Queens at all times. Also from about 6AM until about midnight, additional &quot;A&quot; trains operate between Inwood-207 St and Lefferts Boulevard (trains typically alternate between Lefferts Blvd and Far Rockaway).</gtfs:hasExample>
        <rdfs:comment>Description of a route that provides useful, quality information. Should not be a duplicate of `route_short_name` or `route_long_name`.</rdfs:comment>
        <rdfs:label>route_desc</rdfs:label>
    </owl:NamedIndividual>
    


    <!-- http://gtfs.org/route_id -->


    <owl:NamedIndividual rdf:about="http://gtfs.org/route_id">
        <rdf:type rdf:resource="http://gtfs.org/Field"/>
        <gtfs:isFieldOf rdf:resource="http://gtfs.org/attributions.txt"/>
        <gtfs:isFieldOf rdf:resource="http://gtfs.org/fare_rules.txt"/>
        <gtfs:isFieldOf rdf:resource="http://gtfs.org/routes.txt"/>
        <gtfs:isFieldOf rdf:resource="http://gtfs.org/trips.txt"/>
        <gtfs:isOptionalIn rdf:resource="http://gtfs.org/attributions.txt"/>
        <gtfs:isOptionalIn rdf:resource="http://gtfs.org/fare_rules.txt"/>
        <gtfs:isRequiredIn rdf:resource="http://gtfs.org/routes.txt"/>
        <gtfs:isRequiredIn rdf:resource="http://gtfs.org/trips.txt"/>
        <gtfs:isType rdf:resource="http://gtfs.org/ID"/>
        <gtfs:hasAdditionalInfo>Foreign ID referencing `routes.route_id`</gtfs:hasAdditionalInfo>
        <gtfs:hasAdditionalInfo>Foreign ID referencing routes.route_id</gtfs:hasAdditionalInfo>
        <gtfs:hasAdditionalInfo>Unique ID</gtfs:hasAdditionalInfo>
        <gtfs:hasExample>If fare class &quot;b&quot; is valid on route &quot;TSW&quot; and &quot;TSE&quot;, the fare_rules.txt file would contain these records for the fare class: fare_id,route_id b,TSW b,TSE</gtfs:hasExample>
        <gtfs:isForeignID rdf:resource="http://gtfs.org/attributions.txt"/>
        <gtfs:isForeignID rdf:resource="http://gtfs.org/fare_rules.txt"/>
        <gtfs:isForeignID rdf:resource="http://gtfs.org/trips.txt"/>
        <gtfs:isUniqueID rdf:resource="http://gtfs.org/routes.txt"/>
        <rdfs:comment>Functions in the same way as `agency_id` except the attribution applies to a route. Multiple attributions may apply to the same route.</rdfs:comment>
        <rdfs:comment>Identifies a route associated with the fare class. If several routes with the same fare attributes exist, create a record in fare_rules.txt for each route.</rdfs:comment>
        <rdfs:comment>Identifies a route.</rdfs:comment>
        <rdfs:label>route_id</rdfs:label>
    </owl:NamedIndividual>
    


    <!-- http://gtfs.org/route_long_name -->


    <owl:NamedIndividual rdf:about="http://gtfs.org/route_long_name">
        <rdf:type rdf:resource="http://gtfs.org/Field"/>
        <gtfs:isConditionallyRequiredIn rdf:resource="http://gtfs.org/routes.txt"/>
        <gtfs:isFieldOf rdf:resource="http://gtfs.org/routes.txt"/>
        <gtfs:isType rdf:resource="http://gtfs.org/Text"/>
        <gtfs:hasAdditionalInfo>The name is generally more descriptive than the route_short_name and often includes the route&apos;s destination or stop.</gtfs:hasAdditionalInfo>
        <gtfs:hasCondition>Required if routes.route_short_name is empty. Optional otherwise.</gtfs:hasCondition>
        <rdfs:comment>Full name of a route. This name is generally more descriptive than the route_short_name and often includes the route&apos;s destination or stop. Both route_short_name and route_long_name may be defined.</rdfs:comment>
        <rdfs:label>route_long_name</rdfs:label>
    </owl:NamedIndividual>
    


    <!-- http://gtfs.org/route_short_name -->


    <owl:NamedIndividual rdf:about="http://gtfs.org/route_short_name">
        <rdf:type rdf:resource="http://gtfs.org/Field"/>
        <gtfs:isConditionallyRequiredIn rdf:resource="http://gtfs.org/routes.txt"/>
        <gtfs:isFieldOf rdf:resource="http://gtfs.org/routes.txt"/>
        <gtfs:isType rdf:resource="http://gtfs.org/Text"/>
        <gtfs:hasAdditionalInfo>Both `route_short_name` and `route_long_name` may be defined.</gtfs:hasAdditionalInfo>
        <gtfs:hasCondition>Required if `routes.route_long_name` is empty. Recommended if there is a brief service designation. This should be the commonly-known passenger name of the service, and should be no longer than 12 characters.</gtfs:hasCondition>
        <rdfs:comment>Short name of a route. Often a short, abstract identifier (e.g., &quot;32&quot;, &quot;100X&quot;, &quot;Green&quot;) that riders use to identify a route. Both `route_short_name` and `route_long_name` may be defined.</rdfs:comment>
        <rdfs:label>route_short_name</rdfs:label>
    </owl:NamedIndividual>
    


    <!-- http://gtfs.org/route_sort_order -->


    <owl:NamedIndividual rdf:about="http://gtfs.org/route_sort_order">
        <rdf:type rdf:resource="http://gtfs.org/Field"/>
        <gtfs:isFieldOf rdf:resource="http://gtfs.org/routes.txt"/>
        <gtfs:isOptionalIn rdf:resource="http://gtfs.org/routes.txt"/>
        <gtfs:isType rdf:resource="http://gtfs.org/Integer"/>
        <gtfs:hasAdditionalInfo>Non-negative integer</gtfs:hasAdditionalInfo>
        <rdfs:comment>Orders the routes in a way which is ideal for presentation to customers. Routes with smaller `route_sort_order` values should be displayed first.</rdfs:comment>
        <rdfs:label>route_sort_order</rdfs:label>
    </owl:NamedIndividual>
    


    <!-- http://gtfs.org/route_text_color -->


    <owl:NamedIndividual rdf:about="http://gtfs.org/route_text_color">
        <rdf:type rdf:resource="http://gtfs.org/Field"/>
        <gtfs:isFieldOf rdf:resource="http://gtfs.org/routes.txt"/>
        <gtfs:isOptionalIn rdf:resource="http://gtfs.org/routes.txt"/>
        <gtfs:isType rdf:resource="http://gtfs.org/Color"/>
        <gtfs:hasAdditionalInfo>The color should provide sufficient contrast when viewed on a black and white screen.</gtfs:hasAdditionalInfo>
        <rdfs:comment>Legible color to use for text drawn against a background of `route_color`. Defaults to black (`000000`) when omitted or left empty. The color difference between `route_color` and `route_text_color` should provide sufficient contrast when viewed on a black and white screen.</rdfs:comment>
        <rdfs:label>route_text_color</rdfs:label>
    </owl:NamedIndividual>
    


    <!-- http://gtfs.org/route_type -->


    <owl:NamedIndividual rdf:about="http://gtfs.org/route_type">
        <rdf:type rdf:resource="http://gtfs.org/Field"/>
        <gtfs:isFieldOf rdf:resource="http://gtfs.org/routes.txt"/>
        <gtfs:isPresence rdf:resource="http://gtfs.org/Required"/>
        <gtfs:isRequiredIn rdf:resource="http://gtfs.org/routes.txt"/>
        <gtfs:isType rdf:resource="http://gtfs.org/RouteTypeEnum"/>
        <gtfs:hasAdditionalInfo>Valid options are: 0 - Tram, Streetcar, Light rail. Any light rail or street level system within a metropolitan area. 1 - Subway, Metro. Any underground rail system within a metropolitan area. 2 - Rail. Used for intercity or long-distance travel. 3 - Bus. Used for short- and long-distance bus routes. 4 - Ferry. Used for short- and long-distance boat service. 5 - Cable tram. Used for street-level rail cars where the cable runs beneath the vehicle (e.g., cable car in San Francisco). 6 - Aerial lift, suspended cable car (e.g., gondola lift, aerial tramway). Cable transport where cabins, cars, gondolas or open chairs are suspended by means of one or more cables. 7 - Funicular. Any rail system designed for steep inclines. 11 - Trolleybus. Electric buses that draw power from overhead wires using poles. 12 - Monorail. Railway in which the track consists of a single rail or a beam.</gtfs:hasAdditionalInfo>
        <rdfs:comment>Indicates the type of transportation used on a route.</rdfs:comment>
        <rdfs:label>route_type</rdfs:label>
    </owl:NamedIndividual>
    


    <!-- http://gtfs.org/route_type_0 -->


    <owl:NamedIndividual rdf:about="http://gtfs.org/route_type_0">
        <rdf:type rdf:resource="http://gtfs.org/RouteTypeEnum"/>
        <gtfs:hasEnumValue>0</gtfs:hasEnumValue>
        <rdfs:comment>Tram, Streetcar, Light rail</rdfs:comment>
        <rdfs:label>route_type:0</rdfs:label>
    </owl:NamedIndividual>
    


    <!-- http://gtfs.org/route_type_1 -->


    <owl:NamedIndividual rdf:about="http://gtfs.org/route_type_1">
        <rdf:type rdf:resource="http://gtfs.org/RouteTypeEnum"/>
        <gtfs:hasEnumValue>1</gtfs:hasEnumValue>
        <rdfs:comment>Subway, Metro</rdfs:comment>
        <rdfs:label>route_type:1</rdfs:label>
    </owl:NamedIndividual>
    


    <!-- http://gtfs.org/route_type_11 -->


    <owl:NamedIndividual rdf:about="http://gtfs.org/route_type_11">
        <rdf:type rdf:resource="http://gtfs.org/RouteTypeEnum"/>
        <gtfs:hasEnumValue>11</gtfs:hasEnumValue>
        <rdfs:comment>Trolleybus</rdfs:comment>
        <rdfs:label>route_type:11</rdfs:label>
    </owl:NamedIndividual>
    


    <!-- http://gtfs.org/route_type_12 -->


    <owl:NamedIndividual rdf:about="http://gtfs.org/route_type_12">
        <rdf:type rdf:resource="http://gtfs.org/RouteTypeEnum"/>
        <gtfs:hasEnumValue>12</gtfs:hasEnumValue>
        <rdfs:comment>Monorail</rdfs:comment>
        <rdfs:label>route_type:12</rdfs:label>
    </owl:NamedIndividual>
    


    <!-- http://gtfs.org/route_type_2 -->


    <owl:NamedIndividual rdf:about="http://gtfs.org/route_type_2">
        <rdf:type rdf:resource="http://gtfs.org/RouteTypeEnum"/>
        <gtfs:hasEnumValue>2</gtfs:hasEnumValue>
        <rdfs:comment>Rail</rdfs:comment>
        <rdfs:label>route_type:2</rdfs:label>
    </owl:NamedIndividual>
    


    <!-- http://gtfs.org/route_type_3 -->


    <owl:NamedIndividual rdf:about="http://gtfs.org/route_type_3">
        <rdf:type rdf:resource="http://gtfs.org/RouteTypeEnum"/>
        <gtfs:hasEnumValue>3</gtfs:hasEnumValue>
        <rdfs:comment>Bus</rdfs:comment>
        <rdfs:label>route_type:3</rdfs:label>
    </owl:NamedIndividual>
    


    <!-- http://gtfs.org/route_type_4 -->


    <owl:NamedIndividual rdf:about="http://gtfs.org/route_type_4">
        <rdf:type rdf:resource="http://gtfs.org/RouteTypeEnum"/>
        <gtfs:hasEnumValue>4</gtfs:hasEnumValue>
        <rdfs:comment>Ferry</rdfs:comment>
        <rdfs:label>route_type:4</rdfs:label>
    </owl:NamedIndividual>
    


    <!-- http://gtfs.org/route_type_5 -->


    <owl:NamedIndividual rdf:about="http://gtfs.org/route_type_5">
        <rdf:type rdf:resource="http://gtfs.org/RouteTypeEnum"/>
        <gtfs:hasEnumValue>5</gtfs:hasEnumValue>
        <rdfs:comment>Cable tram</rdfs:comment>
        <rdfs:label>route_type:5</rdfs:label>
    </owl:NamedIndividual>
    


    <!-- http://gtfs.org/route_type_6 -->


    <owl:NamedIndividual rdf:about="http://gtfs.org/route_type_6">
        <rdf:type rdf:resource="http://gtfs.org/RouteTypeEnum"/>
        <gtfs:hasEnumValue>6</gtfs:hasEnumValue>
        <rdfs:comment>Aerial lift, suspended cable car</rdfs:comment>
        <rdfs:label>route_type:6</rdfs:label>
    </owl:NamedIndividual>
    


    <!-- http://gtfs.org/route_type_7 -->


    <owl:NamedIndividual rdf:about="http://gtfs.org/route_type_7">
        <rdf:type rdf:resource="http://gtfs.org/RouteTypeEnum"/>
        <gtfs:hasEnumValue>7</gtfs:hasEnumValue>
        <rdfs:comment>Funicular</rdfs:comment>
        <rdfs:label>route_type:7</rdfs:label>
    </owl:NamedIndividual>
    


    <!-- http://gtfs.org/route_url -->


    <owl:NamedIndividual rdf:about="http://gtfs.org/route_url">
        <rdf:type rdf:resource="http://gtfs.org/Field"/>
        <gtfs:isFieldOf rdf:resource="http://gtfs.org/routes.txt"/>
        <gtfs:isOptionalIn rdf:resource="http://gtfs.org/routes.txt"/>
        <gtfs:isType rdf:resource="http://gtfs.org/URL"/>
        <gtfs:hasAdditionalInfo>URL of a web page about the particular route. Should be different from the `agency.agency_url` value.</gtfs:hasAdditionalInfo>
        <rdfs:comment>URL of a web page about the particular route. Should be different from the `agency.agency_url` value.</rdfs:comment>
        <rdfs:label>route_url</rdfs:label>
    </owl:NamedIndividual>
    


    <!-- http://gtfs.org/routes.txt -->


    <owl:NamedIndividual rdf:about="http://gtfs.org/routes.txt">
        <rdf:type rdf:resource="http://gtfs.org/File"/>
        <gtfs:hasField rdf:resource="http://gtfs.org/agency_id"/>
        <gtfs:hasField rdf:resource="http://gtfs.org/continuous_drop_off"/>
        <gtfs:hasField rdf:resource="http://gtfs.org/continuous_pickup"/>
        <gtfs:hasField rdf:resource="http://gtfs.org/network_id"/>
        <gtfs:hasField rdf:resource="http://gtfs.org/route_color"/>
        <gtfs:hasField rdf:resource="http://gtfs.org/route_desc"/>
        <gtfs:hasField rdf:resource="http://gtfs.org/route_id"/>
        <gtfs:hasField rdf:resource="http://gtfs.org/route_long_name"/>
        <gtfs:hasField rdf:resource="http://gtfs.org/route_short_name"/>
        <gtfs:hasField rdf:resource="http://gtfs.org/route_sort_order"/>
        <gtfs:hasField rdf:resource="http://gtfs.org/route_text_color"/>
        <gtfs:hasField rdf:resource="http://gtfs.org/route_type"/>
        <gtfs:hasField rdf:resource="http://gtfs.org/route_url"/>
        <gtfs:isFileOf rdf:resource="http://gtfs.org/GTFS_Static"/>
        <gtfs:isRequiredIn rdf:resource="http://gtfs.org/GTFS_Static"/>
        <rdfs:comment>Transit routes. A route is a group of trips that are displayed to riders as a single service.</rdfs:comment>
        <rdfs:label>routes.txt</rdfs:label>
    </owl:NamedIndividual>
    


    <!-- http://gtfs.org/saturday -->


    <owl:NamedIndividual rdf:about="http://gtfs.org/saturday">
        <rdf:type rdf:resource="http://gtfs.org/Field"/>
        <gtfs:isFieldOf rdf:resource="http://gtfs.org/calendar.txt"/>
        <gtfs:isPresence rdf:resource="http://gtfs.org/Required"/>
        <gtfs:isRequiredIn rdf:resource="http://gtfs.org/calendar.txt"/>
        <gtfs:isType rdf:resource="http://gtfs.org/SaturdayEnum"/>
        <gtfs:hasAdditionalInfo>Enum type field</gtfs:hasAdditionalInfo>
        <rdfs:comment>Functions in the same way as `monday` except applies to Saturdays.</rdfs:comment>
        <rdfs:label>saturday</rdfs:label>
    </owl:NamedIndividual>
    


    <!-- http://gtfs.org/saturday_example_key -->


    <owl:NamedIndividual rdf:about="http://gtfs.org/saturday_example_key">
        <rdf:type rdf:resource="http://gtfs.org/SaturdayEnum"/>
        <gtfs:hasEnumValue>example_key</gtfs:hasEnumValue>
        <rdfs:comment>example_value</rdfs:comment>
        <rdfs:label>saturday:example_key</rdfs:label>
    </owl:NamedIndividual>
    


    <!-- http://gtfs.org/service_id -->


    <owl:NamedIndividual rdf:about="http://gtfs.org/service_id">
        <rdf:type rdf:resource="http://gtfs.org/Field"/>
        <gtfs:isFieldOf rdf:resource="http://gtfs.org/calendar.txt"/>
        <gtfs:isFieldOf rdf:resource="http://gtfs.org/calendar_dates.txt"/>
        <gtfs:isFieldOf rdf:resource="http://gtfs.org/timeframes.txt"/>
        <gtfs:isFieldOf rdf:resource="http://gtfs.org/trips.txt"/>
        <gtfs:isRequiredIn rdf:resource="http://gtfs.org/calendar.txt"/>
        <gtfs:isRequiredIn rdf:resource="http://gtfs.org/calendar_dates.txt"/>
        <gtfs:isRequiredIn rdf:resource="http://gtfs.org/timeframes.txt"/>
        <gtfs:isRequiredIn rdf:resource="http://gtfs.org/trips.txt"/>
        <gtfs:isType rdf:resource="http://gtfs.org/ID"/>
        <gtfs:hasAdditionalInfo>Foreign ID referencing `calendar.service_id` or `calendar_dates.service_id`</gtfs:hasAdditionalInfo>
        <gtfs:hasAdditionalInfo>Foreign ID referencing calendar.service_id or ID</gtfs:hasAdditionalInfo>
        <gtfs:hasAdditionalInfo>Unique ID</gtfs:hasAdditionalInfo>
        <gtfs:isForeignID rdf:resource="http://gtfs.org/calendar_dates.txt"/>
        <gtfs:isForeignID rdf:resource="http://gtfs.org/timeframes.txt"/>
        <gtfs:isForeignID rdf:resource="http://gtfs.org/trips.txt"/>
        <gtfs:isUniqueID rdf:resource="http://gtfs.org/calendar.txt"/>
        <rdfs:comment>Identifies a set of dates that a timeframe is in effect.</rdfs:comment>
        <rdfs:comment>Identifies a set of dates when a service exception occurs for one or more routes. Each (`service_id`, `date`) pair may only appear once in calendar_dates.txt if using calendar.txt and calendar_dates.txt in conjunction. If a service_id value appears in both calendar.txt and calendar_dates.txt, the information in calendar_dates.txt modifies the service information specified in calendar.txt.</rdfs:comment>
        <rdfs:comment>Identifies a set of dates when service is available for one or more routes.</rdfs:comment>
        <rdfs:comment>Identifies a set of dates when service is available for one or more routes. Each `service_id` value must be unique in a [calendar.txt](#calendartxt) file.</rdfs:comment>
        <rdfs:label>service_id</rdfs:label>
    </owl:NamedIndividual>
    


    <!-- http://gtfs.org/shape_dist_traveled -->


    <owl:NamedIndividual rdf:about="http://gtfs.org/shape_dist_traveled">
        <rdf:type rdf:resource="http://gtfs.org/Field"/>
        <gtfs:isFieldOf rdf:resource="http://gtfs.org/shapes.txt"/>
        <gtfs:isFieldOf rdf:resource="http://gtfs.org/stop_times.txt"/>
        <gtfs:isOptionalIn rdf:resource="http://gtfs.org/shapes.txt"/>
        <gtfs:isOptionalIn rdf:resource="http://gtfs.org/stop_times.txt"/>
        <gtfs:isType rdf:resource="http://gtfs.org/Float"/>
        <gtfs:hasAdditionalInfo>Non-negative float. Must be in the same units as shapes.txt.</gtfs:hasAdditionalInfo>
        <gtfs:hasAdditionalInfo>Recommended for routes that have looping or inlining (the vehicle crosses or travels over the same portion of alignment in one trip).</gtfs:hasAdditionalInfo>
        <gtfs:hasExample>If a bus travels a distance of 5.25 kilometers from the start of the shape to the stop, shape_dist_traveled=5.25.</gtfs:hasExample>
        <rdfs:comment>Actual distance traveled along the associated shape, from the first stop to the stop specified in this record. This field specifies how much of the shape to draw between any two stops during a trip. Must be in the same units used in shapes.txt. Values used for shape_dist_traveled must increase along with stop_sequence; they must not be used to show reverse travel along a route. Recommended for routes that have looping or inlining (the vehicle crosses or travels over the same portion of alignment in one trip). See shapes.shape_dist_traveled.</rdfs:comment>
        <rdfs:comment>Actual distance traveled along the shape from the first shape point to the point specified in this record. Used by trip planners to show the correct portion of the shape on a map. Values must increase along with shape_pt_sequence; they must not be used to show reverse travel along a route. Distance units must be consistent with those used in stop_times.txt. Recommended for routes that have looping or inlining (the vehicle crosses or travels over the same portion of alignment in one trip). If a vehicle retraces or crosses the route alignment at points in the course of a trip, shape_dist_traveled is important to clarify how portions of the points in shapes.txt line up correspond with records in stop_times.txt.</rdfs:comment>
        <rdfs:label>shape_dist_traveled</rdfs:label>
    </owl:NamedIndividual>
    


    <!-- http://gtfs.org/shape_id -->


    <owl:NamedIndividual rdf:about="http://gtfs.org/shape_id">
        <rdf:type rdf:resource="http://gtfs.org/Field"/>
        <gtfs:isConditionallyRequiredIn rdf:resource="http://gtfs.org/trips.txt"/>
        <gtfs:isFieldOf rdf:resource="http://gtfs.org/shapes.txt"/>
        <gtfs:isFieldOf rdf:resource="http://gtfs.org/trips.txt"/>
        <gtfs:isRequiredIn rdf:resource="http://gtfs.org/shapes.txt"/>
        <gtfs:isType rdf:resource="http://gtfs.org/ID"/>
        <gtfs:hasAdditionalInfo>Foreign ID referencing shapes.shape_id</gtfs:hasAdditionalInfo>
        <gtfs:hasAdditionalInfo>This field is used to identify a shape.</gtfs:hasAdditionalInfo>
        <gtfs:hasCondition>Required if the trip has a continuous pickup or drop-off behavior defined either in routes.txt or in stop_times.txt. Optional otherwise.</gtfs:hasCondition>
        <gtfs:isForeignID rdf:resource="http://gtfs.org/trips.txt"/>
        <gtfs:isUniqueID rdf:resource="http://gtfs.org/shapes.txt"/>
        <rdfs:comment>Identifies a geospatial shape describing the vehicle travel path for a trip.</rdfs:comment>
        <rdfs:comment>Identifies a shape.</rdfs:comment>
        <rdfs:label>shape_id</rdfs:label>
    </owl:NamedIndividual>
    


    <!-- http://gtfs.org/shape_pt_lat -->


    <owl:NamedIndividual rdf:about="http://gtfs.org/shape_pt_lat">
        <rdf:type rdf:resource="http://gtfs.org/Field"/>
        <gtfs:isFieldOf rdf:resource="http://gtfs.org/shapes.txt"/>
        <gtfs:isRequiredIn rdf:resource="http://gtfs.org/shapes.txt"/>
        <gtfs:isType rdf:resource="http://gtfs.org/Latitude"/>
        <gtfs:hasAdditionalInfo>Latitude</gtfs:hasAdditionalInfo>
        <rdfs:comment>Latitude of a shape point. Each record in shapes.txt represents a shape point used to define the shape.</rdfs:comment>
        <rdfs:label>shape_pt_lat</rdfs:label>
    </owl:NamedIndividual>
    


    <!-- http://gtfs.org/shape_pt_lon -->


    <owl:NamedIndividual rdf:about="http://gtfs.org/shape_pt_lon">
        <rdf:type rdf:resource="http://gtfs.org/Field"/>
        <gtfs:isFieldOf rdf:resource="http://gtfs.org/shapes.txt"/>
        <gtfs:isRequiredIn rdf:resource="http://gtfs.org/shapes.txt"/>
        <gtfs:isType rdf:resource="http://gtfs.org/Longitude"/>
        <gtfs:hasAdditionalInfo>This field represents the longitude of a shape point on a map.</gtfs:hasAdditionalInfo>
        <rdfs:comment>Longitude of a shape point.</rdfs:comment>
        <rdfs:label>shape_pt_lon</rdfs:label>
    </owl:NamedIndividual>
    


    <!-- http://gtfs.org/shape_pt_sequence -->


    <owl:NamedIndividual rdf:about="http://gtfs.org/shape_pt_sequence">
        <rdf:type rdf:resource="http://gtfs.org/Field"/>
        <gtfs:isFieldOf rdf:resource="http://gtfs.org/shapes.txt"/>
        <gtfs:isRequiredIn rdf:resource="http://gtfs.org/shapes.txt"/>
        <gtfs:isType rdf:resource="http://gtfs.org/Integer"/>
        <gtfs:hasAdditionalInfo>Values must increase along the trip but do not need to be consecutive.</gtfs:hasAdditionalInfo>
        <gtfs:hasExample>If the shape &quot;A_shp&quot; has three points in its definition, the shapes.txt file might contain these records to define the shape: shape_id,shape_pt_lat,shape_pt_lon,shape_pt_sequence A_shp,37.61956,-122.48161,0 A_shp,37.64430,-122.41070,6 A_shp,37.65863,-122.30839,11</gtfs:hasExample>
        <rdfs:comment>Sequence in which the shape points connect to form the shape. Values must increase along the trip but do not need to be consecutive.</rdfs:comment>
        <rdfs:label>shape_pt_sequence</rdfs:label>
    </owl:NamedIndividual>
    


    <!-- http://gtfs.org/shapes.txt -->


    <owl:NamedIndividual rdf:about="http://gtfs.org/shapes.txt">
        <rdf:type rdf:resource="http://gtfs.org/File"/>
        <gtfs:hasField rdf:resource="http://gtfs.org/shape_dist_traveled"/>
        <gtfs:hasField rdf:resource="http://gtfs.org/shape_id"/>
        <gtfs:hasField rdf:resource="http://gtfs.org/shape_pt_lat"/>
        <gtfs:hasField rdf:resource="http://gtfs.org/shape_pt_lon"/>
        <gtfs:hasField rdf:resource="http://gtfs.org/shape_pt_sequence"/>
        <gtfs:isFileOf rdf:resource="http://gtfs.org/GTFS_Static"/>
        <gtfs:isOptionalIn rdf:resource="http://gtfs.org/GTFS_Static"/>
        <rdfs:comment>Rules for mapping vehicle travel paths, sometimes referred to as route alignments.</rdfs:comment>
        <rdfs:label>shapes.txt</rdfs:label>
    </owl:NamedIndividual>
    


    <!-- http://gtfs.org/signposted_as -->


    <owl:NamedIndividual rdf:about="http://gtfs.org/signposted_as">
        <rdf:type rdf:resource="http://gtfs.org/Field"/>
        <gtfs:isFieldOf rdf:resource="http://gtfs.org/pathways.txt"/>
        <gtfs:isOptionalIn rdf:resource="http://gtfs.org/pathways.txt"/>
        <gtfs:isType rdf:resource="http://gtfs.org/Text"/>
        <gtfs:hasAdditionalInfo>May be used to provide text directions to riders, such as &apos;follow signs to &apos;. The text in `singposted_as` should appear exactly how it is printed on the signs. When the physical signage is multilingual, this field may be populated and translated following the example of `stops.stop_name` in the field definition of `feed_info.feed_lang`.</gtfs:hasAdditionalInfo>
        <rdfs:comment>Public facing text from physical signage that is visible to riders. May be used to provide text directions to riders, such as &apos;follow signs to &apos;. The text in `singposted_as` should appear exactly how it is printed on the signs. When the physical signage is multilingual, this field may be populated and translated following the example of `stops.stop_name` in the field definition of `feed_info.feed_lang`.</rdfs:comment>
        <rdfs:label>signposted_as</rdfs:label>
    </owl:NamedIndividual>
    


    <!-- http://gtfs.org/stair_count -->


    <owl:NamedIndividual rdf:about="http://gtfs.org/stair_count">
        <rdf:type rdf:resource="http://gtfs.org/Field"/>
        <gtfs:isFieldOf rdf:resource="http://gtfs.org/pathways.txt"/>
        <gtfs:isOptionalIn rdf:resource="http://gtfs.org/pathways.txt"/>
        <gtfs:isType rdf:resource="http://gtfs.org/Integer"/>
        <gtfs:hasAdditionalInfo>Non-null integer</gtfs:hasAdditionalInfo>
        <rdfs:comment>Number of stairs of the pathway.

A positive `stair_count` implies that the rider walks up from `from_stop_id` to `to_stop_id`. And a negative `stair_count` implies that the rider walks down from `from_stop_id` to `to_stop_id`.

This field is recommended for stairs (`pathway_mode=2`).

If only an estimated stair count can be provided, it is recommended to approximate 15 stairs for 1 floor.</rdfs:comment>
        <rdfs:label>stair_count</rdfs:label>
    </owl:NamedIndividual>
    


    <!-- http://gtfs.org/start_date -->


    <owl:NamedIndividual rdf:about="http://gtfs.org/start_date">
        <rdf:type rdf:resource="http://gtfs.org/Field"/>
        <gtfs:isFieldOf rdf:resource="http://gtfs.org/calendar.txt"/>
        <gtfs:isRequiredIn rdf:resource="http://gtfs.org/calendar.txt"/>
        <gtfs:isType rdf:resource="http://gtfs.org/Date"/>
        <gtfs:hasAdditionalInfo>The start service day for the service interval must be provided in the specified format.</gtfs:hasAdditionalInfo>
        <rdfs:comment>Start service day for the service interval.</rdfs:comment>
        <rdfs:label>start_date</rdfs:label>
    </owl:NamedIndividual>
    


    <!-- http://gtfs.org/start_time -->


    <owl:NamedIndividual rdf:about="http://gtfs.org/start_time">
        <rdf:type rdf:resource="http://gtfs.org/Field"/>
        <gtfs:isConditionallyRequiredIn rdf:resource="http://gtfs.org/timeframes.txt"/>
        <gtfs:isFieldOf rdf:resource="http://gtfs.org/frequencies.txt"/>
        <gtfs:isFieldOf rdf:resource="http://gtfs.org/timeframes.txt"/>
        <gtfs:isRequiredIn rdf:resource="http://gtfs.org/frequencies.txt"/>
        <gtfs:isType rdf:resource="http://gtfs.org/Time"/>
        <gtfs:hasAdditionalInfo>The start time is crucial for scheduling the departure of the first vehicle.</gtfs:hasAdditionalInfo>
        <gtfs:hasCondition>Required if timeframes.end_time is defined. Forbidden otherwise</gtfs:hasCondition>
        <rdfs:comment>Defines the beginning of a timeframe. The interval includes the start time. Values greater than 24:00:00 are forbidden. An empty value in start_time is considered 00:00:00.</rdfs:comment>
        <rdfs:comment>Time at which the first vehicle departs from the first stop of the trip with the specified headway.</rdfs:comment>
        <rdfs:label>start_time</rdfs:label>
    </owl:NamedIndividual>
    


    <!-- http://gtfs.org/stop_areas.txt -->


    <owl:NamedIndividual rdf:about="http://gtfs.org/stop_areas.txt">
        <rdf:type rdf:resource="http://gtfs.org/File"/>
        <gtfs:hasField rdf:resource="http://gtfs.org/area_id"/>
        <gtfs:hasField rdf:resource="http://gtfs.org/stop_id"/>
        <gtfs:isFileOf rdf:resource="http://gtfs.org/GTFS_Static"/>
        <gtfs:isOptionalIn rdf:resource="http://gtfs.org/GTFS_Static"/>
        <rdfs:comment>Rules to assign stops to areas.</rdfs:comment>
        <rdfs:label>stop_areas.txt</rdfs:label>
    </owl:NamedIndividual>
    


    <!-- http://gtfs.org/stop_code -->


    <owl:NamedIndividual rdf:about="http://gtfs.org/stop_code">
        <rdf:type rdf:resource="http://gtfs.org/Field"/>
        <gtfs:isFieldOf rdf:resource="http://gtfs.org/stops.txt"/>
        <gtfs:isOptionalIn rdf:resource="http://gtfs.org/stops.txt"/>
        <gtfs:isType rdf:resource="http://gtfs.org/Text"/>
        <gtfs:hasAdditionalInfo>The `stop_code` field is used to identify locations for riders in transit systems.</gtfs:hasAdditionalInfo>
        <rdfs:comment>Short text or a number that identifies the location for riders. These codes are often used in phone-based transit information systems or printed on signage to make it easier for riders to get information for a particular location. The `stop_code` may be the same as `stop_id` if it is public facing. This field should be left empty for locations without a code presented to riders.</rdfs:comment>
        <rdfs:label>stop_code</rdfs:label>
    </owl:NamedIndividual>
    


    <!-- http://gtfs.org/stop_desc -->


    <owl:NamedIndividual rdf:about="http://gtfs.org/stop_desc">
        <rdf:type rdf:resource="http://gtfs.org/Field"/>
        <gtfs:isFieldOf rdf:resource="http://gtfs.org/stops.txt"/>
        <gtfs:isOptionalIn rdf:resource="http://gtfs.org/stops.txt"/>
        <gtfs:isType rdf:resource="http://gtfs.org/Text"/>
        <gtfs:hasAdditionalInfo>Description of the location that provides useful, quality information. Should not be a duplicate of `stop_name`.</gtfs:hasAdditionalInfo>
        <rdfs:comment>Description of the location that provides useful, quality information. Should not be a duplicate of `stop_name`.</rdfs:comment>
        <rdfs:label>stop_desc</rdfs:label>
    </owl:NamedIndividual>
    


    <!-- http://gtfs.org/stop_headsign -->


    <owl:NamedIndividual rdf:about="http://gtfs.org/stop_headsign">
        <rdf:type rdf:resource="http://gtfs.org/Field"/>
        <gtfs:isFieldOf rdf:resource="http://gtfs.org/stop_times.txt"/>
        <gtfs:isOptionalIn rdf:resource="http://gtfs.org/stop_times.txt"/>
        <gtfs:isType rdf:resource="http://gtfs.org/Text"/>
        <rdfs:comment>Text that appears on signage identifying the trip&apos;s destination to riders. This field overrides the default `trips.trip_headsign` when the headsign changes between stops. If the headsign is displayed for an entire trip, `trips.trip_headsign` should be used instead. A `stop_headsign` value specified for one `stop_time` does not apply to subsequent `stop_time`s in the same trip. If you want to override the `trip_headsign` for multiple `stop_time`s in the same trip, the `stop_headsign` value must be repeated in each `stop_time` row.</rdfs:comment>
        <rdfs:label>stop_headsign</rdfs:label>
    </owl:NamedIndividual>
    


    <!-- http://gtfs.org/stop_id -->


    <owl:NamedIndividual rdf:about="http://gtfs.org/stop_id">
        <rdf:type rdf:resource="http://gtfs.org/Field"/>
        <gtfs:isFieldOf rdf:resource="http://gtfs.org/stop_areas.txt"/>
        <gtfs:isFieldOf rdf:resource="http://gtfs.org/stop_times.txt"/>
        <gtfs:isFieldOf rdf:resource="http://gtfs.org/stops.txt"/>
        <gtfs:isRequiredIn rdf:resource="http://gtfs.org/stop_areas.txt"/>
        <gtfs:isRequiredIn rdf:resource="http://gtfs.org/stop_times.txt"/>
        <gtfs:isRequiredIn rdf:resource="http://gtfs.org/stops.txt"/>
        <gtfs:isType rdf:resource="http://gtfs.org/ID"/>
        <gtfs:hasAdditionalInfo>Foreign ID referencing stops.stop_id</gtfs:hasAdditionalInfo>
        <gtfs:hasAdditionalInfo>Unique ID</gtfs:hasAdditionalInfo>
        <gtfs:isForeignID rdf:resource="http://gtfs.org/stop_areas.txt"/>
        <gtfs:isForeignID rdf:resource="http://gtfs.org/stop_times.txt"/>
        <gtfs:isUniqueID rdf:resource="http://gtfs.org/stops.txt"/>
        <rdfs:comment>Identifies a location: stop/platform, station, entrance/exit, generic node or boarding area (see `location_type`). Multiple routes may use the same `stop_id`.</rdfs:comment>
        <rdfs:comment>Identifies a stop. If a station (i.e. a stop with stops.location_type=1) is defined in this field, it is assumed that all of its platforms (i.e. all stops with stops.location_type=0 that have this station defined as stops.parent_station) are part of the same area. This behavior can be overridden by assigning platforms to other areas.</rdfs:comment>
        <rdfs:comment>Identifies the serviced stop. All stops serviced during a trip must have a record in stop_times.txt. Referenced locations must be stops/platforms, i.e. their stops.location_type value must be 0 or empty. A stop may be serviced multiple times in the same trip, and multiple trips and routes may service the same stop.</rdfs:comment>
        <rdfs:label>stop_id</rdfs:label>
    </owl:NamedIndividual>
    


    <!-- http://gtfs.org/stop_lat -->


    <owl:NamedIndividual rdf:about="http://gtfs.org/stop_lat">
        <rdf:type rdf:resource="http://gtfs.org/Field"/>
        <gtfs:isConditionallyRequiredIn rdf:resource="http://gtfs.org/stops.txt"/>
        <gtfs:isFieldOf rdf:resource="http://gtfs.org/stops.txt"/>
        <gtfs:isType rdf:resource="http://gtfs.org/Latitude"/>
        <gtfs:hasAdditionalInfo>Latitude</gtfs:hasAdditionalInfo>
        <gtfs:hasCondition>Required for locations which are stops (`location_type=0`), stations (`location_type=1`) or entrances/exits (`location_type=2`). Optional for locations which are generic nodes (`location_type=3`) or boarding areas (`location_type=4`)</gtfs:hasCondition>
        <rdfs:comment>Latitude of the location.

For stops/platforms (`location_type=0`) and boarding area (`location_type=4`), the coordinates must be the ones of the bus pole — if exists — and otherwise of where the travelers are boarding the vehicle (on the sidewalk or the platform, and not on the roadway or the track where the vehicle stops). 

Conditionally Required:
- **Required** for locations which are stops (`location_type=0`), stations (`location_type=1`) or entrances/exits (`location_type=2`).
- Optional for locations which are generic nodes (`location_type=3`) or boarding areas (`location_type=4`).</rdfs:comment>
        <rdfs:label>stop_lat</rdfs:label>
    </owl:NamedIndividual>
    


    <!-- http://gtfs.org/stop_lon -->


    <owl:NamedIndividual rdf:about="http://gtfs.org/stop_lon">
        <rdf:type rdf:resource="http://gtfs.org/Field"/>
        <gtfs:isConditionallyRequiredIn rdf:resource="http://gtfs.org/stops.txt"/>
        <gtfs:isFieldOf rdf:resource="http://gtfs.org/stops.txt"/>
        <gtfs:isType rdf:resource="http://gtfs.org/Longitude"/>
        <gtfs:hasAdditionalInfo>The coordinates must be provided for specific location types as mentioned in the description.</gtfs:hasAdditionalInfo>
        <gtfs:hasCondition>Required</gtfs:hasCondition>
        <rdfs:comment>Longitude of the location.

For stops/platforms (`location_type=0`) and boarding area (`location_type=4`), the coordinates must be the ones of the bus pole — if exists — and otherwise of where the travelers are boarding the vehicle (on the sidewalk or the platform, and not on the roadway or the track where the vehicle stops). 

Conditionally Required:
- **Required** for locations which are stops (`location_type=0`), stations (`location_type=1`) or entrances/exits (`location_type=2`).
- Optional for locations which are generic nodes (`location_type=3`) or boarding areas (`location_type=4`).</rdfs:comment>
        <rdfs:label>stop_lon</rdfs:label>
    </owl:NamedIndividual>
    


    <!-- http://gtfs.org/stop_name -->


    <owl:NamedIndividual rdf:about="http://gtfs.org/stop_name">
        <rdf:type rdf:resource="http://gtfs.org/Field"/>
        <gtfs:isConditionallyRequiredIn rdf:resource="http://gtfs.org/stops.txt"/>
        <gtfs:isFieldOf rdf:resource="http://gtfs.org/stops.txt"/>
        <gtfs:isType rdf:resource="http://gtfs.org/Text"/>
        <gtfs:hasAdditionalInfo>The `stop_name` field is used to specify the name of the location in the GTFS data.</gtfs:hasAdditionalInfo>
        <gtfs:hasCondition>Required for locations which are stops (`location_type=0`), stations (`location_type=1`) or entrances/exits (`location_type=2`). Optional for locations which are generic nodes (`location_type=3`) or boarding areas (`location_type=4`).</gtfs:hasCondition>
        <rdfs:comment>Name of the location. The `stop_name` should match the agency&apos;s rider-facing name for the location as printed on a timetable, published online, or represented on signage. For translations into other languages, use `translations.txt`.

When the location is a boarding area (`location_type=4`), the `stop_name` should contains the name of the boarding area as displayed by the agency. It could be just one letter (like on some European intercity railway stations), or text like “Wheelchair boarding area” (NYC’s Subway) or “Head of short trains” (Paris’ RER).

Conditionally Required:
- **Required** for locations which are stops (`location_type=0`), stations (`location_type=1`) or entrances/exits (`location_type=2`).
- Optional for locations which are generic nodes (`location_type=3`) or boarding areas (`location_type=4`).</rdfs:comment>
        <rdfs:label>stop_name</rdfs:label>
    </owl:NamedIndividual>
    


    <!-- http://gtfs.org/stop_sequence -->


    <owl:NamedIndividual rdf:about="http://gtfs.org/stop_sequence">
        <rdf:type rdf:resource="http://gtfs.org/Field"/>
        <gtfs:isFieldOf rdf:resource="http://gtfs.org/stop_times.txt"/>
        <gtfs:isRequiredIn rdf:resource="http://gtfs.org/stop_times.txt"/>
        <gtfs:isType rdf:resource="http://gtfs.org/Integer"/>
        <gtfs:hasAdditionalInfo>Non-negative integer</gtfs:hasAdditionalInfo>
        <gtfs:hasExample>The first location on the trip could have a stop_sequence=1, the second location on the trip could have a stop_sequence=23, the third location could have a stop_sequence=40, and so on.</gtfs:hasExample>
        <rdfs:comment>Order of stops for a particular trip. The values must increase along the trip but do not need to be consecutive.</rdfs:comment>
        <rdfs:label>stop_sequence</rdfs:label>
    </owl:NamedIndividual>
    


    <!-- http://gtfs.org/stop_times.txt -->


    <owl:NamedIndividual rdf:about="http://gtfs.org/stop_times.txt">
        <rdf:type rdf:resource="http://gtfs.org/File"/>
        <gtfs:hasField rdf:resource="http://gtfs.org/arrival_time"/>
        <gtfs:hasField rdf:resource="http://gtfs.org/continuous_drop_off"/>
        <gtfs:hasField rdf:resource="http://gtfs.org/continuous_pickup"/>
        <gtfs:hasField rdf:resource="http://gtfs.org/departure_time"/>
        <gtfs:hasField rdf:resource="http://gtfs.org/drop_off_type"/>
        <gtfs:hasField rdf:resource="http://gtfs.org/pickup_type"/>
        <gtfs:hasField rdf:resource="http://gtfs.org/shape_dist_traveled"/>
        <gtfs:hasField rdf:resource="http://gtfs.org/stop_headsign"/>
        <gtfs:hasField rdf:resource="http://gtfs.org/stop_id"/>
        <gtfs:hasField rdf:resource="http://gtfs.org/stop_sequence"/>
        <gtfs:hasField rdf:resource="http://gtfs.org/timepoint"/>
        <gtfs:hasField rdf:resource="http://gtfs.org/trip_id"/>
        <gtfs:isFileOf rdf:resource="http://gtfs.org/GTFS_Static"/>
        <gtfs:isRequiredIn rdf:resource="http://gtfs.org/GTFS_Static"/>
        <rdfs:comment>Times that a vehicle arrives at and departs from stops for each trip.</rdfs:comment>
        <rdfs:label>stop_times.txt</rdfs:label>
    </owl:NamedIndividual>
    


    <!-- http://gtfs.org/stop_timezone -->


    <owl:NamedIndividual rdf:about="http://gtfs.org/stop_timezone">
        <rdf:type rdf:resource="http://gtfs.org/Field"/>
        <gtfs:isFieldOf rdf:resource="http://gtfs.org/stops.txt"/>
        <gtfs:isOptionalIn rdf:resource="http://gtfs.org/stops.txt"/>
        <gtfs:isType rdf:resource="http://gtfs.org/TimeZone"/>
        <gtfs:hasAdditionalInfo>Timezone of the location. If the location has a parent station, it inherits the parent station’s timezone instead of applying its own. Stations and parentless stops with empty stop_timezone inherit the timezone specified by agency.agency_timezone. If stop_timezone values are provided, the times in stop_times.txt should be entered as the time since midnight in the timezone specified by agency.agency_timezone. This ensures that the time values in a trip always increase over the course of a trip, regardless of which timezones the trip crosses.</gtfs:hasAdditionalInfo>
        <rdfs:comment>Timezone of the location. If the location has a parent station, it inherits the parent station’s timezone instead of applying its own. Stations and parentless stops with empty stop_timezone inherit the timezone specified by agency.agency_timezone. If stop_timezone values are provided, the times in stop_times.txt should be entered as the time since midnight in the timezone specified by agency.agency_timezone. This ensures that the time values in a trip always increase over the course of a trip, regardless of which timezones the trip crosses.</rdfs:comment>
        <rdfs:label>stop_timezone</rdfs:label>
    </owl:NamedIndividual>
    


    <!-- http://gtfs.org/stop_url -->


    <owl:NamedIndividual rdf:about="http://gtfs.org/stop_url">
        <rdf:type rdf:resource="http://gtfs.org/Field"/>
        <gtfs:isFieldOf rdf:resource="http://gtfs.org/stops.txt"/>
        <gtfs:isOptionalIn rdf:resource="http://gtfs.org/stops.txt"/>
        <gtfs:isType rdf:resource="http://gtfs.org/URL"/>
        <gtfs:hasAdditionalInfo>URL should be different from `agency.agency_url` and `routes.route_url` field values.</gtfs:hasAdditionalInfo>
        <rdfs:comment>URL of a web page about the location. This should be different from the `agency.agency_url` and the `routes.route_url` field values.</rdfs:comment>
        <rdfs:label>stop_url</rdfs:label>
    </owl:NamedIndividual>
    


    <!-- http://gtfs.org/stops.txt -->


    <owl:NamedIndividual rdf:about="http://gtfs.org/stops.txt">
        <rdf:type rdf:resource="http://gtfs.org/File"/>
        <gtfs:hasField rdf:resource="http://gtfs.org/level_id"/>
        <gtfs:hasField rdf:resource="http://gtfs.org/location_type"/>
        <gtfs:hasField rdf:resource="http://gtfs.org/parent_station"/>
        <gtfs:hasField rdf:resource="http://gtfs.org/platform_code"/>
        <gtfs:hasField rdf:resource="http://gtfs.org/stop_code"/>
        <gtfs:hasField rdf:resource="http://gtfs.org/stop_desc"/>
        <gtfs:hasField rdf:resource="http://gtfs.org/stop_id"/>
        <gtfs:hasField rdf:resource="http://gtfs.org/stop_lat"/>
        <gtfs:hasField rdf:resource="http://gtfs.org/stop_lon"/>
        <gtfs:hasField rdf:resource="http://gtfs.org/stop_name"/>
        <gtfs:hasField rdf:resource="http://gtfs.org/stop_timezone"/>
        <gtfs:hasField rdf:resource="http://gtfs.org/stop_url"/>
        <gtfs:hasField rdf:resource="http://gtfs.org/tts_stop_name"/>
        <gtfs:hasField rdf:resource="http://gtfs.org/wheelchair_boarding"/>
        <gtfs:hasField rdf:resource="http://gtfs.org/zone_id"/>
        <gtfs:isFileOf rdf:resource="http://gtfs.org/GTFS_Static"/>
        <gtfs:isRequiredIn rdf:resource="http://gtfs.org/GTFS_Static"/>
        <rdfs:comment>Stops where vehicles pick up or drop off riders. Also defines stations and station entrances.</rdfs:comment>
        <rdfs:label>stops.txt</rdfs:label>
    </owl:NamedIndividual>
    


    <!-- http://gtfs.org/sunday -->


    <owl:NamedIndividual rdf:about="http://gtfs.org/sunday">
        <rdf:type rdf:resource="http://gtfs.org/Field"/>
        <gtfs:isFieldOf rdf:resource="http://gtfs.org/calendar.txt"/>
        <gtfs:isPresence rdf:resource="http://gtfs.org/Required"/>
        <gtfs:isRequiredIn rdf:resource="http://gtfs.org/calendar.txt"/>
        <gtfs:isType rdf:resource="http://gtfs.org/SundayEnum"/>
        <gtfs:hasAdditionalInfo>Enum type field that applies to Sundays.</gtfs:hasAdditionalInfo>
        <rdfs:comment>Functions in the same way as `monday` except applies to Sundays.</rdfs:comment>
        <rdfs:label>sunday</rdfs:label>
    </owl:NamedIndividual>
    


    <!-- http://gtfs.org/sunday_1 -->


    <owl:NamedIndividual rdf:about="http://gtfs.org/sunday_1">
        <rdf:type rdf:resource="http://gtfs.org/SundayEnum"/>
        <gtfs:hasEnumValue>1</gtfs:hasEnumValue>
        <rdfs:comment>Applies to Sundays</rdfs:comment>
        <rdfs:label>sunday:1</rdfs:label>
    </owl:NamedIndividual>
    


    <!-- http://gtfs.org/table_name -->


    <owl:NamedIndividual rdf:about="http://gtfs.org/table_name">
        <rdf:type rdf:resource="http://gtfs.org/Field"/>
        <gtfs:isFieldOf rdf:resource="http://gtfs.org/translations.txt"/>
        <gtfs:isPresence rdf:resource="http://gtfs.org/Required"/>
        <gtfs:isRequiredIn rdf:resource="http://gtfs.org/translations.txt"/>
        <gtfs:isType rdf:resource="http://gtfs.org/TableNameEnum"/>
        <gtfs:hasAdditionalInfo>Allowed values: agency, stops, routes, trips, stop_times, pathways, levels, feed_info, attributions</gtfs:hasAdditionalInfo>
        <gtfs:isUniqueID rdf:resource="http://gtfs.org/translations.txt"/>
        <rdfs:comment>Defines the table that contains the field to be translated. Allowed values are: - `agency` - `stops` - `routes` - `trips` - `stop_times` - `pathways` - `levels` - `feed_info` - `attributions`. Any file added to GTFS will have a `table_name` value equivalent to the file name, as listed above (i.e., not including the `.txt` file extension).</rdfs:comment>
        <rdfs:label>table_name</rdfs:label>
    </owl:NamedIndividual>
    


    <!-- http://gtfs.org/table_name_agency -->


    <owl:NamedIndividual rdf:about="http://gtfs.org/table_name_agency">
        <rdf:type rdf:resource="http://gtfs.org/TableNameEnum"/>
        <gtfs:hasEnumValue>agency</gtfs:hasEnumValue>
        <rdfs:comment>Agency</rdfs:comment>
        <rdfs:label>table_name:agency</rdfs:label>
    </owl:NamedIndividual>
    


    <!-- http://gtfs.org/table_name_attributions -->


    <owl:NamedIndividual rdf:about="http://gtfs.org/table_name_attributions">
        <rdf:type rdf:resource="http://gtfs.org/TableNameEnum"/>
        <gtfs:hasEnumValue>attributions</gtfs:hasEnumValue>
        <rdfs:comment>Attributions</rdfs:comment>
        <rdfs:label>table_name:attributions</rdfs:label>
    </owl:NamedIndividual>
    


    <!-- http://gtfs.org/table_name_feed_info -->


    <owl:NamedIndividual rdf:about="http://gtfs.org/table_name_feed_info">
        <rdf:type rdf:resource="http://gtfs.org/TableNameEnum"/>
        <gtfs:hasEnumValue>feed_info</gtfs:hasEnumValue>
        <rdfs:comment>Feed Info</rdfs:comment>
        <rdfs:label>table_name:feed_info</rdfs:label>
    </owl:NamedIndividual>
    


    <!-- http://gtfs.org/table_name_levels -->


    <owl:NamedIndividual rdf:about="http://gtfs.org/table_name_levels">
        <rdf:type rdf:resource="http://gtfs.org/TableNameEnum"/>
        <gtfs:hasEnumValue>levels</gtfs:hasEnumValue>
        <rdfs:comment>Levels</rdfs:comment>
        <rdfs:label>table_name:levels</rdfs:label>
    </owl:NamedIndividual>
    


    <!-- http://gtfs.org/table_name_pathways -->


    <owl:NamedIndividual rdf:about="http://gtfs.org/table_name_pathways">
        <rdf:type rdf:resource="http://gtfs.org/TableNameEnum"/>
        <gtfs:hasEnumValue>pathways</gtfs:hasEnumValue>
        <rdfs:comment>Pathways</rdfs:comment>
        <rdfs:label>table_name:pathways</rdfs:label>
    </owl:NamedIndividual>
    


    <!-- http://gtfs.org/table_name_routes -->


    <owl:NamedIndividual rdf:about="http://gtfs.org/table_name_routes">
        <rdf:type rdf:resource="http://gtfs.org/TableNameEnum"/>
        <gtfs:hasEnumValue>routes</gtfs:hasEnumValue>
        <rdfs:comment>Routes</rdfs:comment>
        <rdfs:label>table_name:routes</rdfs:label>
    </owl:NamedIndividual>
    


    <!-- http://gtfs.org/table_name_stop_times -->


    <owl:NamedIndividual rdf:about="http://gtfs.org/table_name_stop_times">
        <rdf:type rdf:resource="http://gtfs.org/TableNameEnum"/>
        <gtfs:hasEnumValue>stop_times</gtfs:hasEnumValue>
        <rdfs:comment>Stop Times</rdfs:comment>
        <rdfs:label>table_name:stop_times</rdfs:label>
    </owl:NamedIndividual>
    


    <!-- http://gtfs.org/table_name_stops -->


    <owl:NamedIndividual rdf:about="http://gtfs.org/table_name_stops">
        <rdf:type rdf:resource="http://gtfs.org/TableNameEnum"/>
        <gtfs:hasEnumValue>stops</gtfs:hasEnumValue>
        <rdfs:comment>Stops</rdfs:comment>
        <rdfs:label>table_name:stops</rdfs:label>
    </owl:NamedIndividual>
    


    <!-- http://gtfs.org/table_name_trips -->


    <owl:NamedIndividual rdf:about="http://gtfs.org/table_name_trips">
        <rdf:type rdf:resource="http://gtfs.org/TableNameEnum"/>
        <gtfs:hasEnumValue>trips</gtfs:hasEnumValue>
        <rdfs:comment>Trips</rdfs:comment>
        <rdfs:label>table_name:trips</rdfs:label>
    </owl:NamedIndividual>
    


    <!-- http://gtfs.org/thursday -->


    <owl:NamedIndividual rdf:about="http://gtfs.org/thursday">
        <rdf:type rdf:resource="http://gtfs.org/Field"/>
        <gtfs:isFieldOf rdf:resource="http://gtfs.org/calendar.txt"/>
        <gtfs:isPresence rdf:resource="http://gtfs.org/Required"/>
        <gtfs:isRequiredIn rdf:resource="http://gtfs.org/calendar.txt"/>
        <gtfs:isType rdf:resource="http://gtfs.org/ThursdayEnum"/>
        <gtfs:hasAdditionalInfo>Enum type field</gtfs:hasAdditionalInfo>
        <rdfs:comment>Functions in the same way as `monday` except applies to Thursdays</rdfs:comment>
        <rdfs:label>thursday</rdfs:label>
    </owl:NamedIndividual>
    


    <!-- http://gtfs.org/thursday_1 -->


    <owl:NamedIndividual rdf:about="http://gtfs.org/thursday_1">
        <rdf:type rdf:resource="http://gtfs.org/ThursdayEnum"/>
        <gtfs:hasEnumValue>1</gtfs:hasEnumValue>
        <rdfs:comment>Functions in the same way as `monday` except applies to Thursdays</rdfs:comment>
        <rdfs:label>thursday:1</rdfs:label>
    </owl:NamedIndividual>
    


    <!-- http://gtfs.org/timeframe_group_id -->


    <owl:NamedIndividual rdf:about="http://gtfs.org/timeframe_group_id">
        <rdf:type rdf:resource="http://gtfs.org/Field"/>
        <gtfs:isFieldOf rdf:resource="http://gtfs.org/timeframes.txt"/>
        <gtfs:isRequiredIn rdf:resource="http://gtfs.org/timeframes.txt"/>
        <gtfs:isType rdf:resource="http://gtfs.org/ID"/>
        <gtfs:hasAdditionalInfo>Field Type: ID</gtfs:hasAdditionalInfo>
        <gtfs:isUniqueID rdf:resource="http://gtfs.org/timeframes.txt"/>
        <rdfs:comment>Identifies a timeframe or set of timeframes.</rdfs:comment>
        <rdfs:label>timeframe_group_id</rdfs:label>
    </owl:NamedIndividual>
    


    <!-- http://gtfs.org/timeframes.txt -->


    <owl:NamedIndividual rdf:about="http://gtfs.org/timeframes.txt">
        <rdf:type rdf:resource="http://gtfs.org/File"/>
        <gtfs:hasField rdf:resource="http://gtfs.org/end_time"/>
        <gtfs:hasField rdf:resource="http://gtfs.org/service_id"/>
        <gtfs:hasField rdf:resource="http://gtfs.org/start_time"/>
        <gtfs:hasField rdf:resource="http://gtfs.org/timeframe_group_id"/>
        <gtfs:isFileOf rdf:resource="http://gtfs.org/GTFS_Static"/>
        <gtfs:isOptionalIn rdf:resource="http://gtfs.org/GTFS_Static"/>
        <rdfs:comment>Date and time periods to use in fare rules for fares that depend on date and time factors.</rdfs:comment>
        <rdfs:label>timeframes.txt</rdfs:label>
    </owl:NamedIndividual>
    


    <!-- http://gtfs.org/timepoint -->


    <owl:NamedIndividual rdf:about="http://gtfs.org/timepoint">
        <rdf:type rdf:resource="http://gtfs.org/Field"/>
        <gtfs:isFieldOf rdf:resource="http://gtfs.org/stop_times.txt"/>
        <gtfs:isPresence rdf:resource="http://gtfs.org/Recommended"/>
        <gtfs:isRecommendedIn rdf:resource="http://gtfs.org/stop_times.txt"/>
        <gtfs:isType rdf:resource="http://gtfs.org/TimepointEnum"/>
        <gtfs:hasAdditionalInfo>Valid options are: 0 - Times are considered approximate. 1 or empty - Times are considered exact.</gtfs:hasAdditionalInfo>
        <rdfs:comment>Indicates if arrival and departure times for a stop are strictly adhered to by the vehicle or if they are instead approximate and/or interpolated times. This field allows a GTFS producer to provide interpolated stop-times, while indicating that the times are approximate. Valid options are: 0 - Times are considered approximate. 1 or empty - Times are considered exact.</rdfs:comment>
        <rdfs:label>timepoint</rdfs:label>
    </owl:NamedIndividual>
    


    <!-- http://gtfs.org/timepoint_0 -->


    <owl:NamedIndividual rdf:about="http://gtfs.org/timepoint_0">
        <rdf:type rdf:resource="http://gtfs.org/TimepointEnum"/>
        <gtfs:hasEnumValue>0</gtfs:hasEnumValue>
        <rdfs:comment>Times are considered approximate</rdfs:comment>
        <rdfs:label>timepoint:0</rdfs:label>
    </owl:NamedIndividual>
    


    <!-- http://gtfs.org/timepoint_1 -->


    <owl:NamedIndividual rdf:about="http://gtfs.org/timepoint_1">
        <rdf:type rdf:resource="http://gtfs.org/TimepointEnum"/>
        <gtfs:hasEnumValue>1</gtfs:hasEnumValue>
        <rdfs:comment>Times are considered exact</rdfs:comment>
        <rdfs:label>timepoint:1</rdfs:label>
    </owl:NamedIndividual>
    


    <!-- http://gtfs.org/to_area_id -->


    <owl:NamedIndividual rdf:about="http://gtfs.org/to_area_id">
        <rdf:type rdf:resource="http://gtfs.org/Field"/>
        <gtfs:isFieldOf rdf:resource="http://gtfs.org/fare_leg_rules.txt"/>
        <gtfs:isOptionalIn rdf:resource="http://gtfs.org/fare_leg_rules.txt"/>
        <gtfs:isType rdf:resource="http://gtfs.org/ID"/>
        <gtfs:hasAdditionalInfo>Foreign ID referencing areas.area_id</gtfs:hasAdditionalInfo>
        <gtfs:isForeignID rdf:resource="http://gtfs.org/fare_leg_rules.txt"/>
        <rdfs:comment>Identifies an arrival area.

If there are no matching fare_leg_rules.to_area_id values to the area_id being filtered, empty fare_leg_rules.to_area_id will be matched by default.

An empty entry in fare_leg_rules.to_area_id corresponds to all areas defined in areas.area_id excluding the ones listed under fare_leg_rules.to_area_id</rdfs:comment>
        <rdfs:label>to_area_id</rdfs:label>
    </owl:NamedIndividual>
    


    <!-- http://gtfs.org/to_leg_group_id -->


    <owl:NamedIndividual rdf:about="http://gtfs.org/to_leg_group_id">
        <rdf:type rdf:resource="http://gtfs.org/Field"/>
        <gtfs:isFieldOf rdf:resource="http://gtfs.org/fare_transfer_rules.txt"/>
        <gtfs:isOptionalIn rdf:resource="http://gtfs.org/fare_transfer_rules.txt"/>
        <gtfs:isType rdf:resource="http://gtfs.org/ID"/>
        <gtfs:hasAdditionalInfo>Foreign ID referencing fare_leg_rules.leg_group_id</gtfs:hasAdditionalInfo>
        <gtfs:isForeignID rdf:resource="http://gtfs.org/fare_transfer_rules.txt"/>
        <rdfs:comment>Identifies a group of post-transfer fare leg rules.

If there are no matching fare_transfer_rules.to_leg_group_id values to the leg_group_id being filtered, empty fare_transfer_rules.to_leg_group_id will be matched by default.

An empty entry in fare_transfer_rules.to_leg_group_id corresponds to all leg groups defined under fare_leg_rules.leg_group_id excluding the ones listed under fare_transfer_rules.to_leg_group_id</rdfs:comment>
        <rdfs:label>to_leg_group_id</rdfs:label>
    </owl:NamedIndividual>
    


    <!-- http://gtfs.org/to_route_id -->


    <owl:NamedIndividual rdf:about="http://gtfs.org/to_route_id">
        <rdf:type rdf:resource="http://gtfs.org/Field"/>
        <gtfs:isFieldOf rdf:resource="http://gtfs.org/transfers.txt"/>
        <gtfs:isOptionalIn rdf:resource="http://gtfs.org/transfers.txt"/>
        <gtfs:isType rdf:resource="http://gtfs.org/ID"/>
        <gtfs:hasAdditionalInfo>Foreign ID referencing `routes.route_id`</gtfs:hasAdditionalInfo>
        <gtfs:isForeignID rdf:resource="http://gtfs.org/transfers.txt"/>
        <rdfs:comment>Identifies a route where a connection ends. If `to_route_id` is defined, the transfer will apply to the departing trip on the route for the given `to_stop_id`. If both `to_trip_id` and `to_route_id` are defined, the `trip_id` must belong to the `route_id`, and `to_trip_id` will take precedence.</rdfs:comment>
        <rdfs:label>to_route_id</rdfs:label>
    </owl:NamedIndividual>
    


    <!-- http://gtfs.org/to_stop_id -->


    <owl:NamedIndividual rdf:about="http://gtfs.org/to_stop_id">
        <rdf:type rdf:resource="http://gtfs.org/Field"/>
        <gtfs:isConditionallyRequiredIn rdf:resource="http://gtfs.org/transfers.txt"/>
        <gtfs:isFieldOf rdf:resource="http://gtfs.org/pathways.txt"/>
        <gtfs:isFieldOf rdf:resource="http://gtfs.org/transfers.txt"/>
        <gtfs:isRequiredIn rdf:resource="http://gtfs.org/pathways.txt"/>
        <gtfs:isType rdf:resource="http://gtfs.org/ID"/>
        <gtfs:hasAdditionalInfo>Foreign ID referencing `stops.stop_id`</gtfs:hasAdditionalInfo>
        <gtfs:hasAdditionalInfo>Foreign ID referencing stops.stop_id</gtfs:hasAdditionalInfo>
        <gtfs:hasCondition>If this field refers to a station, the transfer rule applies to all child stops. Referring to a station is forbidden for transfer_types 4 and 5.</gtfs:hasCondition>
        <gtfs:isForeignID rdf:resource="http://gtfs.org/pathways.txt"/>
        <gtfs:isForeignID rdf:resource="http://gtfs.org/transfers.txt"/>
        <rdfs:comment>Identifies a stop or station where a connection between routes ends. If this field refers to a station, the transfer rule applies to all child stops. Referring to a station is forbidden for transfer_types 4 and 5.</rdfs:comment>
        <rdfs:comment>Location at which the pathway ends.

Must contain a `stop_id` that identifies a platform (`location_type=0` or empty), entrance/exit (`location_type=2`), generic node (`location_type=3`) or boarding area (`location_type=4`).

Values for `stop_id` that identify stations (`location_type=1`) are forbidden.</rdfs:comment>
        <rdfs:label>to_stop_id</rdfs:label>
    </owl:NamedIndividual>
    


    <!-- http://gtfs.org/to_timeframe_group_id -->


    <owl:NamedIndividual rdf:about="http://gtfs.org/to_timeframe_group_id">
        <rdf:type rdf:resource="http://gtfs.org/Field"/>
        <gtfs:isFieldOf rdf:resource="http://gtfs.org/fare_leg_rules.txt"/>
        <gtfs:isOptionalIn rdf:resource="http://gtfs.org/fare_leg_rules.txt"/>
        <gtfs:isType rdf:resource="http://gtfs.org/ID"/>
        <gtfs:hasAdditionalInfo>Foreign ID referencing timeframes.timeframe_group_id</gtfs:hasAdditionalInfo>
        <gtfs:isForeignID rdf:resource="http://gtfs.org/fare_leg_rules.txt"/>
        <rdfs:comment>Defines the timeframe for the fare validation event at the end of the fare leg.
The “end time” of the fare leg is the time at which the event is scheduled to occur. For example, the time could be the scheduled arrival time of a bus at the end of a fare leg where the rider gets off and validates their fare. For the rule matching semantics below, the end time is computed in local time, as determined by Local Time Semantics of timeframes.txt. The stop or station of the fare leg’s arrival event should be used for timezone resolution, where appropriate.
For a fare leg rule that specifies a to_timeframe_group_id, that rule will match a particular leg if there exists at least one record in timeframes.txt where all of the following conditions are true
- The value of timeframe_group_id is equal to the to_timeframe_group_id value.
- The set of days identified by the record’s service_id contains the “current day” of the fare leg’s end time.
- The “time-of-day” of the fare leg&apos;s end time is greater than or equal to the record’s timeframes.start_time value and less than the timeframes.end_time value.
An empty fare_leg_rules.to_timeframe_group_id indicates that the end time of the leg does not affect the matching of this rule.</rdfs:comment>
        <rdfs:label>to_timeframe_group_id</rdfs:label>
    </owl:NamedIndividual>
    


    <!-- http://gtfs.org/to_trip_id -->


    <owl:NamedIndividual rdf:about="http://gtfs.org/to_trip_id">
        <rdf:type rdf:resource="http://gtfs.org/Field"/>
        <gtfs:isConditionallyRequiredIn rdf:resource="http://gtfs.org/transfers.txt"/>
        <gtfs:isFieldOf rdf:resource="http://gtfs.org/transfers.txt"/>
        <gtfs:isType rdf:resource="http://gtfs.org/ID"/>
        <gtfs:hasAdditionalInfo>Foreign ID referencing `trips.trip_id`</gtfs:hasAdditionalInfo>
        <gtfs:hasCondition>REQUIRED if `transfer_type` is `4` or `5`.</gtfs:hasCondition>
        <gtfs:isForeignID rdf:resource="http://gtfs.org/transfers.txt"/>
        <rdfs:comment>Identifies a trip where a connection between routes ends. If `to_trip_id` is defined, the transfer will apply to the departing trip for the given `to_stop_id`. If both `to_trip_id` and `to_route_id` are defined, the `trip_id` must belong to the `route_id`, and `to_trip_id` will take precedence.</rdfs:comment>
        <rdfs:label>to_trip_id</rdfs:label>
    </owl:NamedIndividual>
    


    <!-- http://gtfs.org/transfer_count -->


    <owl:NamedIndividual rdf:about="http://gtfs.org/transfer_count">
        <rdf:type rdf:resource="http://gtfs.org/Field"/>
        <gtfs:isConditionallyForbiddenIn rdf:resource="http://gtfs.org/fare_transfer_rules.txt"/>
        <gtfs:isFieldOf rdf:resource="http://gtfs.org/fare_transfer_rules.txt"/>
        <gtfs:isType rdf:resource="http://gtfs.org/Integer"/>
        <gtfs:hasCondition>Forbidden if fare_transfer_rules.from_leg_group_id does not equal fare_transfer_rules.to_leg_group_id. Required if fare_transfer_rules.from_leg_group_id equals fare_transfer_rules.to_leg_group_id.</gtfs:hasCondition>
        <rdfs:comment>Defines how many consecutive transfers the transfer rule may be applied to.
Valid options are:
-1 - No limit.
1 or more - Defines how many transfers the transfer rule may span.
If a sub-journey matches multiple records with different transfer_counts, then the rule with the minimum transfer_count that is greater than or equal to the current transfer count of the sub-journey is to be selected.</rdfs:comment>
        <rdfs:label>transfer_count</rdfs:label>
    </owl:NamedIndividual>
    


    <!-- http://gtfs.org/transfer_duration -->


    <owl:NamedIndividual rdf:about="http://gtfs.org/transfer_duration">
        <rdf:type rdf:resource="http://gtfs.org/Field"/>
        <gtfs:isFieldOf rdf:resource="http://gtfs.org/fare_attributes.txt"/>
        <gtfs:isOptionalIn rdf:resource="http://gtfs.org/fare_attributes.txt"/>
        <gtfs:isType rdf:resource="http://gtfs.org/Integer"/>
        <gtfs:hasAdditionalInfo>Non-negative integer</gtfs:hasAdditionalInfo>
        <rdfs:comment>Length of time in seconds before a transfer expires. When `transfers`=`0` this field may be used to indicate how long a ticket is valid for or it may be left empty.</rdfs:comment>
        <rdfs:label>transfer_duration</rdfs:label>
    </owl:NamedIndividual>
    


    <!-- http://gtfs.org/transfer_type -->


    <owl:NamedIndividual rdf:about="http://gtfs.org/transfer_type">
        <rdf:type rdf:resource="http://gtfs.org/Field"/>
        <gtfs:isFieldOf rdf:resource="http://gtfs.org/transfers.txt"/>
        <gtfs:isPresence rdf:resource="http://gtfs.org/Required"/>
        <gtfs:isRequiredIn rdf:resource="http://gtfs.org/transfers.txt"/>
        <gtfs:isType rdf:resource="http://gtfs.org/TransferTypeEnum"/>
        <gtfs:hasAdditionalInfo>Valid options are: 0 or empty - Recommended transfer point between routes. 1 - Timed transfer point between two routes. The departing vehicle is expected to wait for the arriving one and leave sufficient time for a rider to transfer between routes. 2 - Transfer requires a minimum amount of time between arrival and departure to ensure a connection. The time required to transfer is specified by min_transfer_time. 3 - Transfers are not possible between routes at the location. 4 - Passengers can transfer from one trip to another by staying onboard the same vehicle (an &apos;in-seat transfer&apos;). 5 - In-seat transfers are not allowed between sequential trips. The passenger must alight from the vehicle and re-board.</gtfs:hasAdditionalInfo>
        <rdfs:comment>Indicates the type of connection for the specified (from_stop_id, to_stop_id) pair.</rdfs:comment>
        <rdfs:label>transfer_type</rdfs:label>
    </owl:NamedIndividual>
    


    <!-- http://gtfs.org/transfer_type_0 -->


    <owl:NamedIndividual rdf:about="http://gtfs.org/transfer_type_0">
        <rdf:type rdf:resource="http://gtfs.org/TransferTypeEnum"/>
        <gtfs:hasEnumValue>0</gtfs:hasEnumValue>
        <rdfs:comment>Recommended transfer point between routes</rdfs:comment>
        <rdfs:label>transfer_type:0</rdfs:label>
    </owl:NamedIndividual>
    


    <!-- http://gtfs.org/transfer_type_1 -->


    <owl:NamedIndividual rdf:about="http://gtfs.org/transfer_type_1">
        <rdf:type rdf:resource="http://gtfs.org/TransferTypeEnum"/>
        <gtfs:hasEnumValue>1</gtfs:hasEnumValue>
        <rdfs:comment>Timed transfer point between two routes</rdfs:comment>
        <rdfs:label>transfer_type:1</rdfs:label>
    </owl:NamedIndividual>
    


    <!-- http://gtfs.org/transfer_type_2 -->


    <owl:NamedIndividual rdf:about="http://gtfs.org/transfer_type_2">
        <rdf:type rdf:resource="http://gtfs.org/TransferTypeEnum"/>
        <gtfs:hasEnumValue>2</gtfs:hasEnumValue>
        <rdfs:comment>Transfer requires a minimum amount of time between arrival and departure to ensure a connection. The time required to transfer is specified by min_transfer_time</rdfs:comment>
        <rdfs:label>transfer_type:2</rdfs:label>
    </owl:NamedIndividual>
    


    <!-- http://gtfs.org/transfer_type_3 -->


    <owl:NamedIndividual rdf:about="http://gtfs.org/transfer_type_3">
        <rdf:type rdf:resource="http://gtfs.org/TransferTypeEnum"/>
        <gtfs:hasEnumValue>3</gtfs:hasEnumValue>
        <rdfs:comment>Transfers are not possible between routes at the location</rdfs:comment>
        <rdfs:label>transfer_type:3</rdfs:label>
    </owl:NamedIndividual>
    


    <!-- http://gtfs.org/transfer_type_4 -->


    <owl:NamedIndividual rdf:about="http://gtfs.org/transfer_type_4">
        <rdf:type rdf:resource="http://gtfs.org/TransferTypeEnum"/>
        <gtfs:hasEnumValue>4</gtfs:hasEnumValue>
        <rdfs:comment>Passengers can transfer from one trip to another by staying onboard the same vehicle (an &apos;in-seat transfer&apos;)</rdfs:comment>
        <rdfs:label>transfer_type:4</rdfs:label>
    </owl:NamedIndividual>
    


    <!-- http://gtfs.org/transfer_type_5 -->


    <owl:NamedIndividual rdf:about="http://gtfs.org/transfer_type_5">
        <rdf:type rdf:resource="http://gtfs.org/TransferTypeEnum"/>
        <gtfs:hasEnumValue>5</gtfs:hasEnumValue>
        <rdfs:comment>In-seat transfers are not allowed between sequential trips. The passenger must alight from the vehicle and re-board</rdfs:comment>
        <rdfs:label>transfer_type:5</rdfs:label>
    </owl:NamedIndividual>
    


    <!-- http://gtfs.org/transfers -->


    <owl:NamedIndividual rdf:about="http://gtfs.org/transfers">
        <rdf:type rdf:resource="http://gtfs.org/Field"/>
        <gtfs:isFieldOf rdf:resource="http://gtfs.org/fare_attributes.txt"/>
        <gtfs:isPresence rdf:resource="http://gtfs.org/Required"/>
        <gtfs:isRequiredIn rdf:resource="http://gtfs.org/fare_attributes.txt"/>
        <gtfs:isType rdf:resource="http://gtfs.org/TransfersEnum"/>
        <gtfs:hasAdditionalInfo>Enum field with options: 0 - No transfers permitted, 1 - Riders may transfer once, 2 - Riders may transfer twice, empty - Unlimited transfers permitted.</gtfs:hasAdditionalInfo>
        <rdfs:comment>Indicates the number of transfers permitted on this fare. Valid options are: 0 - No transfers permitted on this fare. 1 - Riders may transfer once. 2 - Riders may transfer twice. empty - Unlimited transfers are permitted.</rdfs:comment>
        <rdfs:label>transfers</rdfs:label>
    </owl:NamedIndividual>
    


    <!-- http://gtfs.org/transfers.txt -->


    <owl:NamedIndividual rdf:about="http://gtfs.org/transfers.txt">
        <rdf:type rdf:resource="http://gtfs.org/File"/>
        <gtfs:hasField rdf:resource="http://gtfs.org/from_route_id"/>
        <gtfs:hasField rdf:resource="http://gtfs.org/from_stop_id"/>
        <gtfs:hasField rdf:resource="http://gtfs.org/from_trip_id"/>
        <gtfs:hasField rdf:resource="http://gtfs.org/min_transfer_time"/>
        <gtfs:hasField rdf:resource="http://gtfs.org/to_route_id"/>
        <gtfs:hasField rdf:resource="http://gtfs.org/to_stop_id"/>
        <gtfs:hasField rdf:resource="http://gtfs.org/to_trip_id"/>
        <gtfs:hasField rdf:resource="http://gtfs.org/transfer_type"/>
        <gtfs:isFileOf rdf:resource="http://gtfs.org/GTFS_Static"/>
        <gtfs:isOptionalIn rdf:resource="http://gtfs.org/GTFS_Static"/>
        <rdfs:comment>Rules for making connections at transfer points between routes.</rdfs:comment>
        <rdfs:label>transfers.txt</rdfs:label>
    </owl:NamedIndividual>
    


    <!-- http://gtfs.org/transfers_0 -->


    <owl:NamedIndividual rdf:about="http://gtfs.org/transfers_0">
        <rdf:type rdf:resource="http://gtfs.org/TransfersEnum"/>
        <gtfs:hasEnumValue>0</gtfs:hasEnumValue>
        <rdfs:comment>No transfers permitted on this fare</rdfs:comment>
        <rdfs:label>transfers:0</rdfs:label>
    </owl:NamedIndividual>
    


    <!-- http://gtfs.org/transfers_1 -->


    <owl:NamedIndividual rdf:about="http://gtfs.org/transfers_1">
        <rdf:type rdf:resource="http://gtfs.org/TransfersEnum"/>
        <gtfs:hasEnumValue>1</gtfs:hasEnumValue>
        <rdfs:comment>Riders may transfer once</rdfs:comment>
        <rdfs:label>transfers:1</rdfs:label>
    </owl:NamedIndividual>
    


    <!-- http://gtfs.org/transfers_2 -->


    <owl:NamedIndividual rdf:about="http://gtfs.org/transfers_2">
        <rdf:type rdf:resource="http://gtfs.org/TransfersEnum"/>
        <gtfs:hasEnumValue>2</gtfs:hasEnumValue>
        <rdfs:comment>Riders may transfer twice</rdfs:comment>
        <rdfs:label>transfers:2</rdfs:label>
    </owl:NamedIndividual>
    


    <!-- http://gtfs.org/transfers_empty -->


    <owl:NamedIndividual rdf:about="http://gtfs.org/transfers_empty">
        <rdf:type rdf:resource="http://gtfs.org/TransfersEnum"/>
        <gtfs:hasEnumValue>empty</gtfs:hasEnumValue>
        <rdfs:comment>Unlimited transfers permitted</rdfs:comment>
        <rdfs:label>transfers:empty</rdfs:label>
    </owl:NamedIndividual>
    


    <!-- http://gtfs.org/translation -->


    <owl:NamedIndividual rdf:about="http://gtfs.org/translation">
        <rdf:type rdf:resource="http://gtfs.org/Field"/>
        <gtfs:isFieldOf rdf:resource="http://gtfs.org/translations.txt"/>
        <gtfs:isRequiredIn rdf:resource="http://gtfs.org/translations.txt"/>
        <gtfs:isType rdf:resource="http://gtfs.org/Text"/>
        <gtfs:hasAdditionalInfo>The field can store text, URL, email, or phone number data.</gtfs:hasAdditionalInfo>
        <gtfs:isUniqueID rdf:resource="http://gtfs.org/translations.txt"/>
        <rdfs:comment>Translated value.</rdfs:comment>
        <rdfs:label>translation</rdfs:label>
    </owl:NamedIndividual>
    


    <!-- http://gtfs.org/translations.txt -->


    <owl:NamedIndividual rdf:about="http://gtfs.org/translations.txt">
        <rdf:type rdf:resource="http://gtfs.org/File"/>
        <gtfs:hasField rdf:resource="http://gtfs.org/field_name"/>
        <gtfs:hasField rdf:resource="http://gtfs.org/field_value"/>
        <gtfs:hasField rdf:resource="http://gtfs.org/language"/>
        <gtfs:hasField rdf:resource="http://gtfs.org/record_id"/>
        <gtfs:hasField rdf:resource="http://gtfs.org/record_sub_id"/>
        <gtfs:hasField rdf:resource="http://gtfs.org/table_name"/>
        <gtfs:hasField rdf:resource="http://gtfs.org/translation"/>
        <gtfs:isFileOf rdf:resource="http://gtfs.org/GTFS_Static"/>
        <gtfs:isOptionalIn rdf:resource="http://gtfs.org/GTFS_Static"/>
        <rdfs:comment>Translations of customer-facing dataset values.</rdfs:comment>
        <rdfs:label>translations.txt</rdfs:label>
    </owl:NamedIndividual>
    


    <!-- http://gtfs.org/traversal_time -->


    <owl:NamedIndividual rdf:about="http://gtfs.org/traversal_time">
        <rdf:type rdf:resource="http://gtfs.org/Field"/>
        <gtfs:isFieldOf rdf:resource="http://gtfs.org/pathways.txt"/>
        <gtfs:isOptionalIn rdf:resource="http://gtfs.org/pathways.txt"/>
        <gtfs:isType rdf:resource="http://gtfs.org/Integer"/>
        <gtfs:hasAdditionalInfo>Positive integer</gtfs:hasAdditionalInfo>
        <rdfs:comment>Average time in seconds needed to walk through the pathway from the origin location (defined in `from_stop_id`) to the destination location (defined in `to_stop_id`). This field is recommended for moving sidewalks (`pathway_mode=3`), escalators (`pathway_mode=4`) and elevator (`pathway_mode=5`).</rdfs:comment>
        <rdfs:label>traversal_time</rdfs:label>
    </owl:NamedIndividual>
    


    <!-- http://gtfs.org/trip_headsign -->


    <owl:NamedIndividual rdf:about="http://gtfs.org/trip_headsign">
        <rdf:type rdf:resource="http://gtfs.org/Field"/>
        <gtfs:isFieldOf rdf:resource="http://gtfs.org/trips.txt"/>
        <gtfs:isOptionalIn rdf:resource="http://gtfs.org/trips.txt"/>
        <gtfs:isType rdf:resource="http://gtfs.org/Text"/>
        <gtfs:hasAdditionalInfo>Text that appears on signage identifying the trip&apos;s destination to riders. Should be used to distinguish between different patterns of service on the same route. If the headsign changes during a trip, values for trip_headsign may be overridden by defining values in stop_times.stop_headsign for specific stop_times along the trip.</gtfs:hasAdditionalInfo>
        <rdfs:comment>Text that appears on signage identifying the trip&apos;s destination to riders. Should be used to distinguish between different patterns of service on the same route. If the headsign changes during a trip, values for trip_headsign may be overridden by defining values in stop_times.stop_headsign for specific stop_times along the trip.</rdfs:comment>
        <rdfs:label>trip_headsign</rdfs:label>
    </owl:NamedIndividual>
    


    <!-- http://gtfs.org/trip_id -->


    <owl:NamedIndividual rdf:about="http://gtfs.org/trip_id">
        <rdf:type rdf:resource="http://gtfs.org/Field"/>
        <gtfs:isFieldOf rdf:resource="http://gtfs.org/attributions.txt"/>
        <gtfs:isFieldOf rdf:resource="http://gtfs.org/frequencies.txt"/>
        <gtfs:isFieldOf rdf:resource="http://gtfs.org/stop_times.txt"/>
        <gtfs:isFieldOf rdf:resource="http://gtfs.org/trips.txt"/>
        <gtfs:isOptionalIn rdf:resource="http://gtfs.org/attributions.txt"/>
        <gtfs:isRequiredIn rdf:resource="http://gtfs.org/frequencies.txt"/>
        <gtfs:isRequiredIn rdf:resource="http://gtfs.org/stop_times.txt"/>
        <gtfs:isRequiredIn rdf:resource="http://gtfs.org/trips.txt"/>
        <gtfs:isType rdf:resource="http://gtfs.org/ID"/>
        <gtfs:hasAdditionalInfo>Foreign ID referencing `trips.trip_id`</gtfs:hasAdditionalInfo>
        <gtfs:hasAdditionalInfo>Foreign ID referencing trips.trip_id</gtfs:hasAdditionalInfo>
        <gtfs:hasAdditionalInfo>Unique ID</gtfs:hasAdditionalInfo>
        <gtfs:isForeignID rdf:resource="http://gtfs.org/attributions.txt"/>
        <gtfs:isForeignID rdf:resource="http://gtfs.org/frequencies.txt"/>
        <gtfs:isForeignID rdf:resource="http://gtfs.org/stop_times.txt"/>
        <gtfs:isUniqueID rdf:resource="http://gtfs.org/trips.txt"/>
        <rdfs:comment>Functions in the same way as `agency_id` except the attribution applies to a trip. Multiple attributions may apply to the same trip.</rdfs:comment>
        <rdfs:comment>Identifies a trip to which the specified headway of service applies.</rdfs:comment>
        <rdfs:comment>Identifies a trip.</rdfs:comment>
        <rdfs:label>trip_id</rdfs:label>
    </owl:NamedIndividual>
    


    <!-- http://gtfs.org/trip_short_name -->


    <owl:NamedIndividual rdf:about="http://gtfs.org/trip_short_name">
        <rdf:type rdf:resource="http://gtfs.org/Field"/>
        <gtfs:isFieldOf rdf:resource="http://gtfs.org/trips.txt"/>
        <gtfs:isOptionalIn rdf:resource="http://gtfs.org/trips.txt"/>
        <gtfs:isType rdf:resource="http://gtfs.org/Text"/>
        <gtfs:hasAdditionalInfo>Public facing text used to identify the trip to riders.</gtfs:hasAdditionalInfo>
        <rdfs:comment>Public facing text used to identify the trip to riders, for instance, to identify train numbers for commuter rail trips. If riders do not commonly rely on trip names, `trip_short_name` should be empty. A `trip_short_name` value, if provided, should uniquely identify a trip within a service day; it should not be used for destination names or limited/express designations.</rdfs:comment>
        <rdfs:label>trip_short_name</rdfs:label>
    </owl:NamedIndividual>
    


    <!-- http://gtfs.org/trips.txt -->


    <owl:NamedIndividual rdf:about="http://gtfs.org/trips.txt">
        <rdf:type rdf:resource="http://gtfs.org/File"/>
        <gtfs:hasField rdf:resource="http://gtfs.org/bikes_allowed"/>
        <gtfs:hasField rdf:resource="http://gtfs.org/block_id"/>
        <gtfs:hasField rdf:resource="http://gtfs.org/direction_id"/>
        <gtfs:hasField rdf:resource="http://gtfs.org/route_id"/>
        <gtfs:hasField rdf:resource="http://gtfs.org/service_id"/>
        <gtfs:hasField rdf:resource="http://gtfs.org/shape_id"/>
        <gtfs:hasField rdf:resource="http://gtfs.org/trip_headsign"/>
        <gtfs:hasField rdf:resource="http://gtfs.org/trip_id"/>
        <gtfs:hasField rdf:resource="http://gtfs.org/trip_short_name"/>
        <gtfs:hasField rdf:resource="http://gtfs.org/wheelchair_accessible"/>
        <gtfs:isFileOf rdf:resource="http://gtfs.org/GTFS_Static"/>
        <gtfs:isRequiredIn rdf:resource="http://gtfs.org/GTFS_Static"/>
        <rdfs:comment>Trips for each route. A trip is a sequence of two or more stops that occur during a specific time period.</rdfs:comment>
        <rdfs:label>trips.txt</rdfs:label>
    </owl:NamedIndividual>
    


    <!-- http://gtfs.org/tts_stop_name -->


    <owl:NamedIndividual rdf:about="http://gtfs.org/tts_stop_name">
        <rdf:type rdf:resource="http://gtfs.org/Field"/>
        <gtfs:isFieldOf rdf:resource="http://gtfs.org/stops.txt"/>
        <gtfs:isOptionalIn rdf:resource="http://gtfs.org/stops.txt"/>
        <gtfs:isType rdf:resource="http://gtfs.org/Text"/>
        <gtfs:hasAdditionalInfo>This field provides a text representation of the stop name for text-to-speech purposes.</gtfs:hasAdditionalInfo>
        <rdfs:comment>Readable version of the `stop_name`. See &quot;Text-to-speech field&quot; in the Term Definitions for more.</rdfs:comment>
        <rdfs:label>tts_stop_name</rdfs:label>
    </owl:NamedIndividual>
    


    <!-- http://gtfs.org/tuesday -->


    <owl:NamedIndividual rdf:about="http://gtfs.org/tuesday">
        <rdf:type rdf:resource="http://gtfs.org/Field"/>
        <gtfs:isFieldOf rdf:resource="http://gtfs.org/calendar.txt"/>
        <gtfs:isPresence rdf:resource="http://gtfs.org/Required"/>
        <gtfs:isRequiredIn rdf:resource="http://gtfs.org/calendar.txt"/>
        <gtfs:isType rdf:resource="http://gtfs.org/TuesdayEnum"/>
        <gtfs:hasAdditionalInfo>Enum type field</gtfs:hasAdditionalInfo>
        <rdfs:comment>Functions in the same way as `monday` except applies to Tuesdays</rdfs:comment>
        <rdfs:label>tuesday</rdfs:label>
    </owl:NamedIndividual>
    


    <!-- http://gtfs.org/tuesday_0 -->


    <owl:NamedIndividual rdf:about="http://gtfs.org/tuesday_0">
        <rdf:type rdf:resource="http://gtfs.org/TuesdayEnum"/>
        <gtfs:hasEnumValue>0</gtfs:hasEnumValue>
        <rdfs:comment>Functions in the same way as &apos;monday&apos; except applies to Tuesdays</rdfs:comment>
        <rdfs:label>tuesday:0</rdfs:label>
    </owl:NamedIndividual>
    


    <!-- http://gtfs.org/wednesday -->


    <owl:NamedIndividual rdf:about="http://gtfs.org/wednesday">
        <rdf:type rdf:resource="http://gtfs.org/Field"/>
        <gtfs:isFieldOf rdf:resource="http://gtfs.org/calendar.txt"/>
        <gtfs:isPresence rdf:resource="http://gtfs.org/Required"/>
        <gtfs:isRequiredIn rdf:resource="http://gtfs.org/calendar.txt"/>
        <gtfs:isType rdf:resource="http://gtfs.org/WednesdayEnum"/>
        <gtfs:hasAdditionalInfo>Enum type field</gtfs:hasAdditionalInfo>
        <rdfs:comment>Functions in the same way as `monday` except applies to Wednesdays</rdfs:comment>
        <rdfs:label>wednesday</rdfs:label>
    </owl:NamedIndividual>
    


    <!-- http://gtfs.org/wednesday_1 -->


    <owl:NamedIndividual rdf:about="http://gtfs.org/wednesday_1">
        <rdf:type rdf:resource="http://gtfs.org/WednesdayEnum"/>
        <gtfs:hasEnumValue>1</gtfs:hasEnumValue>
        <rdfs:comment>Functions in the same way as `monday` except applies to Wednesdays</rdfs:comment>
        <rdfs:label>wednesday:1</rdfs:label>
    </owl:NamedIndividual>
    


    <!-- http://gtfs.org/wheelchair_accessible -->


    <owl:NamedIndividual rdf:about="http://gtfs.org/wheelchair_accessible">
        <rdf:type rdf:resource="http://gtfs.org/Field"/>
        <gtfs:isFieldOf rdf:resource="http://gtfs.org/trips.txt"/>
        <gtfs:isOptionalIn rdf:resource="http://gtfs.org/trips.txt"/>
        <gtfs:isPresence rdf:resource="http://gtfs.org/Optional"/>
        <gtfs:isType rdf:resource="http://gtfs.org/WheelchairAccessibleEnum"/>
        <gtfs:hasAdditionalInfo>Enum field with options 0, 1, 2</gtfs:hasAdditionalInfo>
        <rdfs:comment>Indicates wheelchair accessibility. Valid options are: 0 or empty - No accessibility information for the trip. 1 - Vehicle being used on this particular trip can accommodate at least one rider in a wheelchair. 2 - No riders in wheelchairs can be accommodated on this trip.</rdfs:comment>
        <rdfs:label>wheelchair_accessible</rdfs:label>
    </owl:NamedIndividual>
    


    <!-- http://gtfs.org/wheelchair_accessible_0 -->


    <owl:NamedIndividual rdf:about="http://gtfs.org/wheelchair_accessible_0">
        <rdf:type rdf:resource="http://gtfs.org/WheelchairAccessibleEnum"/>
        <gtfs:hasEnumValue>0</gtfs:hasEnumValue>
        <rdfs:comment>No accessibility information for the trip</rdfs:comment>
        <rdfs:label>wheelchair_accessible:0</rdfs:label>
    </owl:NamedIndividual>
    


    <!-- http://gtfs.org/wheelchair_accessible_1 -->


    <owl:NamedIndividual rdf:about="http://gtfs.org/wheelchair_accessible_1">
        <rdf:type rdf:resource="http://gtfs.org/WheelchairAccessibleEnum"/>
        <gtfs:hasEnumValue>1</gtfs:hasEnumValue>
        <rdfs:comment>Vehicle can accommodate at least one rider in a wheelchair</rdfs:comment>
        <rdfs:label>wheelchair_accessible:1</rdfs:label>
    </owl:NamedIndividual>
    


    <!-- http://gtfs.org/wheelchair_accessible_2 -->


    <owl:NamedIndividual rdf:about="http://gtfs.org/wheelchair_accessible_2">
        <rdf:type rdf:resource="http://gtfs.org/WheelchairAccessibleEnum"/>
        <gtfs:hasEnumValue>2</gtfs:hasEnumValue>
        <rdfs:comment>No riders in wheelchairs can be accommodated on this trip</rdfs:comment>
        <rdfs:label>wheelchair_accessible:2</rdfs:label>
    </owl:NamedIndividual>
    


    <!-- http://gtfs.org/wheelchair_boarding -->


    <owl:NamedIndividual rdf:about="http://gtfs.org/wheelchair_boarding">
        <rdf:type rdf:resource="http://gtfs.org/Field"/>
        <gtfs:isFieldOf rdf:resource="http://gtfs.org/stops.txt"/>
        <gtfs:isOptionalIn rdf:resource="http://gtfs.org/stops.txt"/>
        <gtfs:isPresence rdf:resource="http://gtfs.org/Optional"/>
        <gtfs:isType rdf:resource="http://gtfs.org/WheelchairBoardingEnum"/>
        <rdfs:comment>Indicates whether wheelchair boardings are possible from the location. Valid options are: For parentless stops: 0 or empty - No accessibility information for the stop. 1 - Some vehicles at this stop can be boarded by a rider in a wheelchair. 2 - Wheelchair boarding is not possible at this stop. For child stops: 0 or empty - Stop will inherit its wheelchair_boarding behavior from the parent station, if specified in the parent. 1 - There exists some accessible path from outside the station to the specific stop/platform. 2 - There exists no accessible path from outside the station to the specific stop/platform. For station entrances/exits: 0 or empty - Station entrance will inherit its wheelchair_boarding behavior from the parent station, if specified for the parent. 1 - Station entrance is wheelchair accessible. 2 - No accessible path from station entrance to stops/platforms.</rdfs:comment>
        <rdfs:label>wheelchair_boarding</rdfs:label>
    </owl:NamedIndividual>
    


    <!-- http://gtfs.org/wheelchair_boarding_0 -->


    <owl:NamedIndividual rdf:about="http://gtfs.org/wheelchair_boarding_0">
        <rdf:type rdf:resource="http://gtfs.org/WheelchairBoardingEnum"/>
        <gtfs:hasEnumValue>0</gtfs:hasEnumValue>
        <rdfs:comment>No accessibility information for the stop</rdfs:comment>
        <rdfs:label>wheelchair_boarding:0</rdfs:label>
    </owl:NamedIndividual>
    


    <!-- http://gtfs.org/wheelchair_boarding_1 -->


    <owl:NamedIndividual rdf:about="http://gtfs.org/wheelchair_boarding_1">
        <rdf:type rdf:resource="http://gtfs.org/WheelchairBoardingEnum"/>
        <gtfs:hasEnumValue>1</gtfs:hasEnumValue>
        <rdfs:comment>Some vehicles at this stop can be boarded by a rider in a wheelchair</rdfs:comment>
        <rdfs:label>wheelchair_boarding:1</rdfs:label>
    </owl:NamedIndividual>
    


    <!-- http://gtfs.org/wheelchair_boarding_2 -->


    <owl:NamedIndividual rdf:about="http://gtfs.org/wheelchair_boarding_2">
        <rdf:type rdf:resource="http://gtfs.org/WheelchairBoardingEnum"/>
        <gtfs:hasEnumValue>2</gtfs:hasEnumValue>
        <rdfs:comment>Wheelchair boarding is not possible at this stop</rdfs:comment>
        <rdfs:label>wheelchair_boarding:2</rdfs:label>
    </owl:NamedIndividual>
    


    <!-- http://gtfs.org/zone_id -->


    <owl:NamedIndividual rdf:about="http://gtfs.org/zone_id">
        <rdf:type rdf:resource="http://gtfs.org/Field"/>
        <gtfs:isConditionallyRequiredIn rdf:resource="http://gtfs.org/stops.txt"/>
        <gtfs:isFieldOf rdf:resource="http://gtfs.org/stops.txt"/>
        <gtfs:isType rdf:resource="http://gtfs.org/ID"/>
        <gtfs:hasAdditionalInfo>If this record represents a station or station entrance, the `zone_id` is ignored.</gtfs:hasAdditionalInfo>
        <gtfs:hasCondition>Required if providing fare information using fare_rules.txt, Optional otherwise</gtfs:hasCondition>
        <rdfs:comment>Identifies the fare zone for a stop. If this record represents a station or station entrance, the `zone_id` is ignored.</rdfs:comment>
        <rdfs:label>zone_id</rdfs:label>
    </owl:NamedIndividual>
    


    <!-- 
    ///////////////////////////////////////////////////////////////////////////////////////
    //
    // Annotations
    //
    ///////////////////////////////////////////////////////////////////////////////////////
     -->


    <rdf:Description rdf:about="http://gtfs.org/BikesAllowedEnum">
        <rdfs:comment>Enumeration class for bikes_allowed</rdfs:comment>
        <rdfs:label>BikesAllowedEnum</rdfs:label>
    </rdf:Description>
    <rdf:Description rdf:about="http://gtfs.org/ContinuousDropOffEnum">
        <rdfs:comment>Enumeration class for continuous_drop_off</rdfs:comment>
        <rdfs:label>ContinuousDropOffEnum</rdfs:label>
    </rdf:Description>
    <rdf:Description rdf:about="http://gtfs.org/ContinuousPickupEnum">
        <rdfs:comment>Enumeration class for continuous_pickup</rdfs:comment>
        <rdfs:label>ContinuousPickupEnum</rdfs:label>
    </rdf:Description>
    <rdf:Description rdf:about="http://gtfs.org/CurrencyAmount">
        <rdfs:comment xml:lang="en">A decimal value indicating a currency amount. The number of decimal places is specified by ISO 4217 for the accompanying Currency code. All financial calculations should be processed as decimal, currency, or another equivalent type suitable for financial calculations depending on the programming language used to consume data. Processing currency amounts as float is discouraged due to gains or losses of money during calculations.</rdfs:comment>
        <rdfs:label xml:lang="en">CurrencyAmount</rdfs:label>
    </rdf:Description>
    <rdf:Description rdf:about="http://gtfs.org/Date">
        <rdfs:comment xml:lang="en">Service day in the YYYYMMDD format. Since time within a service day may be above 24:00:00, a service day may contain information for the subsequent day(s).</rdfs:comment>
        <rdfs:label xml:lang="en">Date</rdfs:label>
    </rdf:Description>
    <rdf:Description rdf:about="http://gtfs.org/DirectionIdEnum">
        <rdfs:comment>Enumeration class for direction_id</rdfs:comment>
        <rdfs:label>DirectionIdEnum</rdfs:label>
    </rdf:Description>
    <rdf:Description rdf:about="http://gtfs.org/DropOffTypeEnum">
        <rdfs:comment>Enumeration class for drop_off_type</rdfs:comment>
        <rdfs:label>DropOffTypeEnum</rdfs:label>
    </rdf:Description>
    <rdf:Description rdf:about="http://gtfs.org/DurationLimitTypeEnum">
        <rdfs:comment>Enumeration class for duration_limit_type</rdfs:comment>
        <rdfs:label>DurationLimitTypeEnum</rdfs:label>
    </rdf:Description>
    <rdf:Description rdf:about="http://gtfs.org/Email">
        <rdfs:comment xml:lang="en">An email address.</rdfs:comment>
        <rdfs:label xml:lang="en">Email</rdfs:label>
    </rdf:Description>
    <rdf:Description rdf:about="http://gtfs.org/ExactTimesEnum">
        <rdfs:comment>Enumeration class for exact_times</rdfs:comment>
        <rdfs:label>ExactTimesEnum</rdfs:label>
    </rdf:Description>
    <rdf:Description rdf:about="http://gtfs.org/ExceptionTypeEnum">
        <rdfs:comment>Enumeration class for exception_type</rdfs:comment>
        <rdfs:label>ExceptionTypeEnum</rdfs:label>
    </rdf:Description>
    <rdf:Description rdf:about="http://gtfs.org/FareMediaTypeEnum">
        <rdfs:comment>Enumeration class for fare_media_type</rdfs:comment>
        <rdfs:label>FareMediaTypeEnum</rdfs:label>
    </rdf:Description>
    <rdf:Description rdf:about="http://gtfs.org/FareTransferTypeEnum">
        <rdfs:comment>Enumeration class for fare_transfer_type</rdfs:comment>
        <rdfs:label>FareTransferTypeEnum</rdfs:label>
    </rdf:Description>
    <rdf:Description rdf:about="http://gtfs.org/Float">
        <rdfs:comment xml:lang="en">A floating point number.</rdfs:comment>
        <rdfs:label xml:lang="en">Float</rdfs:label>
    </rdf:Description>
    <rdf:Description rdf:about="http://gtfs.org/FridayEnum">
        <rdfs:comment>Enumeration class for friday</rdfs:comment>
        <rdfs:label>FridayEnum</rdfs:label>
    </rdf:Description>
    <rdf:Description rdf:about="http://gtfs.org/ID">
        <rdfs:comment xml:lang="en">An ID field value is an internal ID, not intended to be shown to riders, and is a sequence of any UTF-8 characters. Using only printable ASCII characters is recommended. An ID is labeled &quot;unique ID&quot; when it must be unique within a file. IDs defined in one .txt file are often referenced in another .txt file. IDs that reference an ID in another table are labeled &quot;foreign ID&quot;.</rdfs:comment>
        <rdfs:label xml:lang="en">ID</rdfs:label>
    </rdf:Description>
    <rdf:Description rdf:about="http://gtfs.org/Integer">
        <rdfs:comment>An integer</rdfs:comment>
        <rdfs:label xml:lang="en">Integer</rdfs:label>
    </rdf:Description>
    <rdf:Description rdf:about="http://gtfs.org/IsAuthorityEnum">
        <rdfs:comment>Enumeration class for is_authority</rdfs:comment>
        <rdfs:label>IsAuthorityEnum</rdfs:label>
    </rdf:Description>
    <rdf:Description rdf:about="http://gtfs.org/IsBidirectionalEnum">
        <rdfs:comment>Enumeration class for is_bidirectional</rdfs:comment>
        <rdfs:label>IsBidirectionalEnum</rdfs:label>
    </rdf:Description>
    <rdf:Description rdf:about="http://gtfs.org/IsOperatorEnum">
        <rdfs:comment>Enumeration class for is_operator</rdfs:comment>
        <rdfs:label>IsOperatorEnum</rdfs:label>
    </rdf:Description>
    <rdf:Description rdf:about="http://gtfs.org/IsProducerEnum">
        <rdfs:comment>Enumeration class for is_producer</rdfs:comment>
        <rdfs:label>IsProducerEnum</rdfs:label>
    </rdf:Description>
    <rdf:Description rdf:about="http://gtfs.org/LanguageCode">
        <rdfs:comment>An IETF BCP 47 language code. For an introduction to IETF BCP 47, refer to http://www.rfc-editor.org/rfc/bcp/bcp47.txt and</rdfs:comment>
        <rdfs:label xml:lang="en">LanguageCode</rdfs:label>
    </rdf:Description>
    <rdf:Description rdf:about="http://gtfs.org/Latitude">
        <rdfs:comment>WGS84 latitude in decimal degrees. The value must be greater than or equal to -90.0 and less than or equal to 90.0.</rdfs:comment>
        <rdfs:label xml:lang="en">Latitude</rdfs:label>
    </rdf:Description>
    <rdf:Description rdf:about="http://gtfs.org/LocationTypeEnum">
        <rdfs:comment>Enumeration class for location_type</rdfs:comment>
        <rdfs:label>LocationTypeEnum</rdfs:label>
    </rdf:Description>
    <rdf:Description rdf:about="http://gtfs.org/Longitude">
        <rdfs:comment>WGS84 longitude in decimal degrees. The value must be greater than or equal to -90.0 and less than or equal to 90.0.</rdfs:comment>
        <rdfs:label xml:lang="en">Longitude</rdfs:label>
    </rdf:Description>
    <rdf:Description rdf:about="http://gtfs.org/MondayEnum">
        <rdfs:comment>Enumeration class for monday</rdfs:comment>
        <rdfs:label>MondayEnum</rdfs:label>
    </rdf:Description>
    <rdf:Description rdf:about="http://gtfs.org/PathwayModeEnum">
        <rdfs:comment>Enumeration class for pathway_mode</rdfs:comment>
        <rdfs:label>PathwayModeEnum</rdfs:label>
    </rdf:Description>
    <rdf:Description rdf:about="http://gtfs.org/PaymentMethodEnum">
        <rdfs:comment>Enumeration class for payment_method</rdfs:comment>
        <rdfs:label>PaymentMethodEnum</rdfs:label>
    </rdf:Description>
    <rdf:Description rdf:about="http://gtfs.org/PhoneNumber">
        <rdfs:comment>A phone number</rdfs:comment>
        <rdfs:label xml:lang="en">PhoneNumber</rdfs:label>
    </rdf:Description>
    <rdf:Description rdf:about="http://gtfs.org/PickupTypeEnum">
        <rdfs:comment>Enumeration class for pickup_type</rdfs:comment>
        <rdfs:label>PickupTypeEnum</rdfs:label>
    </rdf:Description>
    <rdf:Description rdf:about="http://gtfs.org/Recommended">
        <rdfs:comment>The field or file may be omitted from the dataset, but it is a best practice to include it. Before omitting this field or file, the best practice should be carefully evaluated and the full implications of omission should be understood.</rdfs:comment>
        <rdfs:label xml:lang="en">Recommended</rdfs:label>
    </rdf:Description>
    <rdf:Description rdf:about="http://gtfs.org/RouteTypeEnum">
        <rdfs:comment>Enumeration class for route_type</rdfs:comment>
        <rdfs:label>RouteTypeEnum</rdfs:label>
    </rdf:Description>
    <rdf:Description rdf:about="http://gtfs.org/SaturdayEnum">
        <rdfs:comment>Enumeration class for saturday</rdfs:comment>
        <rdfs:label>SaturdayEnum</rdfs:label>
    </rdf:Description>
    <rdf:Description rdf:about="http://gtfs.org/SundayEnum">
        <rdfs:comment>Enumeration class for sunday</rdfs:comment>
        <rdfs:label>SundayEnum</rdfs:label>
    </rdf:Description>
    <rdf:Description rdf:about="http://gtfs.org/TableNameEnum">
        <rdfs:comment>Enumeration class for table_name</rdfs:comment>
        <rdfs:label>TableNameEnum</rdfs:label>
    </rdf:Description>
    <rdf:Description rdf:about="http://gtfs.org/Text">
        <rdfs:label xml:lang="en">Text</rdfs:label>
    </rdf:Description>
    <rdf:Description rdf:about="http://gtfs.org/ThursdayEnum">
        <rdfs:comment>Enumeration class for thursday</rdfs:comment>
        <rdfs:label>ThursdayEnum</rdfs:label>
    </rdf:Description>
    <rdf:Description rdf:about="http://gtfs.org/Time">
        <rdfs:comment>Time in the HH:MM:SS format (H:MM:SS is also accepted). The time is measured from &quot;noon minus 12h&quot; of the service day (effectively midnight except for days on which daylight savings time changes occur). For times occurring after midnight on the service day, enter the time as a value greater than 24:00:00 in HH:MM:SS.</rdfs:comment>
        <rdfs:label xml:lang="en">Time</rdfs:label>
    </rdf:Description>
    <rdf:Description rdf:about="http://gtfs.org/TimeZone">
        <rdfs:comment>TZ timezone from the https://www.iana.org/time-zones. Timezone names never contain the space character but may contain an underscore. Refer to http://en.wikipedia.org/wiki/List_of_tz_zones for a list of valid values.</rdfs:comment>
        <rdfs:label xml:lang="en">TimeZone</rdfs:label>
    </rdf:Description>
    <rdf:Description rdf:about="http://gtfs.org/TimepointEnum">
        <rdfs:comment>Enumeration class for timepoint</rdfs:comment>
        <rdfs:label>TimepointEnum</rdfs:label>
    </rdf:Description>
    <rdf:Description rdf:about="http://gtfs.org/TransferTypeEnum">
        <rdfs:comment>Enumeration class for transfer_type</rdfs:comment>
        <rdfs:label>TransferTypeEnum</rdfs:label>
    </rdf:Description>
    <rdf:Description rdf:about="http://gtfs.org/TransfersEnum">
        <rdfs:comment>Enumeration class for transfers</rdfs:comment>
        <rdfs:label>TransfersEnum</rdfs:label>
    </rdf:Description>
    <rdf:Description rdf:about="http://gtfs.org/TuesdayEnum">
        <rdfs:comment>Enumeration class for tuesday</rdfs:comment>
        <rdfs:label>TuesdayEnum</rdfs:label>
    </rdf:Description>
    <rdf:Description rdf:about="http://gtfs.org/URL">
        <rdfs:comment>A fully qualified URL that includes http:// or https://, and any special characters in the URL must be correctly escaped. See the following http://www.w3.org/Addressing/URL/4_URI_Recommentations.html for a description of how to create fully qualified URL values.</rdfs:comment>
        <rdfs:label xml:lang="en">URL</rdfs:label>
    </rdf:Description>
    <rdf:Description rdf:about="http://gtfs.org/WednesdayEnum">
        <rdfs:comment>Enumeration class for wednesday</rdfs:comment>
        <rdfs:label>WednesdayEnum</rdfs:label>
    </rdf:Description>
    <rdf:Description rdf:about="http://gtfs.org/WheelchairAccessibleEnum">
        <rdfs:comment>Enumeration class for wheelchair_accessible</rdfs:comment>
        <rdfs:label>WheelchairAccessibleEnum</rdfs:label>
    </rdf:Description>
    <rdf:Description rdf:about="http://gtfs.org/WheelchairBoardingEnum">
        <rdfs:comment>Enumeration class for wheelchair_boarding</rdfs:comment>
        <rdfs:label>WheelchairBoardingEnum</rdfs:label>
    </rdf:Description>
</rdf:RDF>



<!-- Generated by the OWL API (version 5.1.18) https://github.com/owlcs/owlapi/ -->


